<?xml version="1.0"?>
<rdf:RDF xmlns="http://purl.org/iot/ontology/fiesta-iot#"
     xml:base="http://purl.org/iot/ontology/fiesta-iot"
     xmlns:onemtom="http://www.onem2m.org/ontology/Base_Ontology/base_ontology#"
     xmlns:qudt="http://data.qudt.org/qudt/owl/1.0.0/unit.owl#"
     xmlns:iot-lite="http://purl.oclc.org/NET/UNIS/fiware/iot-lite#"
     xmlns:qu="http://purl.org/NET/ssnx/qu/qu#"
     xmlns:owl="http://www.w3.org/2002/07/owl#"
     xmlns:ns="http://creativecommons.org/ns#"
     xmlns:swrlb="http://www.w3.org/2003/11/swrlb#"
     xmlns:swrl="http://www.w3.org/2003/11/swrl#"
     xmlns:fiesta-iot="http://purl.org/iot/ontology/fiesta-iot#"
     xmlns:xsd="http://www.w3.org/2001/XMLSchema#"
     xmlns:rdfs="http://www.w3.org/2000/01/rdf-schema#"
     xmlns:swrla="http://swrl.stanford.edu/ontologies/3.3/swrla.owl#"
     xmlns:ssn="http://purl.oclc.org/NET/ssnx/ssn#"
     xmlns:geo="http://www.w3.org/2003/01/geo/wgs84_pos#"
     xmlns:rdf="http://www.w3.org/1999/02/22-rdf-syntax-ns#"
     xmlns:xml="http://www.w3.org/XML/1998/namespace"
     xmlns:dcterms="http://purl.org/dc/terms/"
     xmlns:dul="http://www.loa.istc.cnr.it/ontologies/DUL.owl#"
     xmlns:time="http://www.w3.org/2006/time#"
     xmlns:mthreelite="http://purl.org/iot/vocab/m3-lite#"
     xmlns:vann="http://purl.org/vocab/vann/"
     xmlns:dc="http://purl.org/dc/elements/1.1/">
    <owl:Ontology rdf:about="http://purl.org/iot/ontology/fiesta-iot#">
        <dc:creator xml:lang="en">Luis Sanchez, UC, Santander</dc:creator>
        <dc:contributor xml:lang="en">(Past) Amelie Gyrard, NUIG, Galway</dc:contributor>
        <dc:rights>Copyright EU H2020 FIESTA-IoT</dc:rights>
        <dc:creator xml:lang="en">David Gomez, UC, Santander</dc:creator>
        <dc:description rdf:resource="http://ontology.fiesta-iot.eu/ontologyDocs/resourcegraph.png"/>
        <rdfs:label rdf:datatype="http://www.w3.org/2001/XMLSchema#string">FIESTA-IoT</rdfs:label>
        <dcterms:bibliographicCitation xml:lang="en">R. Agarwal, D. Fernandez, T. Elsaleh, A. Gyrard, J. Lanza, L. Sanchez, N. Georgantas, V. Issarny, &quot;Unified IoT Ontology to Enable Interoperability and Federation of Testbeds&quot;, 3rd IEEE WF-IoT, Reston, VA, USA, 12-14 December 2016. (https://hal.inria.fr/hal-01386917/document)</dcterms:bibliographicCitation>
        <dc:contributor xml:lang="en">(Past) Garvita Bajaj, Inria, Paris</dc:contributor>
        <dcterms:bibliographicCitation xml:lang="en">FIESTA-IoT Consortium (R. Agarwal editor), &quot;Deliverable D3.1.1 Semantic Models for Testbeds, Interoperability and Mobility Support, and Best Practices&quot;, project FIESTA-IoT deliverable, 2016.</dcterms:bibliographicCitation>
        <dc:creator xml:lang="en">Rachit Agarwal, Inria, Paris</dc:creator>
        <dcterms:modified rdf:datatype="http://www.w3.org/2001/XMLSchema#date">2017-07-29</dcterms:modified>
        <dc:description rdf:resource="http://ontology.fiesta-iot.eu/ontologyDocs/fiesta-iot.png"/>
        <owl:versionInfo>3.0</owl:versionInfo>
        <vann:preferredNamespacePrefix>fiesta-iot</vann:preferredNamespacePrefix>
        <dc:creator xml:lang="en">Tarek Elsaleh, UNIS, Surrey</dc:creator>
        <rdfs:comment xml:lang="en">After a thorough analysis of existing Internet of Things (IoT) related ontologies, we propose FIESTA-IoT Ontology that aims to achieve semantic interoperability among heterogeneous testbeds. The Ontology is framed within the EU H2020 FIESTA-IoT project, that aims to seamlessly support the federation of testbeds through the usage of semantic-based technologies. The  FIESTA-IoT ontology takes inspiration from the well-known Noy et al. methodology for reusing and interconnecting existing ontologies. To build the ontology, we leverage a number of core concepts from various mainstream ontologies and taxonomies, such as Semantic Sensor Network (SSN), M3-lite (a lite version of M3 ontology), WGS84, IoT-lite, Time, and DUL ontology. Please report any errors to rachit.agarwal@inria.fr</rdfs:comment>
        <dcterms:issued rdf:datatype="http://www.w3.org/2001/XMLSchema#date">2016-04-28</dcterms:issued>
        <dc:description xml:lang="en">Many testbeds owning devices or applications interacting with the sensors, store their inherent observations and other related data in their own proprietary format. In other words, making a testbed independent and isolated from others that cannot directly interact with each other. Differences in the data format lead to interoperability issues between the testbeds and much work has to be done in order to ensure the compatibility. One has to understand different data formats and create the mapping between them. As a result, a testbed must understand other testbed&apos;s format and create the mapping both while sending and receiving information. One method to accomplish interoperability is through the usage of semantic-based technologies to annotate all the information shared by the platforms. Nevertheless, some of the relevant existing ontologies promise interoperability but: 

- do not address the problem to describe the observation in an interoperable manner to ease further tasks, such as reasoning, 
- many of them are domain-specific and cannot be applied across domains, 
- they have missing concepts and do not suffice the needs of the measurements provided by the sensors, and 
- many ontologies do not follow best practices making it hard to correctly interpret and reuse concepts.


In order to address the above-mentioned limitations, we provide FIESTA-IoT ontology (a unified semantic model) that follows best practices. FIESTA-IoT Ontology is a merge of concepts from various ontologies such as IoT-lite, M3-lite Taxonomy, SSN, Time and DUL (see Figure 1). The FIESTA-IoT Ontology is divided into 2 parts: resource description and observations produced. One has to follow the Figure 2 and Figure 3, respectively, for understanding what all concepts are associated with resource description and observation. Using such information testbeds can annotate their data to FIESTA-IoT specific requirements and the annotators developed can achieve FIESTA-IoT certification. For reference we provide sample annotations as figure (see Figure 4 and Figure 5) for both resource graph and observation graph.

For more details please see:

- R. Agarwal, D. Fernandez, T. Elsaleh, A. Gyrard, J. Lanza, L. Sanchez, N. Georgantas, V. Issarny, &quot;Unified IoT Ontology to Enable Interoperability and Federation of Testbeds&quot;, 3rd IEEE WF-IoT, Reston, VA, USA, 12-14 December 2016. (https://hal.inria.fr/hal-01386917/document)
- FIESTA-IoT Consortium (R. Agarwal editor), &quot;Deliverable D3.1.2 Semantic Models for Testbeds, Interoperability and Mobility Support, and Best Practices&quot;, project FIESTA-IoT deliverable, 2016.
- FIESTA-IoT Consortium (R. Agarwal editor), &quot;Deliverable D3.1.1 Semantic Models for Testbeds, Interoperability and Mobility Support, and Best Practices&quot;, project FIESTA-IoT deliverable, 2016.

We further acknowledge, testbed provider such as SmartSantander, UniS, KETI, Inria, and other open call testbeds for their valuable comments. Please report any errors to rachit.agarwal@inria.fr. 
        </dc:description>
        <dc:description rdf:resource="http://ontology.fiesta-iot.eu/ontologyDocs/observationannotation.png"/>
        <dcterms:bibliographicCitation xml:lang="en">FIESTA-IoT Consortium (R. Agarwal editor), &quot;Deliverable D3.1.2 Semantic Models for Testbeds, Interoperability and Mobility Support, and Best Practices&quot;, project FIESTA-IoT deliverable, 2016.</dcterms:bibliographicCitation>
        <dc:description rdf:resource="http://ontology.fiesta-iot.eu/ontologyDocs/resourceannotation.png"/>
        <dc:description rdf:resource="http://ontology.fiesta-iot.eu/ontologyDocs/observationgraph.png"/>
        <dc:title xml:lang="en">FIESTA-IoT Ontology</dc:title>
        <dc:creator xml:lang="en">Jorge Lanza, UC, Santander</dc:creator>
        <vann:preferredNamespaceUri>http://purl.org/iot/ontology/fiesta-iot#</vann:preferredNamespaceUri>
    </owl:Ontology>
    


    <!-- 
    ///////////////////////////////////////////////////////////////////////////////////////
    //
    // Annotation properties
    //
    ///////////////////////////////////////////////////////////////////////////////////////
     -->

    


    <!-- http://creativecommons.org/ns#license -->

    <owl:AnnotationProperty rdf:about="http://creativecommons.org/ns#license"/>
    


    <!-- http://purl.oclc.org/NET/UNIS/fiware/iot-lite#altRelative -->

    <owl:AnnotationProperty rdf:about="http://purl.oclc.org/NET/UNIS/fiware/iot-lite#altRelative">
        <rdfs:comment xml:lang="en">Relative Altitude can be used in place of an absolute altitude, especially in buildings, where it makes more sense to locate by levels or floors. For example the value &quot;0&quot; would indicate &quot;ground floor&quot;, and &quot;1&quot; would indicate &quot;1st floor&quot; and so on.</rdfs:comment>
        <rdfs:range rdf:resource="http://www.w3.org/2001/XMLSchema#string"/>
        <rdfs:domain rdf:resource="http://www.w3.org/2003/01/geo/wgs84_pos#Point"/>
    </owl:AnnotationProperty>
    


    <!-- http://purl.oclc.org/NET/UNIS/fiware/iot-lite#relativeLocation -->

    <owl:AnnotationProperty rdf:about="http://purl.oclc.org/NET/UNIS/fiware/iot-lite#relativeLocation">
        <rdfs:comment xml:lang="en">Relative Location is used to provide a place for where the Device is in. For example, Geonames URIs can be used to represent a place, city, area, or region. For &quot;University of Surrey&quot; this would be &quot;http://sws.geonames.org/6695971/&quot;</rdfs:comment>
        <rdfs:range rdf:resource="http://www.w3.org/2001/XMLSchema#string"/>
        <rdfs:domain rdf:resource="http://www.w3.org/2003/01/geo/wgs84_pos#Point"/>
    </owl:AnnotationProperty>
    


    <!-- http://purl.org/dc/elements/1.1/contributor -->

    <owl:AnnotationProperty rdf:about="http://purl.org/dc/elements/1.1/contributor"/>
    


    <!-- http://purl.org/dc/elements/1.1/creator -->

    <owl:AnnotationProperty rdf:about="http://purl.org/dc/elements/1.1/creator"/>
    


    <!-- http://purl.org/dc/elements/1.1/date -->

    <owl:AnnotationProperty rdf:about="http://purl.org/dc/elements/1.1/date"/>
    


    <!-- http://purl.org/dc/elements/1.1/description -->

    <owl:AnnotationProperty rdf:about="http://purl.org/dc/elements/1.1/description"/>
    


    <!-- http://purl.org/dc/elements/1.1/identifier -->

    <owl:AnnotationProperty rdf:about="http://purl.org/dc/elements/1.1/identifier"/>
    


    <!-- http://purl.org/dc/elements/1.1/issued -->

    <owl:AnnotationProperty rdf:about="http://purl.org/dc/elements/1.1/issued"/>
    


    <!-- http://purl.org/dc/elements/1.1/modified -->

    <owl:AnnotationProperty rdf:about="http://purl.org/dc/elements/1.1/modified"/>
    


    <!-- http://purl.org/dc/elements/1.1/rights -->

    <owl:AnnotationProperty rdf:about="http://purl.org/dc/elements/1.1/rights"/>
    


    <!-- http://purl.org/dc/elements/1.1/source -->

    <owl:AnnotationProperty rdf:about="http://purl.org/dc/elements/1.1/source"/>
    


    <!-- http://purl.org/dc/elements/1.1/title -->

    <owl:AnnotationProperty rdf:about="http://purl.org/dc/elements/1.1/title"/>
    


    <!-- http://purl.org/dc/terms/bibliographicCitation -->

    <owl:AnnotationProperty rdf:about="http://purl.org/dc/terms/bibliographicCitation"/>
    


    <!-- http://purl.org/vocab/vann/preferredNamespacePrefix -->

    <owl:AnnotationProperty rdf:about="http://purl.org/vocab/vann/preferredNamespacePrefix"/>
    


    <!-- http://purl.org/vocab/vann/preferredNamespaceUri -->

    <owl:AnnotationProperty rdf:about="http://purl.org/vocab/vann/preferredNamespaceUri"/>
    


    <!-- http://swrl.stanford.edu/ontologies/3.3/swrla.owl#isRuleEnabled -->

    <owl:AnnotationProperty rdf:about="http://swrl.stanford.edu/ontologies/3.3/swrla.owl#isRuleEnabled"/>
    


    <!-- http://www.loa.istc.cnr.it/ontologies/DUL.owl#mappableTo -->

    <owl:AnnotationProperty rdf:about="http://www.loa.istc.cnr.it/ontologies/DUL.owl#mappableTo">
        <rdfs:label xml:lang="en">mappable to</rdfs:label>
    </owl:AnnotationProperty>
    


    <!-- http://www.w3.org/2000/01/rdf-schema#comment -->

    <owl:AnnotationProperty rdf:about="http://www.w3.org/2000/01/rdf-schema#comment"/>
    


    <!-- http://www.w3.org/2000/01/rdf-schema#isDefinedBy -->

    <owl:AnnotationProperty rdf:about="http://www.w3.org/2000/01/rdf-schema#isDefinedBy"/>
    


    <!-- http://www.w3.org/2000/01/rdf-schema#label -->

    <owl:AnnotationProperty rdf:about="http://www.w3.org/2000/01/rdf-schema#label"/>
    


    <!-- http://www.w3.org/2000/01/rdf-schema#seeAlso -->

    <owl:AnnotationProperty rdf:about="http://www.w3.org/2000/01/rdf-schema#seeAlso"/>
    


    <!-- http://www.w3.org/2002/07/owl#equivalentClass -->

    <owl:AnnotationProperty rdf:about="http://www.w3.org/2002/07/owl#equivalentClass"/>
    


    <!-- http://www.w3.org/2002/07/owl#versionInfo -->

    <owl:AnnotationProperty rdf:about="http://www.w3.org/2002/07/owl#versionInfo"/>
    


    <!-- http://www.w3.org/2003/01/geo/wgs84_pos#alt -->

    <owl:AnnotationProperty rdf:about="http://www.w3.org/2003/01/geo/wgs84_pos#alt">
        <rdfs:domain rdf:resource="http://www.w3.org/2003/01/geo/wgs84_pos#Point"/>
    </owl:AnnotationProperty>
    


    <!-- http://www.w3.org/2003/01/geo/wgs84_pos#lat -->

    <owl:AnnotationProperty rdf:about="http://www.w3.org/2003/01/geo/wgs84_pos#lat">
        <rdfs:domain rdf:resource="http://www.w3.org/2003/01/geo/wgs84_pos#Point"/>
    </owl:AnnotationProperty>
    


    <!-- http://www.w3.org/2003/01/geo/wgs84_pos#long -->

    <owl:AnnotationProperty rdf:about="http://www.w3.org/2003/01/geo/wgs84_pos#long">
        <rdfs:domain rdf:resource="http://www.w3.org/2003/01/geo/wgs84_pos#Point"/>
    </owl:AnnotationProperty>
    


    <!-- 
    ///////////////////////////////////////////////////////////////////////////////////////
    //
    // Object Properties
    //
    ///////////////////////////////////////////////////////////////////////////////////////
     -->

    


    <!-- http://purl.oclc.org/NET/UNIS/fiware/iot-lite#exposedBy -->

    <owl:ObjectProperty rdf:about="http://purl.oclc.org/NET/UNIS/fiware/iot-lite#exposedBy">
        <owl:inverseOf rdf:resource="http://purl.oclc.org/NET/UNIS/fiware/iot-lite#exposes"/>
        <rdfs:domain rdf:resource="http://purl.oclc.org/NET/ssnx/ssn#Device"/>
        <rdfs:range rdf:resource="http://purl.oclc.org/NET/UNIS/fiware/iot-lite#Service"/>
        <rdfs:comment xml:lang="en">A device is exposed by a service.</rdfs:comment>
        <rdfs:label xml:lang="en">Exposed By</rdfs:label>
    </owl:ObjectProperty>
    


    <!-- http://purl.oclc.org/NET/UNIS/fiware/iot-lite#exposes -->

    <owl:ObjectProperty rdf:about="http://purl.oclc.org/NET/UNIS/fiware/iot-lite#exposes">
        <rdfs:domain rdf:resource="http://purl.oclc.org/NET/UNIS/fiware/iot-lite#Service"/>
        <rdfs:range rdf:resource="http://purl.oclc.org/NET/ssnx/ssn#Device"/>
        <rdfs:comment xml:lang="en">For service-oriented queries. The inverse of exposedBy.</rdfs:comment>
        <rdfs:label xml:lang="en">Exposes</rdfs:label>
    </owl:ObjectProperty>
    


    <!-- http://purl.oclc.org/NET/UNIS/fiware/iot-lite#hasAttribute -->

    <owl:ObjectProperty rdf:about="http://purl.oclc.org/NET/UNIS/fiware/iot-lite#hasAttribute">
        <rdfs:domain rdf:resource="http://purl.oclc.org/NET/UNIS/fiware/iot-lite#Entity"/>
        <rdfs:domain rdf:resource="http://purl.oclc.org/NET/UNIS/fiware/iot-lite#Object"/>
        <rdfs:range rdf:resource="http://purl.oclc.org/NET/UNIS/fiware/iot-lite#Attribute"/>
        <rdfs:comment xml:lang="en">Links the devices with their attributes.</rdfs:comment>
        <rdfs:label xml:lang="en">Has Attribute</rdfs:label>
    </owl:ObjectProperty>
    


    <!-- http://purl.oclc.org/NET/UNIS/fiware/iot-lite#hasCoverage -->

    <owl:ObjectProperty rdf:about="http://purl.oclc.org/NET/UNIS/fiware/iot-lite#hasCoverage">
        <rdfs:domain rdf:resource="http://purl.oclc.org/NET/ssnx/ssn#Device"/>
        <rdfs:range rdf:resource="http://purl.oclc.org/NET/UNIS/fiware/iot-lite#Coverage"/>
        <rdfs:comment xml:lang="en">Links the devices with their coverages.</rdfs:comment>
        <rdfs:label xml:lang="en">Has Coverage</rdfs:label>
    </owl:ObjectProperty>
    


    <!-- http://purl.oclc.org/NET/UNIS/fiware/iot-lite#hasMetadata -->

    <owl:ObjectProperty rdf:about="http://purl.oclc.org/NET/UNIS/fiware/iot-lite#hasMetadata">
        <rdfs:range rdf:resource="http://purl.oclc.org/NET/UNIS/fiware/iot-lite#Metadata"/>
        <rdfs:comment xml:lang="en">Links any concept with metadata about that concept.</rdfs:comment>
        <rdfs:label xml:lang="en">Has Metadata</rdfs:label>
    </owl:ObjectProperty>
    


    <!-- http://purl.oclc.org/NET/UNIS/fiware/iot-lite#hasQuantityKind -->

    <owl:ObjectProperty rdf:about="http://purl.oclc.org/NET/UNIS/fiware/iot-lite#hasQuantityKind">
        <owl:equivalentProperty rdf:resource="http://www.onem2m.org/ontology/Base_Ontology/base_ontology#hasThingProperty"/>
        <rdfs:domain rdf:resource="http://purl.oclc.org/NET/UNIS/fiware/iot-lite#Attribute"/>
        <rdfs:domain rdf:resource="http://purl.oclc.org/NET/ssnx/ssn#Sensor"/>
        <rdfs:range rdf:resource="http://purl.org/NET/ssnx/qu/qu#QuantityKind"/>
        <rdfs:comment xml:lang="en">Links a sensor or an attribute with the quantity  kind it measures (e.g. A sensor -sensor1- measures temperature: sensor1 hasQuantityKind temperature).</rdfs:comment>
        <rdfs:label xml:lang="en">Has Quantity Kind</rdfs:label>
    </owl:ObjectProperty>
    


    <!-- http://purl.oclc.org/NET/UNIS/fiware/iot-lite#hasUnit -->

    <owl:ObjectProperty rdf:about="http://purl.oclc.org/NET/UNIS/fiware/iot-lite#hasUnit">
        <owl:equivalentProperty rdf:resource="http://www.onem2m.org/ontology/Base_Ontology/base_ontology#hasMetaData"/>
        <rdfs:domain rdf:resource="http://purl.oclc.org/NET/ssnx/ssn#MeasurementProperty"/>
        <rdfs:domain rdf:resource="http://purl.oclc.org/NET/ssnx/ssn#ObservationValue"/>
        <rdfs:domain rdf:resource="http://purl.oclc.org/NET/ssnx/ssn#Sensor"/>
        <rdfs:range rdf:resource="http://purl.org/NET/ssnx/qu/qu#Unit"/>
        <rdfs:comment>Links the sensor with the units of the quantity kind it measures (e.g. A sensor -sensor1- measures temperature in Celsius: senso1 hasUnit Celsius).</rdfs:comment>
        <rdfs:label xml:lang="en">Has Unit</rdfs:label>
    </owl:ObjectProperty>
    


    <!-- http://purl.oclc.org/NET/UNIS/fiware/iot-lite#isAssociatedWith -->

    <owl:ObjectProperty rdf:about="http://purl.oclc.org/NET/UNIS/fiware/iot-lite#isAssociatedWith">
        <rdfs:domain rdf:resource="http://purl.oclc.org/NET/UNIS/fiware/iot-lite#Entity"/>
        <rdfs:domain rdf:resource="http://purl.oclc.org/NET/UNIS/fiware/iot-lite#Object"/>
        <rdfs:range rdf:resource="http://purl.oclc.org/NET/UNIS/fiware/iot-lite#Service"/>
        <rdfs:comment>Defines the associations between objects and sensors (e.g. A table (object) has an attribute (temperature at the table) which is associated with a sensor (the temperature sensor of the room). </rdfs:comment>
        <rdfs:label xml:lang="en">Is Associated With</rdfs:label>
    </owl:ObjectProperty>
    


    <!-- http://purl.oclc.org/NET/UNIS/fiware/iot-lite#isSubSystemOf -->

    <owl:ObjectProperty rdf:about="http://purl.oclc.org/NET/UNIS/fiware/iot-lite#isSubSystemOf">
        <owl:inverseOf rdf:resource="http://purl.oclc.org/NET/ssnx/ssn#hasSubSystem"/>
        <rdfs:domain rdf:resource="http://purl.oclc.org/NET/ssnx/ssn#System"/>
        <rdfs:range rdf:resource="http://purl.oclc.org/NET/ssnx/ssn#System"/>
        <rdfs:comment xml:lang="en">This defines that a devices system is a subsystem of another system. For example, a multi-sensor device is a subsystem of a smart building testbed. This is the inverse of the SSN object property &quot;hasSubSystem&quot;. It allows a graph to start from a subsystem. This is useful for resource-centric graphs.</rdfs:comment>
        <rdfs:label xml:lang="en">Is Sub System Of</rdfs:label>
    </owl:ObjectProperty>
    


    <!-- http://purl.oclc.org/NET/ssnx/ssn#attachedSystem -->

    <owl:ObjectProperty rdf:about="http://purl.oclc.org/NET/ssnx/ssn#attachedSystem">
        <owl:inverseOf rdf:resource="http://purl.oclc.org/NET/ssnx/ssn#onPlatform"/>
        <rdfs:domain rdf:resource="http://purl.oclc.org/NET/ssnx/ssn#Platform"/>
        <rdfs:range rdf:resource="http://purl.oclc.org/NET/ssnx/ssn#System"/>
        <rdfs:comment>Relation between a Platform and any Systems (e.g., Sensors) that are attached to the Platform.</rdfs:comment>
        <rdfs:label xml:lang="en">Attached System</rdfs:label>
    </owl:ObjectProperty>
    


    <!-- http://purl.oclc.org/NET/ssnx/ssn#hasDeployment -->

    <owl:ObjectProperty rdf:about="http://purl.oclc.org/NET/ssnx/ssn#hasDeployment">
        <rdfs:domain rdf:resource="http://purl.oclc.org/NET/ssnx/ssn#System"/>
        <rdfs:range rdf:resource="http://purl.oclc.org/NET/ssnx/ssn#Deployment"/>
        <rdfs:comment>Relation between a System and a Deployment, recording that the System/Sensor was deployed in that Deployment.</rdfs:comment>
        <rdfs:label xml:lang="en">Has Deployment</rdfs:label>
    </owl:ObjectProperty>
    


    <!-- http://purl.oclc.org/NET/ssnx/ssn#hasMeasurementCapability -->

    <owl:ObjectProperty rdf:about="http://purl.oclc.org/NET/ssnx/ssn#hasMeasurementCapability">
        <rdfs:domain rdf:resource="http://purl.oclc.org/NET/ssnx/ssn#Sensor"/>
        <rdfs:range rdf:resource="http://purl.oclc.org/NET/ssnx/ssn#MeasurementCapability"/>
        <rdfs:comment>Relation from a Sensor to a MeasurementCapability describing the measurement properties of the sensor.</rdfs:comment>
        <rdfs:isDefinedBy>http://purl.oclc.org/NET/ssnx/ssn</rdfs:isDefinedBy>
        <rdfs:label>has measurement  capability</rdfs:label>
        <rdfs:seeAlso>http://www.w3.org/2005/Incubator/ssn/wiki/SSN_Sensor#MeasuringCapability</rdfs:seeAlso>
    </owl:ObjectProperty>
    


    <!-- http://purl.oclc.org/NET/ssnx/ssn#hasMeasurementProperty -->

    <owl:ObjectProperty rdf:about="http://purl.oclc.org/NET/ssnx/ssn#hasMeasurementProperty">
        <rdfs:domain rdf:resource="http://purl.oclc.org/NET/ssnx/ssn#MeasurementCapability"/>
        <rdfs:range rdf:resource="http://purl.oclc.org/NET/ssnx/ssn#MeasurementProperty"/>
        <rdfs:comment>Relation from a MeasurementCapability to a MeasurementProperty.  For example, to an accuracy (see notes at MeasurementCapability).</rdfs:comment>
        <rdfs:isDefinedBy>http://purl.oclc.org/NET/ssnx/ssn</rdfs:isDefinedBy>
        <rdfs:label>has measurement property</rdfs:label>
        <rdfs:seeAlso>http://www.w3.org/2005/Incubator/ssn/wiki/SSN_Sensor#MeasuringCapability</rdfs:seeAlso>
    </owl:ObjectProperty>
    


    <!-- http://purl.oclc.org/NET/ssnx/ssn#hasSubSystem -->

    <owl:ObjectProperty rdf:about="http://purl.oclc.org/NET/ssnx/ssn#hasSubSystem">
        <rdfs:domain rdf:resource="http://purl.oclc.org/NET/ssnx/ssn#System"/>
        <rdfs:range rdf:resource="http://purl.oclc.org/NET/ssnx/ssn#System"/>
        <rdfs:comment>Haspart relation between a system and its parts.</rdfs:comment>
        <rdfs:label xml:lang="en">Has Sub System</rdfs:label>
    </owl:ObjectProperty>
    


    <!-- http://purl.oclc.org/NET/ssnx/ssn#hasValue -->

    <owl:ObjectProperty rdf:about="http://purl.oclc.org/NET/ssnx/ssn#hasValue">
        <rdfs:domain rdf:resource="http://purl.oclc.org/NET/ssnx/ssn#SensorOutput"/>
        <rdfs:range rdf:resource="http://purl.oclc.org/NET/ssnx/ssn#ObservationValue"/>
        <rdfs:comment xml:lang="en">Provides a relation between observationValue and actual value.</rdfs:comment>
    </owl:ObjectProperty>
    


    <!-- http://purl.oclc.org/NET/ssnx/ssn#madeObservation -->

    <owl:ObjectProperty rdf:about="http://purl.oclc.org/NET/ssnx/ssn#madeObservation">
        <owl:equivalentProperty rdf:resource="http://www.onem2m.org/ontology/Base_Ontology/base_ontology#hasService"/>
        <owl:inverseOf rdf:resource="http://purl.oclc.org/NET/ssnx/ssn#observedBy"/>
        <rdfs:domain rdf:resource="http://purl.oclc.org/NET/ssnx/ssn#Sensor"/>
        <rdfs:range rdf:resource="http://purl.oclc.org/NET/ssnx/ssn#Observation"/>
        <rdfs:comment>Relation between a Sensor and Observations it has made.</rdfs:comment>
    </owl:ObjectProperty>
    


    <!-- http://purl.oclc.org/NET/ssnx/ssn#observationResult -->

    <owl:ObjectProperty rdf:about="http://purl.oclc.org/NET/ssnx/ssn#observationResult">
        <rdfs:domain rdf:resource="http://purl.oclc.org/NET/ssnx/ssn#Observation"/>
        <rdfs:range rdf:resource="http://purl.oclc.org/NET/ssnx/ssn#SensorOutput"/>
        <dc:source>skos:closeMatch &apos;result&apos; [O&amp;M - ISO/DIS 19156] 
		                    http://portal.opengeospatial.org/files/?artifact_id=41579</dc:source>
        <rdfs:comment>Relation linking an Observation (i.e., a description of the context, the Situation, in which the observation was made) and a Result, which contains a value representing the value associated with the observed Property.</rdfs:comment>
    </owl:ObjectProperty>
    


    <!-- http://purl.oclc.org/NET/ssnx/ssn#observationSamplingTime -->

    <owl:ObjectProperty rdf:about="http://purl.oclc.org/NET/ssnx/ssn#observationSamplingTime">
        <rdfs:domain rdf:resource="http://purl.oclc.org/NET/ssnx/ssn#Observation"/>
        <rdfs:range rdf:resource="http://www.w3.org/2006/time#Instant"/>
        <rdfs:comment>Rebadged as phenomenon time in [O&amp;M]. The phenomenon time shall describe the time that the result applies to the property of the feature-of-interest. This is often the time of interaction by a sampling procedure or observation procedure with a real-world feature.</rdfs:comment>
        <rdfs:comment>The sampling time is the time that the result applies to the feature-of-interest. This is the time usually required for geospatial analysis of the result.</rdfs:comment>
        <rdfs:label xml:lang="en">Observation Sampling Time</rdfs:label>
    </owl:ObjectProperty>
    


    <!-- http://purl.oclc.org/NET/ssnx/ssn#observedBy -->

    <owl:ObjectProperty rdf:about="http://purl.oclc.org/NET/ssnx/ssn#observedBy">
        <rdfs:domain rdf:resource="http://purl.oclc.org/NET/ssnx/ssn#Observation"/>
        <rdfs:range rdf:resource="http://purl.oclc.org/NET/ssnx/ssn#Sensor"/>
        <rdfs:comment xml:lang="en">Relation between a observation and it sensor.</rdfs:comment>
        <rdfs:label xml:lang="en">observed by</rdfs:label>
    </owl:ObjectProperty>
    


    <!-- http://purl.oclc.org/NET/ssnx/ssn#observedProperty -->

    <owl:ObjectProperty rdf:about="http://purl.oclc.org/NET/ssnx/ssn#observedProperty">
        <rdfs:domain rdf:resource="http://purl.oclc.org/NET/ssnx/ssn#Observation"/>
        <rdfs:range rdf:resource="http://purl.org/NET/ssnx/qu/qu#QuantityKind"/>
        <dc:source>skos:exactMatch &apos;observedProperty&apos; [O&amp;M - ISO/DIS 19156] 
		                    http://portal.opengeospatial.org/files/?artifact_id=41579</dc:source>
        <rdfs:comment>Relation linking an Observation to the Property that was observed.  The observedProperty should be a Property (hasProperty) of the FeatureOfInterest (linked by featureOfInterest) of this observation.</rdfs:comment>
        <rdfs:label>Observed Property</rdfs:label>
    </owl:ObjectProperty>
    


    <!-- http://purl.oclc.org/NET/ssnx/ssn#onPlatform -->

    <owl:ObjectProperty rdf:about="http://purl.oclc.org/NET/ssnx/ssn#onPlatform">
        <rdfs:domain rdf:resource="http://purl.oclc.org/NET/ssnx/ssn#System"/>
        <rdfs:range rdf:resource="http://purl.oclc.org/NET/ssnx/ssn#Platform"/>
        <rdfs:comment>Relation between a System (e.g., a Sensor) and a Platform.  The relation locates the sensor relative to other described entities: i.e., the Sensor s1&apos;s location is Platform p1.  More precise locations for sensors in space (relative to other entities, where attached to another entity, or in 3D space) are made using DOLCE&apos;s Regions (SpaceRegion).</rdfs:comment>
        <rdfs:label>On Platform</rdfs:label>
    </owl:ObjectProperty>
    


    <!-- http://purl.org/iot/vocab/m3-lite#hasDirection -->

    <owl:ObjectProperty rdf:about="http://purl.org/iot/vocab/m3-lite#hasDirection">
        <rdfs:domain rdf:resource="http://purl.oclc.org/NET/ssnx/ssn#Observation"/>
        <rdfs:range>
            <owl:Restriction>
                <owl:onProperty rdf:resource="http://purl.org/iot/vocab/m3-lite#hasDirection"/>
                <owl:maxQualifiedCardinality rdf:datatype="http://www.w3.org/2001/XMLSchema#nonNegativeInteger">1</owl:maxQualifiedCardinality>
                <owl:onClass rdf:resource="http://purl.org/iot/vocab/m3-lite#Direction"/>
            </owl:Restriction>
        </rdfs:range>
        <rdfs:comment xml:lang="en">The observations made by the sensors are affected by the direction of the sensing device. This property allows observations of the sensor to be associated to the Direction concept</rdfs:comment>
        <rdfs:label xml:lang="en">Has Direction</rdfs:label>
    </owl:ObjectProperty>
    


    <!-- http://purl.org/iot/vocab/m3-lite#hasDomainOfInterest -->

    <owl:ObjectProperty rdf:about="http://purl.org/iot/vocab/m3-lite#hasDomainOfInterest">
        <rdfs:domain rdf:resource="http://purl.oclc.org/NET/ssnx/ssn#Device"/>
        <rdfs:range rdf:resource="http://purl.org/iot/vocab/m3-lite#DomainOfInterest"/>
        <rdfs:comment xml:lang="en">This property is used to classify devices by DomainOfInterest (e.g., blood pressure sensor is used in healthcare)</rdfs:comment>
        <rdfs:label xml:lang="en">Has Domain Of Interest</rdfs:label>
    </owl:ObjectProperty>
    


    <!-- http://purl.org/iot/vocab/m3-lite#hasMeasurementType -->

    <owl:ObjectProperty rdf:about="http://purl.org/iot/vocab/m3-lite#hasMeasurementType">
        <rdfs:domain rdf:resource="http://purl.oclc.org/NET/ssnx/ssn#Observation"/>
        <rdfs:range>
            <owl:Restriction>
                <owl:onProperty rdf:resource="http://purl.org/iot/vocab/m3-lite#hasMeasurementType"/>
                <owl:maxQualifiedCardinality rdf:datatype="http://www.w3.org/2001/XMLSchema#nonNegativeInteger">1</owl:maxQualifiedCardinality>
                <owl:onClass rdf:resource="http://purl.org/iot/vocab/m3-lite#MeasurementType"/>
            </owl:Restriction>
        </rdfs:range>
        <rdfs:comment xml:lang="en">Each sensing device can have a different sensing mechanism which may result in different kinds of sensor data. This property links observation of the sensor to the associated MeasurementType.</rdfs:comment>
        <rdfs:label xml:lang="en">Has Measurement Type</rdfs:label>
    </owl:ObjectProperty>
    


    <!-- http://purl.org/iot/vocab/m3-lite#hasSoundSource -->

    <owl:ObjectProperty rdf:about="http://purl.org/iot/vocab/m3-lite#hasSoundSource">
        <rdfs:subPropertyOf rdf:resource="http://purl.org/iot/vocab/m3-lite#hasSource"/>
        <rdfs:domain rdf:resource="http://purl.org/iot/vocab/m3-lite#Sound"/>
        <rdfs:range rdf:resource="http://purl.org/iot/vocab/m3-lite#SoundSource"/>
        <rdfs:comment xml:lang="en">This property links sound to its environmental source.</rdfs:comment>
        <rdfs:label xml:lang="en">Has Sound Source</rdfs:label>
    </owl:ObjectProperty>
    


    <!-- http://purl.org/iot/vocab/m3-lite#hasSource -->

    <owl:ObjectProperty rdf:about="http://purl.org/iot/vocab/m3-lite#hasSource">
        <rdfs:domain rdf:resource="http://purl.org/NET/ssnx/qu/qu#QuantityKind"/>
        <rdfs:range rdf:resource="http://purl.org/iot/vocab/m3-lite#Source"/>
        <rdfs:comment xml:lang="en">This property links sensed phenomena to its environmental source.</rdfs:comment>
        <rdfs:label xml:lang="en">Has Source</rdfs:label>
    </owl:ObjectProperty>
    


    <!-- http://www.onem2m.org/ontology/Base_Ontology/base_ontology#hasMetaData -->

    <owl:ObjectProperty rdf:about="http://www.onem2m.org/ontology/Base_Ontology/base_ontology#hasMetaData">
        <rdfs:comment>A Value of a Thing can have MetaData (like units, precision-ranges).</rdfs:comment>
        <rdfs:label xml:lang="en">Has MetaData</rdfs:label>
    </owl:ObjectProperty>
    


    <!-- http://www.onem2m.org/ontology/Base_Ontology/base_ontology#hasService -->

    <owl:ObjectProperty rdf:about="http://www.onem2m.org/ontology/Base_Ontology/base_ontology#hasService">
        <rdfs:comment>The Functionalities of a Device are exposed in the network as Services of the Device</rdfs:comment>
        <rdfs:label xml:lang="en">Has Service</rdfs:label>
    </owl:ObjectProperty>
    


    <!-- http://www.onem2m.org/ontology/Base_Ontology/base_ontology#hasThingProperty -->

    <owl:ObjectProperty rdf:about="http://www.onem2m.org/ontology/Base_Ontology/base_ontology#hasThingProperty">
        <rdfs:comment>A Thing may have properties that can be described by Values</rdfs:comment>
        <rdfs:label xml:lang="en">Has Thing Property</rdfs:label>
    </owl:ObjectProperty>
    


    <!-- http://www.w3.org/2003/01/geo/wgs84_pos#location -->

    <owl:ObjectProperty rdf:about="http://www.w3.org/2003/01/geo/wgs84_pos#location">
        <rdfs:range rdf:resource="http://www.w3.org/2003/01/geo/wgs84_pos#Point"/>
        <rdfs:comment xml:lang="en">Provides relation between object and its physical location.</rdfs:comment>
    </owl:ObjectProperty>
    


    <!-- 
    ///////////////////////////////////////////////////////////////////////////////////////
    //
    // Data properties
    //
    ///////////////////////////////////////////////////////////////////////////////////////
     -->

    


    <!-- http://purl.oclc.org/NET/UNIS/fiware/iot-lite#endpoint -->

    <owl:DatatypeProperty rdf:about="http://purl.oclc.org/NET/UNIS/fiware/iot-lite#endpoint">
        <rdfs:domain rdf:resource="http://purl.oclc.org/NET/UNIS/fiware/iot-lite#Service"/>
        <rdfs:range rdf:resource="http://www.w3.org/2001/XMLSchema#anyURI"/>
        <rdfs:comment>Endpoint of the service. It is usually a URL where the service is available.</rdfs:comment>
        <rdfs:label xml:lang="en">Endpoint</rdfs:label>
    </owl:DatatypeProperty>
    


    <!-- http://purl.oclc.org/NET/UNIS/fiware/iot-lite#id -->

    <owl:DatatypeProperty rdf:about="http://purl.oclc.org/NET/UNIS/fiware/iot-lite#id">
        <rdfs:domain rdf:resource="http://purl.oclc.org/NET/UNIS/fiware/iot-lite#Entity"/>
        <rdfs:domain rdf:resource="http://purl.oclc.org/NET/ssnx/ssn#Device"/>
        <rdfs:range rdf:resource="http://www.w3.org/2001/XMLSchema#string"/>
        <rdfs:comment xml:lang="en">The ID of the Device or Entity.</rdfs:comment>
        <rdfs:label xml:lang="en">ID</rdfs:label>
    </owl:DatatypeProperty>
    


    <!-- http://purl.oclc.org/NET/UNIS/fiware/iot-lite#interfaceDescription -->

    <owl:DatatypeProperty rdf:about="http://purl.oclc.org/NET/UNIS/fiware/iot-lite#interfaceDescription">
        <rdfs:domain rdf:resource="http://purl.oclc.org/NET/UNIS/fiware/iot-lite#Service"/>
        <rdfs:range rdf:resource="http://www.w3.org/2001/XMLSchema#anyURI"/>
        <rdfs:comment>Interface Description of the service, e.g. WADL, WSDL, NGSI9 etc.</rdfs:comment>
        <rdfs:label xml:lang="en">Interface Description</rdfs:label>
    </owl:DatatypeProperty>
    


    <!-- http://purl.oclc.org/NET/UNIS/fiware/iot-lite#interfaceType -->

    <owl:DatatypeProperty rdf:about="http://purl.oclc.org/NET/UNIS/fiware/iot-lite#interfaceType">
        <rdfs:domain rdf:resource="http://purl.oclc.org/NET/UNIS/fiware/iot-lite#Service"/>
        <rdfs:range rdf:resource="http://www.w3.org/2001/XMLSchema#string"/>
        <rdfs:comment xml:lang="en">Defines the type of interface of the service endpoint, e.g. RESTful, NGSI-9, MQTT, CoAP etc.</rdfs:comment>
        <rdfs:label xml:lang="en">Interface Type</rdfs:label>
    </owl:DatatypeProperty>
    


    <!-- http://purl.oclc.org/NET/UNIS/fiware/iot-lite#isMobile -->

    <owl:DatatypeProperty rdf:about="http://purl.oclc.org/NET/UNIS/fiware/iot-lite#isMobile">
        <rdfs:domain rdf:resource="http://purl.oclc.org/NET/ssnx/ssn#Platform"/>
        <rdfs:range rdf:resource="http://www.w3.org/2001/XMLSchema#boolean"/>
        <rdfs:comment xml:lang="en">Is the Device mobile? This can be used by an IoT management platform to enable tracking of the device&apos;s location.</rdfs:comment>
        <rdfs:label xml:lang="en">Is Mobile</rdfs:label>
    </owl:DatatypeProperty>
    


    <!-- http://purl.oclc.org/NET/UNIS/fiware/iot-lite#isOnline -->

    <owl:DatatypeProperty rdf:about="http://purl.oclc.org/NET/UNIS/fiware/iot-lite#isOnline">
        <rdfs:domain rdf:resource="http://purl.oclc.org/NET/UNIS/fiware/iot-lite#Service"/>
        <rdfs:range rdf:resource="http://www.w3.org/2001/XMLSchema#boolean"/>
        <rdfs:comment xml:lang="en">Identifies if the service is online or not.</rdfs:comment>
    </owl:DatatypeProperty>
    


    <!-- http://purl.oclc.org/NET/UNIS/fiware/iot-lite#metadataType -->

    <owl:DatatypeProperty rdf:about="http://purl.oclc.org/NET/UNIS/fiware/iot-lite#metadataType">
        <rdfs:domain rdf:resource="http://purl.oclc.org/NET/UNIS/fiware/iot-lite#Metadata"/>
        <rdfs:range rdf:resource="http://www.w3.org/2001/XMLSchema#string"/>
        <rdfs:comment>Defines the type pf the metadata value (e.g. resolution of the sensor).</rdfs:comment>
        <rdfs:label xml:lang="en">Metadata Type</rdfs:label>
    </owl:DatatypeProperty>
    


    <!-- http://purl.oclc.org/NET/UNIS/fiware/iot-lite#metadataValue -->

    <owl:DatatypeProperty rdf:about="http://purl.oclc.org/NET/UNIS/fiware/iot-lite#metadataValue">
        <rdfs:domain rdf:resource="http://purl.oclc.org/NET/UNIS/fiware/iot-lite#Metadata"/>
        <rdfs:range rdf:resource="http://www.w3.org/2001/XMLSchema#string"/>
        <rdfs:comment>Value of the metadata</rdfs:comment>
        <rdfs:label xml:lang="en">Metadata Value</rdfs:label>
    </owl:DatatypeProperty>
    


    <!-- http://purl.oclc.org/NET/UNIS/fiware/iot-lite#radius -->

    <owl:DatatypeProperty rdf:about="http://purl.oclc.org/NET/UNIS/fiware/iot-lite#radius">
        <rdfs:domain rdf:resource="http://purl.oclc.org/NET/UNIS/fiware/iot-lite#Circle"/>
        <rdfs:range rdf:resource="http://www.w3.org/2001/XMLSchema#double"/>
        <rdfs:comment>Specifies the radius of a circle coverage defined by a point -the centre of the circle- and its radius.</rdfs:comment>
        <rdfs:label xml:lang="en">Radius</rdfs:label>
    </owl:DatatypeProperty>
    


    <!-- http://purl.org/iot/ontology/fiesta-iot#hasWaterFlow -->

    <owl:DatatypeProperty rdf:about="http://purl.org/iot/ontology/fiesta-iot#hasWaterFlow">
        <rdfs:subPropertyOf rdf:resource="http://www.w3.org/2002/07/owl#topDataProperty"/>
        <rdfs:range rdf:resource="http://www.w3.org/2001/XMLSchema#boolean"/>
    </owl:DatatypeProperty>
    


    <!-- http://www.loa.istc.cnr.it/ontologies/DUL.owl#hasDataValue -->

    <owl:DatatypeProperty rdf:about="http://www.loa.istc.cnr.it/ontologies/DUL.owl#hasDataValue">
        <rdfs:domain rdf:resource="http://purl.oclc.org/NET/ssnx/ssn#MeasurementProperty"/>
        <rdfs:domain rdf:resource="http://purl.oclc.org/NET/ssnx/ssn#ObservationValue"/>
        <rdfs:range rdf:resource="http://www.w3.org/2001/XMLSchema#boolean"/>
        <rdfs:range rdf:resource="http://www.w3.org/2001/XMLSchema#dateTime"/>
        <rdfs:range rdf:resource="http://www.w3.org/2001/XMLSchema#double"/>
        <rdfs:range rdf:resource="http://www.w3.org/2001/XMLSchema#int"/>
        <rdfs:range rdf:resource="http://www.w3.org/2001/XMLSchema#string"/>
        <rdfs:comment>A datatype property that encodes values from a datatype for an Entity. 
There are several ways to encode values in DOLCE (Ultralite):

1) Directly assert an xsd:_ value to an Entity by using hasDataValue
2) Assert a Region for an Entity by using hasRegion, and then assert an xsd:_ value to that Region, by using hasRegionDataValue
3) Assert a Quality for an Entity by using hasQuality, then assert a Region for that Quality, and assert an xsd:_ value to that Region, by using hasRegionDataValue
4) When the value is required, but not directly observed, assert a Parameter for an xsd:_ value by using hasParameterDataValue, and then associate the Parameter to an Entity by using isConstraintFor
5) When the value is required, but not directly observed, you can also assert a Parameter for a Region by using parametrizes, and then assert an xsd:_ value to that Region, by using hasRegionDataValue

The five approaches obey different requirements. 
For example, a simple value can be easily asserted by using pattern (1), but if one needs to assert an interval between two values, a Region should be introduced to materialize that interval, as pattern (2) suggests. 
Furthermore, if one needs to distinguish the individual Quality of a value, e.g. the particular nature of the density of a substance, pattern (3) can be used. 
Patterns (4) and (5) should be used instead when a constraint or a selection is modelled, independently from the actual observation of values in the real world.</rdfs:comment>
    </owl:DatatypeProperty>
    


    <!-- http://www.w3.org/2006/time#inXSDDateTime -->

    <owl:DatatypeProperty rdf:about="http://www.w3.org/2006/time#inXSDDateTime">
        <rdfs:domain rdf:resource="http://www.w3.org/2006/time#Instant"/>
        <rdfs:range rdf:resource="http://www.w3.org/2001/XMLSchema#dateTime"/>
        <rdfs:comment xml:lang="en">It is the property relating Time Instant with the datetime value</rdfs:comment>
        <rdfs:label xml:lang="en">In XSD DateTime</rdfs:label>
    </owl:DatatypeProperty>
    


    <!-- 
    ///////////////////////////////////////////////////////////////////////////////////////
    //
    // Classes
    //
    ///////////////////////////////////////////////////////////////////////////////////////
     -->

    


    <!-- http://purl.oclc.org/NET/UNIS/fiware/iot-lite#ActuatingDevice -->

    <owl:Class rdf:about="http://purl.oclc.org/NET/UNIS/fiware/iot-lite#ActuatingDevice">
        <rdfs:subClassOf rdf:resource="http://purl.oclc.org/NET/ssnx/ssn#Device"/>
        <rdfs:comment xml:lang="en">Device that can actuate over an object or QuantityKind (e.g., switch on/off the light).</rdfs:comment>
        <rdfs:label xml:lang="en">Actuating Device</rdfs:label>
    </owl:Class>
    


    <!-- http://purl.oclc.org/NET/UNIS/fiware/iot-lite#Attribute -->

    <owl:Class rdf:about="http://purl.oclc.org/NET/UNIS/fiware/iot-lite#Attribute">
        <rdfs:subClassOf>
            <owl:Restriction>
                <owl:onProperty rdf:resource="http://purl.oclc.org/NET/UNIS/fiware/iot-lite#hasQuantityKind"/>
                <owl:qualifiedCardinality rdf:datatype="http://www.w3.org/2001/XMLSchema#nonNegativeInteger">1</owl:qualifiedCardinality>
                <owl:onClass rdf:resource="http://purl.org/NET/ssnx/qu/qu#QuantityKind"/>
            </owl:Restriction>
        </rdfs:subClassOf>
        <rdfs:comment xml:lang="en">An attribute of an IoT object that can be exposed by an IoT service (i.e. a room (IoT Object) has a temperature (Attribute), that can be exposed by a temperature sensor (IoT device).</rdfs:comment>
        <rdfs:label xml:lang="en">Attribute</rdfs:label>
    </owl:Class>
    


    <!-- http://purl.oclc.org/NET/UNIS/fiware/iot-lite#Circle -->

    <owl:Class rdf:about="http://purl.oclc.org/NET/UNIS/fiware/iot-lite#Circle">
        <rdfs:subClassOf rdf:resource="http://purl.oclc.org/NET/UNIS/fiware/iot-lite#Coverage"/>
        <rdfs:comment xml:lang="en">Circle coverage it needs the location of the sensor as the centre of the circle and the radius as a DataProperty.</rdfs:comment>
        <rdfs:label xml:lang="en">Circle</rdfs:label>
    </owl:Class>
    


    <!-- http://purl.oclc.org/NET/UNIS/fiware/iot-lite#Coverage -->

    <owl:Class rdf:about="http://purl.oclc.org/NET/UNIS/fiware/iot-lite#Coverage">
        <rdfs:subClassOf>
            <owl:Restriction>
                <owl:onProperty rdf:resource="http://www.w3.org/2003/01/geo/wgs84_pos#location"/>
                <owl:qualifiedCardinality rdf:datatype="http://www.w3.org/2001/XMLSchema#nonNegativeInteger">1</owl:qualifiedCardinality>
                <owl:onClass rdf:resource="http://www.w3.org/2003/01/geo/wgs84_pos#Point"/>
            </owl:Restriction>
        </rdfs:subClassOf>
        <rdfs:comment xml:lang="en">The coverage of an IoT device (i.e. a temperature sensor inside a room has a coverage of that room).</rdfs:comment>
        <rdfs:label xml:lang="en">Coverage</rdfs:label>
    </owl:Class>
    


    <!-- http://purl.oclc.org/NET/UNIS/fiware/iot-lite#Entity -->

    <owl:Class rdf:about="http://purl.oclc.org/NET/UNIS/fiware/iot-lite#Entity">
        <owl:equivalentClass rdf:resource="http://purl.oclc.org/NET/UNIS/fiware/iot-lite#Object"/>
        <rdfs:subClassOf>
            <owl:Restriction>
                <owl:onProperty rdf:resource="http://purl.oclc.org/NET/UNIS/fiware/iot-lite#hasAttribute"/>
                <owl:minQualifiedCardinality rdf:datatype="http://www.w3.org/2001/XMLSchema#nonNegativeInteger">1</owl:minQualifiedCardinality>
                <owl:onClass rdf:resource="http://purl.oclc.org/NET/UNIS/fiware/iot-lite#Attribute"/>
            </owl:Restriction>
        </rdfs:subClassOf>
        <rdfs:subClassOf>
            <owl:Restriction>
                <owl:onProperty rdf:resource="http://purl.oclc.org/NET/UNIS/fiware/iot-lite#isAssociatedWith"/>
                <owl:minQualifiedCardinality rdf:datatype="http://www.w3.org/2001/XMLSchema#nonNegativeInteger">1</owl:minQualifiedCardinality>
                <owl:onClass rdf:resource="http://purl.oclc.org/NET/UNIS/fiware/iot-lite#Service"/>
            </owl:Restriction>
        </rdfs:subClassOf>
        <rdfs:subClassOf>
            <owl:Restriction>
                <owl:onProperty rdf:resource="http://www.w3.org/2003/01/geo/wgs84_pos#location"/>
                <owl:qualifiedCardinality rdf:datatype="http://www.w3.org/2001/XMLSchema#nonNegativeInteger">1</owl:qualifiedCardinality>
                <owl:onClass rdf:resource="http://www.w3.org/2003/01/geo/wgs84_pos#Point"/>
            </owl:Restriction>
        </rdfs:subClassOf>
        <rdfs:comment xml:lang="en">Any object that is relevant from a user or application perspective. (IoT-A Definition)</rdfs:comment>
        <rdfs:label xml:lang="en">Entity</rdfs:label>
    </owl:Class>
    


    <!-- http://purl.oclc.org/NET/UNIS/fiware/iot-lite#Metadata -->

    <owl:Class rdf:about="http://purl.oclc.org/NET/UNIS/fiware/iot-lite#Metadata">
        <rdfs:comment xml:lang="en">Class used to describe properties that cannot be described by QuantityKind and Units. i.e. the resolution of a sensor.</rdfs:comment>
        <rdfs:label xml:lang="en">Metadata</rdfs:label>
    </owl:Class>
    


    <!-- http://purl.oclc.org/NET/UNIS/fiware/iot-lite#Object -->

    <owl:Class rdf:about="http://purl.oclc.org/NET/UNIS/fiware/iot-lite#Object">
        <rdfs:comment xml:lang="en">IoT entity</rdfs:comment>
        <rdfs:label xml:lang="en">IoT Entity or Object</rdfs:label>
    </owl:Class>
    


    <!-- http://purl.oclc.org/NET/UNIS/fiware/iot-lite#Polygon -->

    <owl:Class rdf:about="http://purl.oclc.org/NET/UNIS/fiware/iot-lite#Polygon">
        <rdfs:subClassOf rdf:resource="http://purl.oclc.org/NET/UNIS/fiware/iot-lite#Coverage"/>
        <rdfs:comment xml:lang="en">The coverage is made up by linking several points by strait lines.</rdfs:comment>
        <rdfs:label xml:lang="en">Polygon</rdfs:label>
    </owl:Class>
    


    <!-- http://purl.oclc.org/NET/UNIS/fiware/iot-lite#Rectangle -->

    <owl:Class rdf:about="http://purl.oclc.org/NET/UNIS/fiware/iot-lite#Rectangle">
        <rdfs:subClassOf rdf:resource="http://purl.oclc.org/NET/UNIS/fiware/iot-lite#Coverage"/>
        <rdfs:comment xml:lang="en">The coverage is made up by giving two points which are the opposite corners of a rectangle.</rdfs:comment>
        <rdfs:label xml:lang="en">Rectangle</rdfs:label>
    </owl:Class>
    


    <!-- http://purl.oclc.org/NET/UNIS/fiware/iot-lite#Service -->

    <owl:Class rdf:about="http://purl.oclc.org/NET/UNIS/fiware/iot-lite#Service">
        <rdfs:subClassOf>
            <owl:Restriction>
                <owl:onProperty rdf:resource="http://purl.oclc.org/NET/UNIS/fiware/iot-lite#exposes"/>
                <owl:minQualifiedCardinality rdf:datatype="http://www.w3.org/2001/XMLSchema#nonNegativeInteger">1</owl:minQualifiedCardinality>
                <owl:onClass rdf:resource="http://purl.oclc.org/NET/ssnx/ssn#Device"/>
            </owl:Restriction>
        </rdfs:subClassOf>
        <rdfs:comment xml:lang="en">Service provided by an IoT Device</rdfs:comment>
        <rdfs:label xml:lang="en">Service</rdfs:label>
    </owl:Class>
    


    <!-- http://purl.oclc.org/NET/UNIS/fiware/iot-lite#TagDevice -->

    <owl:Class rdf:about="http://purl.oclc.org/NET/UNIS/fiware/iot-lite#TagDevice">
        <rdfs:subClassOf rdf:resource="http://purl.oclc.org/NET/ssnx/ssn#Device"/>
        <rdfs:comment xml:lang="en">Device that can redirect to a resource with information (i.e. RFID, NFC, QR-codes, bar-codes).</rdfs:comment>
        <rdfs:label xml:lang="en">Tagging Device</rdfs:label>
    </owl:Class>
    


    <!-- http://purl.oclc.org/NET/UNIS/fiware/iot-lite#VirtualEntity -->

    <owl:Class rdf:about="http://purl.oclc.org/NET/UNIS/fiware/iot-lite#VirtualEntity">
        <rdfs:subClassOf rdf:resource="http://purl.oclc.org/NET/UNIS/fiware/iot-lite#Entity"/>
        <rdfs:comment xml:lang="en">Computational or data element representing a Physical Entity. Virtual Entities can be either Active or Passive Digital Entities.

Physical Entities are represented in the digital world by a Virtual Entity. This
term is also referred to as virtual counterpart in the literature (Romer et al. 2002),
but using the same root term entity in both concepts clearer shows the relationship
of these concepts. There are many kinds of digital representations of Physical
Entities: 3D models, avatars, database entries, objects (or instances of a class in an
object-oriented programming language), and even a social-network account could
be viewed as such a representation, because it digitally represents certain aspects of
its human owner, such as a photograph or a list of his hobbies.

Also see, Enabling Things to Talk: Designing IoT solutions with the IoT Architectural Reference Model, Alessandro Bassi, Martin Bauer, Martin Fiedler, Thorsten Kramp,
Rob van Kranenburg, Sebastian Lange, Stefan Meissner</rdfs:comment>
        <rdfs:label xml:lang="en">Virtual Entity</rdfs:label>
    </owl:Class>
    


    <!-- http://purl.oclc.org/NET/ssnx/ssn#Accuracy -->

    <owl:Class rdf:about="http://purl.oclc.org/NET/ssnx/ssn#Accuracy">
        <rdfs:subClassOf rdf:resource="http://purl.oclc.org/NET/ssnx/ssn#MeasurementProperty"/>
        <dc:source>skos:exactMatch &apos;measurement accuracy/accuracy&apos; [VIM 2.13] 
                            http://www.bipm.org/utils/common/documents/jcgm/JCGM_200_2008.pdf</dc:source>
        <rdfs:comment>The closeness of agreement between the value of an observation and the true value of the observed quality.</rdfs:comment>
        <rdfs:isDefinedBy>http://purl.oclc.org/NET/ssnx/ssn</rdfs:isDefinedBy>
        <rdfs:label>Accuracy</rdfs:label>
        <rdfs:seeAlso>http://www.w3.org/2005/Incubator/ssn/wiki/SSN_Sensor#MeasuringCapability</rdfs:seeAlso>
    </owl:Class>
    


    <!-- http://purl.oclc.org/NET/ssnx/ssn#Deployment -->

    <owl:Class rdf:about="http://purl.oclc.org/NET/ssnx/ssn#Deployment">
        <dc:source>skos:closeMatch &apos;Deployment&apos; [MMI Dev]
                                 http://marinemetadata.org/community/teams/ontdevices</dc:source>
        <rdfs:comment>The ongoing Process of Entities (for the purposes of this ontology, mainly sensors) deployed for a particular purpose.  For example, a particular Sensor deployed on a Platform, or a whole network of Sensors deployed for an observation campaign.  The deployment may have sub processes, such as installation, maintenance, addition, and decommissioning and removal.</rdfs:comment>
        <rdfs:label xml:lang="en">Deployment</rdfs:label>
        <rdfs:seeAlso>http://www.w3.org/2005/Incubator/ssn/wiki/SSN_Deploy#Deployment</rdfs:seeAlso>
    </owl:Class>
    


    <!-- http://purl.oclc.org/NET/ssnx/ssn#Device -->

    <owl:Class rdf:about="http://purl.oclc.org/NET/ssnx/ssn#Device">
        <rdfs:subClassOf rdf:resource="http://purl.oclc.org/NET/ssnx/ssn#System"/>
        <rdfs:subClassOf>
            <owl:Restriction>
                <owl:onProperty rdf:resource="http://purl.oclc.org/NET/UNIS/fiware/iot-lite#exposedBy"/>
                <owl:someValuesFrom rdf:resource="http://purl.oclc.org/NET/UNIS/fiware/iot-lite#Service"/>
            </owl:Restriction>
        </rdfs:subClassOf>
        <rdfs:subClassOf>
            <owl:Restriction>
                <owl:onProperty rdf:resource="http://purl.org/iot/vocab/m3-lite#hasDomainOfInterest"/>
                <owl:minQualifiedCardinality rdf:datatype="http://www.w3.org/2001/XMLSchema#nonNegativeInteger">1</owl:minQualifiedCardinality>
                <owl:onClass rdf:resource="http://purl.org/iot/vocab/m3-lite#DomainOfInterest"/>
            </owl:Restriction>
        </rdfs:subClassOf>
        <rdfs:subClassOf>
            <owl:Restriction>
                <owl:onProperty rdf:resource="http://purl.oclc.org/NET/UNIS/fiware/iot-lite#hasCoverage"/>
                <owl:maxQualifiedCardinality rdf:datatype="http://www.w3.org/2001/XMLSchema#nonNegativeInteger">1</owl:maxQualifiedCardinality>
                <owl:onClass rdf:resource="http://purl.oclc.org/NET/UNIS/fiware/iot-lite#Coverage"/>
            </owl:Restriction>
        </rdfs:subClassOf>
        <dc:source>http://www.w3.org/2005/Incubator/ssn/</dc:source>
        <rdfs:comment>A device is a physical piece of technology - a system in a box. Devices may of course be built of smaller devices and software components (i.e. systems have components).</rdfs:comment>
        <rdfs:label xml:lang="en">Device</rdfs:label>
        <rdfs:seeAlso>http://www.w3.org/2005/Incubator/ssn/wiki/SSN_Device#Device</rdfs:seeAlso>
    </owl:Class>
    


    <!-- http://purl.oclc.org/NET/ssnx/ssn#Frequency -->

    <owl:Class rdf:about="http://purl.oclc.org/NET/ssnx/ssn#Frequency">
        <rdfs:subClassOf rdf:resource="http://purl.oclc.org/NET/ssnx/ssn#MeasurementProperty"/>
        <rdfs:comment>The smallest possible time between one observation and the next.</rdfs:comment>
        <rdfs:isDefinedBy>http://purl.oclc.org/NET/ssnx/ssn</rdfs:isDefinedBy>
        <rdfs:label>Frequency</rdfs:label>
        <rdfs:seeAlso>http://www.w3.org/2005/Incubator/ssn/wiki/SSN_Sensor#MeasuringCapability</rdfs:seeAlso>
    </owl:Class>
    


    <!-- http://purl.oclc.org/NET/ssnx/ssn#Latency -->

    <owl:Class rdf:about="http://purl.oclc.org/NET/ssnx/ssn#Latency">
        <rdfs:subClassOf rdf:resource="http://purl.oclc.org/NET/ssnx/ssn#MeasurementProperty"/>
        <rdfs:comment>The time between a request for an observation and the sensor providing a result.</rdfs:comment>
        <rdfs:isDefinedBy>http://purl.oclc.org/NET/ssnx/ssn</rdfs:isDefinedBy>
        <rdfs:label>Latency</rdfs:label>
        <rdfs:seeAlso>http://www.w3.org/2005/Incubator/ssn/wiki/SSN_Sensor#MeasuringCapability</rdfs:seeAlso>
    </owl:Class>
    


    <!-- http://purl.oclc.org/NET/ssnx/ssn#MeasurementCapability -->

    <owl:Class rdf:about="http://purl.oclc.org/NET/ssnx/ssn#MeasurementCapability">
        <rdfs:subClassOf>
            <owl:Restriction>
                <owl:onProperty rdf:resource="http://purl.oclc.org/NET/ssnx/ssn#hasMeasurementProperty"/>
                <owl:allValuesFrom rdf:resource="http://purl.oclc.org/NET/ssnx/ssn#MeasurementProperty"/>
            </owl:Restriction>
        </rdfs:subClassOf>
        <dc:source>Similar idea to MeasurementCapability in MMI Device Ontology
                                  http://marinemetadata.org/community/teams/ontdevices

But the the two express the relationship between constraints and multiple measurement properties differently.

The conditions linked to a MeasurementCapability are skos:exactMatch to &apos;influence quantity&apos; [VIM 2.52]
http://www.bipm.org/utils/common/documents/jcgm/JCGM_200_2008.pdf</dc:source>
        <rdfs:comment>Collects together measurement properties (accuracy, range, precision, etc) and the environmental conditions in which those properties hold, representing a specification of a sensor&apos;s capability in those conditions.

The conditions specified here are those that affect the measurement properties, while those in OperatingRange represent the sensor&apos;s standard operating conditions, including conditions that don&apos;t affect the observations.</rdfs:comment>
        <rdfs:isDefinedBy>http://purl.oclc.org/NET/ssnx/ssn</rdfs:isDefinedBy>
        <rdfs:label>Measurement Capability</rdfs:label>
        <rdfs:seeAlso>http://www.w3.org/2005/Incubator/ssn/wiki/SSN_Sensor#MeasuringCapability</rdfs:seeAlso>
    </owl:Class>
    


    <!-- http://purl.oclc.org/NET/ssnx/ssn#MeasurementProperty -->

    <owl:Class rdf:about="http://purl.oclc.org/NET/ssnx/ssn#MeasurementProperty">
        <rdfs:comment>An identifiable and observable characteristic of a sensor&apos;s observations or ability to make observations.</rdfs:comment>
        <rdfs:isDefinedBy>http://purl.oclc.org/NET/ssnx/ssn</rdfs:isDefinedBy>
        <rdfs:label>Measurement  Property</rdfs:label>
        <rdfs:seeAlso>http://www.w3.org/2005/Incubator/ssn/wiki/SSN_Sensor#MeasuringCapability</rdfs:seeAlso>
    </owl:Class>
    


    <!-- http://purl.oclc.org/NET/ssnx/ssn#Observation -->

    <owl:Class rdf:about="http://purl.oclc.org/NET/ssnx/ssn#Observation">
        <owl:equivalentClass rdf:resource="http://www.onem2m.org/ontology/Base_Ontology/base_ontology#Service"/>
        <rdfs:subClassOf>
            <owl:Restriction>
                <owl:onProperty rdf:resource="http://purl.org/iot/vocab/m3-lite#hasMeasurementType"/>
                <owl:someValuesFrom rdf:resource="http://purl.org/iot/vocab/m3-lite#MeasurementType"/>
            </owl:Restriction>
        </rdfs:subClassOf>
        <rdfs:subClassOf>
            <owl:Restriction>
                <owl:onProperty rdf:resource="http://purl.oclc.org/NET/ssnx/ssn#observationSamplingTime"/>
                <owl:minCardinality rdf:datatype="http://www.w3.org/2001/XMLSchema#nonNegativeInteger">0</owl:minCardinality>
            </owl:Restriction>
        </rdfs:subClassOf>
        <rdfs:subClassOf>
            <owl:Restriction>
                <owl:onProperty rdf:resource="http://purl.oclc.org/NET/ssnx/ssn#observedBy"/>
                <owl:qualifiedCardinality rdf:datatype="http://www.w3.org/2001/XMLSchema#nonNegativeInteger">1</owl:qualifiedCardinality>
                <owl:onClass rdf:resource="http://purl.oclc.org/NET/ssnx/ssn#Sensor"/>
            </owl:Restriction>
        </rdfs:subClassOf>
        <rdfs:subClassOf>
            <owl:Restriction>
                <owl:onProperty rdf:resource="http://purl.oclc.org/NET/ssnx/ssn#observedProperty"/>
                <owl:qualifiedCardinality rdf:datatype="http://www.w3.org/2001/XMLSchema#nonNegativeInteger">1</owl:qualifiedCardinality>
                <owl:onClass rdf:resource="http://purl.org/NET/ssnx/qu/qu#QuantityKind"/>
            </owl:Restriction>
        </rdfs:subClassOf>
        <rdfs:subClassOf>
            <owl:Restriction>
                <owl:onProperty rdf:resource="http://www.w3.org/2003/01/geo/wgs84_pos#location"/>
                <owl:qualifiedCardinality rdf:datatype="http://www.w3.org/2001/XMLSchema#nonNegativeInteger">1</owl:qualifiedCardinality>
                <owl:onClass rdf:resource="http://www.w3.org/2003/01/geo/wgs84_pos#Point"/>
            </owl:Restriction>
        </rdfs:subClassOf>
        <dc:source>skos:closeMatch &apos;observation&apos; [O&amp;M] 
		                    http://www.opengeospatial.org/standards/om 

Observation in this ontology and O&amp;M are described differently (O&amp;M records an observation as an act/event), but they record the same thing and are essentially interchangeable.  The difference is in the ontological structure of the two, not the data or use.

Observation here records a Situation (the estimation of the value of a Property) and a description of the method that was used (along with the participants), while O&amp;M interprets an Observation as the event itself; there must, however, have been an event that lead to our situation, so both are records of events.  The distinction is between the event itself and the record of what happened in that event.


skos:closeMatch &apos;measurement result&apos; [VIM 2.9] http://www.bipm.org/utils/common/documents/jcgm/JCGM_200_2008.pdf

Measurement result in VIM is the measured value plus any other relevant information, which means that measurement result and observation will often be associated to the same data (a value, a time, a property, etc.).</dc:source>
        <rdfs:comment>An Observation is a Situation in which a Sensing method has been used to estimate or calculate a value of a Property of a FeatureOfInterest.  Links to Sensing and Sensor describe what made the Observation and how; links to Property and Feature detail what was sensed; the result is the output of a Sensor; other metadata details times etc.</rdfs:comment>
        <rdfs:label xml:lang="en">Observation</rdfs:label>
        <rdfs:seeAlso>http://www.w3.org/2005/Incubator/ssn/wiki/SSN_Skeleton#Skeleton</rdfs:seeAlso>
    </owl:Class>
    


    <!-- http://purl.oclc.org/NET/ssnx/ssn#ObservationValue -->

    <owl:Class rdf:about="http://purl.oclc.org/NET/ssnx/ssn#ObservationValue">
        <owl:equivalentClass rdf:resource="http://www.onem2m.org/ontology/Base_Ontology/base_ontology#OperationOutput"/>
        <rdfs:subClassOf>
            <owl:Restriction>
                <owl:onProperty rdf:resource="http://purl.oclc.org/NET/UNIS/fiware/iot-lite#hasUnit"/>
                <owl:qualifiedCardinality rdf:datatype="http://www.w3.org/2001/XMLSchema#nonNegativeInteger">1</owl:qualifiedCardinality>
                <owl:onClass rdf:resource="http://purl.org/NET/ssnx/qu/qu#Unit"/>
            </owl:Restriction>
        </rdfs:subClassOf>
        <dc:source>skos:exactMatch &apos;measured quantity value&apos; [VIM 2.10]
                                  http://www.bipm.org/utils/common/documents/jcgm/JCGM_200_2008.pdf

skos:exactMatch &apos;observed value&apos; [SensorML OGC-0700]
http://www.opengeospatial.org/standards/sensorml 

skos:closeMatch &apos;observation result&apos; [O&amp;M]
http://www.opengeospatial.org/standards/om 

O&amp;M conflates what we have as SensorOutput and ObservationValue into observation result, though the OGC standard does say &quot;result contains a value&quot; and &quot;a result which has a value&quot;, which fits naturally with the model here.</dc:source>
        <rdfs:comment>The value of the result of an Observation.  An Observation has a result which is the output of some sensor, the result is an information object that encodes some value for a Feature.</rdfs:comment>
        <rdfs:label>Observation Value</rdfs:label>
        <rdfs:seeAlso>http://www.w3.org/2005/Incubator/ssn/wiki/SSN_Base#Data</rdfs:seeAlso>
    </owl:Class>
    


    <!-- http://purl.oclc.org/NET/ssnx/ssn#Platform -->

    <owl:Class rdf:about="http://purl.oclc.org/NET/ssnx/ssn#Platform">
        <rdfs:subClassOf>
            <owl:Restriction>
                <owl:onProperty rdf:resource="http://purl.oclc.org/NET/ssnx/ssn#attachedSystem"/>
                <owl:allValuesFrom rdf:resource="http://purl.oclc.org/NET/ssnx/ssn#System"/>
            </owl:Restriction>
        </rdfs:subClassOf>
        <rdfs:subClassOf>
            <owl:Restriction>
                <owl:onProperty rdf:resource="http://www.w3.org/2003/01/geo/wgs84_pos#location"/>
                <owl:qualifiedCardinality rdf:datatype="http://www.w3.org/2001/XMLSchema#nonNegativeInteger">1</owl:qualifiedCardinality>
                <owl:onClass rdf:resource="http://www.w3.org/2003/01/geo/wgs84_pos#Point"/>
            </owl:Restriction>
        </rdfs:subClassOf>
        <dc:source>skos:exactMatch &apos;platform&apos; [SensorML OGC-0700]
                                  http://www.opengeospatial.org/standards/sensorml</dc:source>
        <rdfs:comment>An Entity to which other Entities can be attached - particularly Sensors and other Platforms.  For example, a post might act as the Platform, a buoy might act as a Platform, or a fish might act as a Platform for an attached sensor.</rdfs:comment>
        <rdfs:label xml:lang="en">Platform</rdfs:label>
        <rdfs:seeAlso>http://www.w3.org/2005/Incubator/ssn/wiki/SSN_Deploy#PlatformSite</rdfs:seeAlso>
    </owl:Class>
    


    <!-- http://purl.oclc.org/NET/ssnx/ssn#Precision -->

    <owl:Class rdf:about="http://purl.oclc.org/NET/ssnx/ssn#Precision">
        <rdfs:subClassOf rdf:resource="http://purl.oclc.org/NET/ssnx/ssn#MeasurementProperty"/>
        <dc:source>skos:exactMatch &apos;measurement precision/precision&apos; [VIM 2.15]
                                   http://www.bipm.org/utils/common/documents/jcgm/JCGM_200_2008.pdf</dc:source>
        <rdfs:comment>The closeness of agreement between replicate observations on an unchanged or similar quality value: i.e., a measure of a sensor&apos;s ability to consitently reproduce an observation.</rdfs:comment>
        <rdfs:isDefinedBy>http://purl.oclc.org/NET/ssnx/ssn</rdfs:isDefinedBy>
        <rdfs:label>Precision</rdfs:label>
        <rdfs:seeAlso>http://www.w3.org/2005/Incubator/ssn/wiki/SSN_Sensor#MeasuringCapability</rdfs:seeAlso>
    </owl:Class>
    


    <!-- http://purl.oclc.org/NET/ssnx/ssn#Resolution -->

    <owl:Class rdf:about="http://purl.oclc.org/NET/ssnx/ssn#Resolution">
        <rdfs:subClassOf rdf:resource="http://purl.oclc.org/NET/ssnx/ssn#MeasurementProperty"/>
        <dc:source>skos:exactMatch &apos;resolution&apos; [VIM 4.14]
                                  http://www.bipm.org/utils/common/documents/jcgm/JCGM_200_2008.pdf</dc:source>
        <rdfs:comment>The smallest difference in the value of a quality being observed that would result in perceptably different values of observation results.</rdfs:comment>
        <rdfs:isDefinedBy>http://purl.oclc.org/NET/ssnx/ssn</rdfs:isDefinedBy>
        <rdfs:label>Resolution</rdfs:label>
        <rdfs:seeAlso>http://www.w3.org/2005/Incubator/ssn/wiki/SSN_Sensor#MeasuringCapability</rdfs:seeAlso>
    </owl:Class>
    


    <!-- http://purl.oclc.org/NET/ssnx/ssn#ResponseTime -->

    <owl:Class rdf:about="http://purl.oclc.org/NET/ssnx/ssn#ResponseTime">
        <rdfs:subClassOf rdf:resource="http://purl.oclc.org/NET/ssnx/ssn#MeasurementProperty"/>
        <dc:source>skos:exactMatch &apos;step response time&apos; [VIM 4.23]
                                  http://www.bipm.org/utils/common/documents/jcgm/JCGM_200_2008.pdf</dc:source>
        <rdfs:comment>The time between a (step) change inthe value of an observed quality and a sensor (possibly with specified error) &apos;settling&apos; on an observed value.</rdfs:comment>
        <rdfs:isDefinedBy>http://purl.oclc.org/NET/ssnx/ssn</rdfs:isDefinedBy>
        <rdfs:label>Response time</rdfs:label>
        <rdfs:seeAlso>http://www.w3.org/2005/Incubator/ssn/wiki/SSN_Sensor#MeasuringCapability</rdfs:seeAlso>
    </owl:Class>
    


    <!-- http://purl.oclc.org/NET/ssnx/ssn#SensingDevice -->

    <owl:Class rdf:about="http://purl.oclc.org/NET/ssnx/ssn#SensingDevice">
        <owl:equivalentClass rdf:resource="http://www.onem2m.org/ontology/Base_Ontology/base_ontology#Device"/>
        <rdfs:subClassOf rdf:resource="http://purl.oclc.org/NET/ssnx/ssn#Device"/>
        <rdfs:subClassOf rdf:resource="http://purl.oclc.org/NET/ssnx/ssn#Sensor"/>
        <dc:source>http://www.w3.org/2005/Incubator/ssn/</dc:source>
        <rdfs:comment>A sensing device is a device that implements sensing.</rdfs:comment>
        <rdfs:label xml:lang="en">Sensing Device</rdfs:label>
        <rdfs:seeAlso>http://www.w3.org/2005/Incubator/ssn/wiki/SSN_Sensor#Measuring</rdfs:seeAlso>
    </owl:Class>
    


    <!-- http://purl.oclc.org/NET/ssnx/ssn#Sensor -->

    <owl:Class rdf:about="http://purl.oclc.org/NET/ssnx/ssn#Sensor">
        <owl:equivalentClass rdf:resource="http://www.onem2m.org/ontology/Base_Ontology/base_ontology#Thing"/>
        <rdfs:subClassOf>
            <owl:Restriction>
                <owl:onProperty rdf:resource="http://purl.oclc.org/NET/ssnx/ssn#madeObservation"/>
                <owl:someValuesFrom rdf:resource="http://purl.oclc.org/NET/ssnx/ssn#Observation"/>
            </owl:Restriction>
        </rdfs:subClassOf>
        <rdfs:subClassOf>
            <owl:Restriction>
                <owl:onProperty rdf:resource="http://purl.oclc.org/NET/UNIS/fiware/iot-lite#hasQuantityKind"/>
                <owl:qualifiedCardinality rdf:datatype="http://www.w3.org/2001/XMLSchema#nonNegativeInteger">1</owl:qualifiedCardinality>
                <owl:onClass rdf:resource="http://purl.org/NET/ssnx/qu/qu#QuantityKind"/>
            </owl:Restriction>
        </rdfs:subClassOf>
        <rdfs:subClassOf>
            <owl:Restriction>
                <owl:onProperty rdf:resource="http://purl.oclc.org/NET/UNIS/fiware/iot-lite#hasUnit"/>
                <owl:qualifiedCardinality rdf:datatype="http://www.w3.org/2001/XMLSchema#nonNegativeInteger">1</owl:qualifiedCardinality>
                <owl:onClass rdf:resource="http://purl.org/NET/ssnx/qu/qu#Unit"/>
            </owl:Restriction>
        </rdfs:subClassOf>
        <rdfs:subClassOf>
            <owl:Restriction>
                <owl:onProperty rdf:resource="http://purl.oclc.org/NET/ssnx/ssn#hasMeasurementCapability"/>
                <owl:qualifiedCardinality rdf:datatype="http://www.w3.org/2001/XMLSchema#nonNegativeInteger">1</owl:qualifiedCardinality>
                <owl:onClass rdf:resource="http://purl.oclc.org/NET/ssnx/ssn#MeasurementCapability"/>
            </owl:Restriction>
        </rdfs:subClassOf>
        <dc:source>skos:exactMatch &apos;sensor&apos; [SensorML OGC-0700]
		                    http://www.opengeospatial.org/standards/sensorml 

                                skos:closeMatch &apos;observation procedure&apos; [O&amp;M] 
                                http://www.opengeospatial.org/standards/om 

O&amp;M allows sensors, methods, instruments, systems, algorithms and process chains as the processUsed of an observation; this ontology allows a similar range of things (anything that can do sensing), just they are all grouped under the term sensor (which is thus wider than the O&amp;M concept).</dc:source>
        <rdfs:comment>A sensor can do (implements) sensing: that is, a sensor is any entity that can follow a sensing method and thus observe some Property of a FeatureOfInterest.  Sensors may be physical devices, computational methods, a laboratory setup with a person following a method, or any other thing that can follow a Sensing Method to observe a Property.</rdfs:comment>
        <rdfs:label xml:lang="en">Sensor</rdfs:label>
        <rdfs:seeAlso>http://www.w3.org/2005/Incubator/ssn/wiki/SSN_Skeleton#Skeleton</rdfs:seeAlso>
    </owl:Class>
    


    <!-- http://purl.oclc.org/NET/ssnx/ssn#SensorOutput -->

    <owl:Class rdf:about="http://purl.oclc.org/NET/ssnx/ssn#SensorOutput">
        <rdfs:subClassOf>
            <owl:Restriction>
                <owl:onProperty rdf:resource="http://purl.oclc.org/NET/ssnx/ssn#hasValue"/>
                <owl:qualifiedCardinality rdf:datatype="http://www.w3.org/2001/XMLSchema#nonNegativeInteger">1</owl:qualifiedCardinality>
                <owl:onClass rdf:resource="http://purl.oclc.org/NET/ssnx/ssn#ObservationValue"/>
            </owl:Restriction>
        </rdfs:subClassOf>
        <rdfs:comment>A sensor outputs a piece of information (an observed value), the value itself being represented by an ObservationValue.</rdfs:comment>
        <rdfs:label xml:lang="en">Sensor Output</rdfs:label>
        <rdfs:seeAlso>http://www.w3.org/2005/Incubator/ssn/wiki/SSN_Skeleton#Skeleton</rdfs:seeAlso>
    </owl:Class>
    


    <!-- http://purl.oclc.org/NET/ssnx/ssn#System -->

    <owl:Class rdf:about="http://purl.oclc.org/NET/ssnx/ssn#System">
        <rdfs:subClassOf>
            <owl:Restriction>
                <owl:onProperty rdf:resource="http://purl.oclc.org/NET/ssnx/ssn#hasSubSystem"/>
                <owl:someValuesFrom rdf:resource="http://purl.oclc.org/NET/ssnx/ssn#System"/>
            </owl:Restriction>
        </rdfs:subClassOf>
        <rdfs:subClassOf>
            <owl:Restriction>
                <owl:onProperty rdf:resource="http://purl.oclc.org/NET/UNIS/fiware/iot-lite#isSubSystemOf"/>
                <owl:qualifiedCardinality rdf:datatype="http://www.w3.org/2001/XMLSchema#nonNegativeInteger">1</owl:qualifiedCardinality>
                <owl:onClass rdf:resource="http://purl.oclc.org/NET/ssnx/ssn#System"/>
            </owl:Restriction>
        </rdfs:subClassOf>
        <rdfs:subClassOf>
            <owl:Restriction>
                <owl:onProperty rdf:resource="http://purl.oclc.org/NET/ssnx/ssn#hasDeployment"/>
                <owl:qualifiedCardinality rdf:datatype="http://www.w3.org/2001/XMLSchema#nonNegativeInteger">1</owl:qualifiedCardinality>
                <owl:onClass rdf:resource="http://purl.oclc.org/NET/ssnx/ssn#Deployment"/>
            </owl:Restriction>
        </rdfs:subClassOf>
        <rdfs:subClassOf>
            <owl:Restriction>
                <owl:onProperty rdf:resource="http://purl.oclc.org/NET/ssnx/ssn#onPlatform"/>
                <owl:qualifiedCardinality rdf:datatype="http://www.w3.org/2001/XMLSchema#nonNegativeInteger">1</owl:qualifiedCardinality>
                <owl:onClass rdf:resource="http://purl.oclc.org/NET/ssnx/ssn#Platform"/>
            </owl:Restriction>
        </rdfs:subClassOf>
        <dc:source>http://www.w3.org/2005/Incubator/ssn/</dc:source>
        <rdfs:comment>System is a unit of abstraction for pieces of infrastructure (and we largely care that they are) for sensing. A system has components, its subsystems, which are other systems.</rdfs:comment>
        <rdfs:label xml:lang="en">System</rdfs:label>
        <rdfs:seeAlso>http://www.w3.org/2005/Incubator/ssn/wiki/SSN_Model#System</rdfs:seeAlso>
    </owl:Class>
    


    <!-- http://purl.org/NET/ssnx/qu/qu#QuantityKind -->

    <owl:Class rdf:about="http://purl.org/NET/ssnx/qu/qu#QuantityKind">
        <owl:equivalentClass rdf:resource="http://www.onem2m.org/ontology/Base_Ontology/base_ontology#ThingProperty"/>
        <rdfs:subClassOf>
            <owl:Restriction>
                <owl:onProperty rdf:resource="http://purl.org/iot/vocab/m3-lite#hasSource"/>
                <owl:someValuesFrom rdf:resource="http://purl.org/iot/vocab/m3-lite#Source"/>
            </owl:Restriction>
        </rdfs:subClassOf>
        <rdfs:comment xml:lang="en">A QuantityKind is an abstract classifier that represents the concept of kind of quantity that is defined as aspect common to mutually comparable quantities. A QuantityKind represents the essence of a quantity without any numerical value or unit. Quantities of the same kind within a given system of quantities have the same quantity dimension. However, quantities of the same dimension are not necessarily of the same kind.</rdfs:comment>
        <rdfs:label xml:lang="en">Quantity Kind</rdfs:label>
    </owl:Class>
    


    <!-- http://purl.org/NET/ssnx/qu/qu#Unit -->

    <owl:Class rdf:about="http://purl.org/NET/ssnx/qu/qu#Unit">
        <owl:equivalentClass rdf:resource="http://www.onem2m.org/ontology/Base_Ontology/base_ontology#MetaData"/>
        <rdfs:comment xml:lang="en">A Unit is an abstract classifier that represents the concept of measurement unit that is defined as real scalar quantity, defined and adopted by convention, with which any other quantity of the same kind can be compared to express the ratio of the two quantities as a number.
        </rdfs:comment>
        <rdfs:label xml:lang="en">Unit</rdfs:label>
    </owl:Class>
    


    <!-- http://purl.org/iot/ontology/fiesta-iot#Water_Flow -->

    <owl:Class rdf:about="http://purl.org/iot/ontology/fiesta-iot#Water_Flow">
        <rdfs:subClassOf rdf:resource="http://purl.oclc.org/NET/ssnx/ssn#SensingDevice"/>
    </owl:Class>
    


    <!-- http://purl.org/iot/vocab/m3-lite#ABS -->

    <owl:Class rdf:about="http://purl.org/iot/vocab/m3-lite#ABS">
        <rdfs:subClassOf rdf:resource="http://purl.oclc.org/NET/UNIS/fiware/iot-lite#ActuatingDevice"/>
        <rdfs:subClassOf>
            <owl:Restriction>
                <owl:onProperty rdf:resource="http://purl.org/iot/vocab/m3-lite#hasDomainOfInterest"/>
                <owl:someValuesFrom rdf:resource="http://purl.org/iot/vocab/m3-lite#Transportation"/>
            </owl:Restriction>
        </rdfs:subClassOf>
        <rdfs:comment xml:lang="en">The ABS (Anti-lock Braking System) receives information from ABS computer to control the pressure on the breaks, This helps the wheels not to get locked up, it adjust the break pressure and prevents the wheels from locking. (Definition Source Google).</rdfs:comment>
        <rdfs:label xml:lang="en">ABS (Anti-lock Braking System) Actuating Device</rdfs:label>
    </owl:Class>
    


    <!-- http://purl.org/iot/vocab/m3-lite#AccInitialERabEstabSuccRate -->

    <owl:Class rdf:about="http://purl.org/iot/vocab/m3-lite#AccInitialERabEstabSuccRate">
        <rdfs:subClassOf rdf:resource="http://purl.org/iot/vocab/m3-lite#Communication"/>
        <rdfs:comment xml:lang="en">Initial E-UTRAN Radio Access Bearer establishment success rate.</rdfs:comment>
        <rdfs:label xml:lang="en">Initial E-RAB Establishment Success Rate</rdfs:label>
    </owl:Class>
    


    <!-- http://purl.org/iot/vocab/m3-lite#AccInitialERabSetupSuccRate -->

    <owl:Class rdf:about="http://purl.org/iot/vocab/m3-lite#AccInitialERabSetupSuccRate">
        <rdfs:subClassOf rdf:resource="http://purl.org/iot/vocab/m3-lite#Communication"/>
        <rdfs:comment xml:lang="en">Initial E-UTRAN Radio Access Bearer setup success rate.</rdfs:comment>
        <rdfs:label xml:lang="en">Initial E-RAB Setup Success Rate</rdfs:label>
    </owl:Class>
    


    <!-- http://purl.org/iot/vocab/m3-lite#AccRrcConnSetupSuccRate -->

    <owl:Class rdf:about="http://purl.org/iot/vocab/m3-lite#AccRrcConnSetupSuccRate">
        <rdfs:subClassOf rdf:resource="http://purl.org/iot/vocab/m3-lite#Communication"/>
        <rdfs:comment xml:lang="en">Radio Resource Control connection setup success rate.</rdfs:comment>
        <rdfs:label xml:lang="en">RRC Connection Setup Success Rate</rdfs:label>
    </owl:Class>
    


    <!-- http://purl.org/iot/vocab/m3-lite#AccS1SigEstabSuccRate -->

    <owl:Class rdf:about="http://purl.org/iot/vocab/m3-lite#AccS1SigEstabSuccRate">
        <rdfs:subClassOf rdf:resource="http://purl.org/iot/vocab/m3-lite#Communication"/>
        <rdfs:comment xml:lang="en">S1 (S1 standardized interface between eNB and Evolved Packet Core) signalling establishment success rate.</rdfs:comment>
        <rdfs:label xml:lang="en">S1 Signalling Establishment Success Rate</rdfs:label>
    </owl:Class>
    


    <!-- http://purl.org/iot/vocab/m3-lite#Acceleration -->

    <owl:Class rdf:about="http://purl.org/iot/vocab/m3-lite#Acceleration">
        <rdfs:subClassOf rdf:resource="http://purl.org/NET/ssnx/qu/qu#QuantityKind"/>
        <rdfs:comment xml:lang="en">The rate of change of the velocity of a particle with respect to time.</rdfs:comment>
        <rdfs:label xml:lang="en">Acceleration</rdfs:label>
        <rdfs:seeAlso>http://purl.oclc.org/NET/ssnx/qu/dim#Acceleration</rdfs:seeAlso>
    </owl:Class>
    


    <!-- http://purl.org/iot/vocab/m3-lite#AccelerationInstantaneous -->

    <owl:Class rdf:about="http://purl.org/iot/vocab/m3-lite#AccelerationInstantaneous">
        <rdfs:subClassOf rdf:resource="http://purl.org/iot/vocab/m3-lite#Acceleration"/>
        <rdfs:comment xml:lang="en">The acceleration at a given instant of time.</rdfs:comment>
        <rdfs:label xml:lang="en">Instantaneous Acceleration</rdfs:label>
    </owl:Class>
    


    <!-- http://purl.org/iot/vocab/m3-lite#Accelerometer -->

    <owl:Class rdf:about="http://purl.org/iot/vocab/m3-lite#Accelerometer">
        <rdfs:subClassOf rdf:resource="http://purl.oclc.org/NET/ssnx/ssn#SensingDevice"/>
        <rdfs:subClassOf>
            <owl:Restriction>
                <owl:onProperty rdf:resource="http://purl.org/iot/vocab/m3-lite#hasDomainOfInterest"/>
                <owl:someValuesFrom rdf:resource="http://purl.org/iot/vocab/m3-lite#Transportation"/>
            </owl:Restriction>
        </rdfs:subClassOf>
        <rdfs:comment xml:lang="en"> Accelerometers are used to automatically determine the orientation in which the user is holding the IoT Object (portrait or landscape).</rdfs:comment>
        <rdfs:label xml:lang="en">Accelerometer</rdfs:label>
        <rdfs:seeAlso rdf:resource="http://casas.wsu.edu/owl/cose.owl#Accelerometer"/>
    </owl:Class>
    


    <!-- http://purl.org/iot/vocab/m3-lite#ActivePower -->

    <owl:Class rdf:about="http://purl.org/iot/vocab/m3-lite#ActivePower">
        <rdfs:subClassOf rdf:resource="http://purl.org/iot/vocab/m3-lite#Power"/>
        <rdfs:comment xml:lang="en">The product of the voltage across a branch of an alternating-current circuit and the component of the electric current that is in phase with the voltage.</rdfs:comment>
        <rdfs:label xml:lang="en">Active Power</rdfs:label>
        <rdfs:seeAlso>http://purl.oclc.org/NET/ssnx/qu/quantity#activePower</rdfs:seeAlso>
    </owl:Class>
    


    <!-- http://purl.org/iot/vocab/m3-lite#Agriculture -->

    <owl:Class rdf:about="http://purl.org/iot/vocab/m3-lite#Agriculture">
        <rdfs:subClassOf rdf:resource="http://purl.org/iot/vocab/m3-lite#DomainOfInterest"/>
        <rdfs:comment xml:lang="en">Agriculture, Smart farm as an Internet of Things (IoT) applicative domain.</rdfs:comment>
        <rdfs:label xml:lang="en">Agriculture DOI</rdfs:label>
    </owl:Class>
    


    <!-- http://purl.org/iot/vocab/m3-lite#AirConditioner -->

    <owl:Class rdf:about="http://purl.org/iot/vocab/m3-lite#AirConditioner">
        <rdfs:subClassOf rdf:resource="http://purl.oclc.org/NET/UNIS/fiware/iot-lite#ActuatingDevice"/>
        <rdfs:subClassOf>
            <owl:Restriction>
                <owl:onProperty rdf:resource="http://purl.org/iot/vocab/m3-lite#hasDomainOfInterest"/>
                <owl:someValuesFrom rdf:resource="http://purl.org/iot/vocab/m3-lite#BuildingAutomation"/>
            </owl:Restriction>
        </rdfs:subClassOf>
        <rdfs:subClassOf>
            <owl:Restriction>
                <owl:onProperty rdf:resource="http://purl.org/iot/vocab/m3-lite#hasDomainOfInterest"/>
                <owl:someValuesFrom rdf:resource="http://purl.org/iot/vocab/m3-lite#Transportation"/>
            </owl:Restriction>
        </rdfs:subClassOf>
        <rdfs:comment xml:lang="en">An actuator to automatically switch on/off the air conditioner.</rdfs:comment>
        <rdfs:label xml:lang="en">Air Conditioner Actuating Device</rdfs:label>
    </owl:Class>
    


    <!-- http://purl.org/iot/vocab/m3-lite#AirHumiditySensor -->

    <owl:Class rdf:about="http://purl.org/iot/vocab/m3-lite#AirHumiditySensor">
        <rdfs:subClassOf rdf:resource="http://purl.org/iot/vocab/m3-lite#HumiditySensor"/>
        <rdfs:subClassOf>
            <owl:Restriction>
                <owl:onProperty rdf:resource="http://purl.org/iot/vocab/m3-lite#hasDomainOfInterest"/>
                <owl:someValuesFrom rdf:resource="http://purl.org/iot/vocab/m3-lite#Environment"/>
            </owl:Restriction>
        </rdfs:subClassOf>
        <rdfs:comment xml:lang="en">Sensor used to measure air humidity.</rdfs:comment>
        <rdfs:label xml:lang="en">Air Humidity Sensor</rdfs:label>
    </owl:Class>
    


    <!-- http://purl.org/iot/vocab/m3-lite#AirPollutantSensor -->

    <owl:Class rdf:about="http://purl.org/iot/vocab/m3-lite#AirPollutantSensor">
        <rdfs:subClassOf rdf:resource="http://purl.oclc.org/NET/ssnx/ssn#SensingDevice"/>
        <rdfs:subClassOf>
            <owl:Restriction>
                <owl:onProperty rdf:resource="http://purl.org/iot/vocab/m3-lite#hasDomainOfInterest"/>
                <owl:someValuesFrom rdf:resource="http://purl.org/iot/vocab/m3-lite#Environment"/>
            </owl:Restriction>
        </rdfs:subClassOf>
        <rdfs:comment xml:lang="en">Air Pollutant Sensor are devices that detect and monitor the presence of air pollution in the surrounding area (source Wikipedia).</rdfs:comment>
        <rdfs:label xml:lang="en">Air Pollutant Sensor</rdfs:label>
    </owl:Class>
    


    <!-- http://purl.org/iot/vocab/m3-lite#AirPollution -->

    <owl:Class rdf:about="http://purl.org/iot/vocab/m3-lite#AirPollution">
        <rdfs:subClassOf rdf:resource="http://purl.org/NET/ssnx/qu/qu#QuantityKind"/>
        <rdfs:comment xml:lang="en">Usually measured using Air Quality Index (AQI), it is the measure of Air Pollution in the environment. It is similar to Air Quality.</rdfs:comment>
        <rdfs:label xml:lang="en">Air Pollution Quantity Kind</rdfs:label>
    </owl:Class>
    


    <!-- http://purl.org/iot/vocab/m3-lite#AirQuality -->

    <owl:Class rdf:about="http://purl.org/iot/vocab/m3-lite#AirQuality">
        <rdfs:subClassOf rdf:resource="http://purl.org/NET/ssnx/qu/qu#QuantityKind"/>
        <rdfs:comment xml:lang="en">Usually measured using an air quality index (AQI) that is a number used by government agencies to communicate to the public how polluted the air currently is or how polluted it is forecast to become. Different countries have their own air quality indices, corresponding to different national air quality standards. It is the measure of Air Quality of the environment. It is similar to Air Pollution. (Source Wikipedia).</rdfs:comment>
        <rdfs:label xml:lang="en">Air Quality Quantity Kind</rdfs:label>
    </owl:Class>
    


    <!-- http://purl.org/iot/vocab/m3-lite#AirTemperature -->

    <owl:Class rdf:about="http://purl.org/iot/vocab/m3-lite#AirTemperature">
        <rdfs:subClassOf rdf:resource="http://purl.org/iot/vocab/m3-lite#Temperature"/>
        <rdfs:comment xml:lang="en">The temperature of the air that would be indicated by a thermometer exposed to the air at a location sheltered from direct solar radiation.</rdfs:comment>
        <rdfs:label xml:lang="en">Air Temperature, Weather Temperature, Ambient Temperature</rdfs:label>
        <rdfs:seeAlso rdf:resource="http://openiot.eu/ontology/ns/AirTemperature"/>
        <rdfs:seeAlso rdf:resource="http://paul.staroch.name/thesis/SmartHomeWeather.owl#Temperature"/>
    </owl:Class>
    


    <!-- http://purl.org/iot/vocab/m3-lite#AirThermometer -->

    <owl:Class rdf:about="http://purl.org/iot/vocab/m3-lite#AirThermometer">
        <rdfs:subClassOf rdf:resource="http://purl.org/iot/vocab/m3-lite#Thermometer"/>
        <rdfs:comment xml:lang="en">Device to measure the Air temperature of either indoor or outdoor atmosphere.</rdfs:comment>
        <rdfs:label xml:lang="en">Air Thermometer</rdfs:label>
    </owl:Class>
    


    <!-- http://purl.org/iot/vocab/m3-lite#AlarmSystem -->

    <owl:Class rdf:about="http://purl.org/iot/vocab/m3-lite#AlarmSystem">
        <rdfs:subClassOf rdf:resource="http://purl.oclc.org/NET/UNIS/fiware/iot-lite#ActuatingDevice"/>
        <rdfs:comment xml:lang="en">An actuator to automatically switch on/off the alarm system.</rdfs:comment>
        <rdfs:label xml:lang="en">Alarm System Actuating Device</rdfs:label>
    </owl:Class>
    


    <!-- http://purl.org/iot/vocab/m3-lite#AlcoholLevel -->

    <owl:Class rdf:about="http://purl.org/iot/vocab/m3-lite#AlcoholLevel">
        <rdfs:subClassOf rdf:resource="http://purl.org/NET/ssnx/qu/qu#QuantityKind"/>
        <rdfs:comment xml:lang="en">Measure of Alcohol Level in the system.</rdfs:comment>
        <rdfs:label xml:lang="en">Alcohol Level Quantity Kind</rdfs:label>
    </owl:Class>
    


    <!-- http://purl.org/iot/vocab/m3-lite#AlcoholLevelSensor -->

    <owl:Class rdf:about="http://purl.org/iot/vocab/m3-lite#AlcoholLevelSensor">
        <rdfs:subClassOf rdf:resource="http://purl.oclc.org/NET/ssnx/ssn#SensingDevice"/>
        <rdfs:subClassOf>
            <owl:Restriction>
                <owl:onProperty rdf:resource="http://purl.org/iot/vocab/m3-lite#hasDomainOfInterest"/>
                <owl:someValuesFrom rdf:resource="http://purl.org/iot/vocab/m3-lite#Transportation"/>
            </owl:Restriction>
        </rdfs:subClassOf>
        <rdfs:comment xml:lang="en">Device used to detect and measure Alcohol Level in the system.</rdfs:comment>
        <rdfs:label xml:lang="en">Alcohol Level Sensor</rdfs:label>
    </owl:Class>
    


    <!-- http://purl.org/iot/vocab/m3-lite#Ampere -->

    <owl:Class rdf:about="http://purl.org/iot/vocab/m3-lite#Ampere">
        <rdfs:subClassOf rdf:resource="http://purl.org/NET/ssnx/qu/qu#Unit"/>
        <rdfs:comment xml:lang="en">The ampere is the SI unit for measuring an electric current which is the flow of electric charges through a surface at the rate of one coulomb per second.The ampere is the SI unit for measuring an electric current which is the flow of electric charges through a surface at the rate of one coulomb per second.</rdfs:comment>
        <rdfs:label xml:lang="en">Ampere (A)</rdfs:label>
        <rdfs:seeAlso rdf:resource="http://data.qudt.org/qudt/owl/1.0.0/unit.owl#Ampere"/>
        <rdfs:seeAlso rdf:resource="http://sweet.jpl.nasa.gov/ontology/units.owl#ampere"/>
        <rdfs:seeAlso>http://purl.oclc.org/NET/ssnx/qu/unit#ampere</rdfs:seeAlso>
    </owl:Class>
    


    <!-- http://purl.org/iot/vocab/m3-lite#AngularSpeed -->

    <owl:Class rdf:about="http://purl.org/iot/vocab/m3-lite#AngularSpeed">
        <rdfs:subClassOf rdf:resource="http://purl.org/NET/ssnx/qu/qu#QuantityKind"/>
        <rdfs:comment xml:lang="en">It is the rate of change of angular displacement and is a vector quantity (more precisely, a pseudovector) that specifies the angular speed (rotational speed) of an object and the axis about which the object is rotating. (Source Wikipedia).</rdfs:comment>
        <rdfs:label xml:lang="en">Angular Speed</rdfs:label>
    </owl:Class>
    


    <!-- http://purl.org/iot/vocab/m3-lite#Animals -->

    <owl:Class rdf:about="http://purl.org/iot/vocab/m3-lite#Animals">
        <rdfs:subClassOf rdf:resource="http://purl.org/iot/vocab/m3-lite#SoundSource"/>
        <rdfs:comment xml:lang="en">when the source of the sound were animals.</rdfs:comment>
        <rdfs:label xml:lang="en">Animals as Sound Source</rdfs:label>
    </owl:Class>
    


    <!-- http://purl.org/iot/vocab/m3-lite#AtmosphericPressure -->

    <owl:Class rdf:about="http://purl.org/iot/vocab/m3-lite#AtmosphericPressure">
        <rdfs:subClassOf rdf:resource="http://purl.org/iot/vocab/m3-lite#Pressure"/>
        <rdfs:comment xml:lang="en">The pressure exerted by the atmosphere as a consequence of gravitational attraction exerted upon the column of air lying directly above the point in question.</rdfs:comment>
        <rdfs:label xml:lang="en">Atmospheric Pressure</rdfs:label>
        <rdfs:seeAlso rdf:resource="http://openiot.eu/ontology/ns/AtmospherePressure"/>
        <rdfs:seeAlso rdf:resource="http://paul.staroch.name/thesis/SmartHomeWeather.owl#AtmosphericPressure"/>
        <rdfs:seeAlso>http://purl.oclc.org/NET/ssnx/qu/quantity#atmosphericPressure</rdfs:seeAlso>
    </owl:Class>
    


    <!-- http://purl.org/iot/vocab/m3-lite#AtmosphericPressureSensor -->

    <owl:Class rdf:about="http://purl.org/iot/vocab/m3-lite#AtmosphericPressureSensor">
        <rdfs:subClassOf rdf:resource="http://purl.oclc.org/NET/ssnx/ssn#SensingDevice"/>
        <rdfs:subClassOf>
            <owl:Restriction>
                <owl:onProperty rdf:resource="http://purl.org/iot/vocab/m3-lite#hasDomainOfInterest"/>
                <owl:someValuesFrom rdf:resource="http://purl.org/iot/vocab/m3-lite#Agriculture"/>
            </owl:Restriction>
        </rdfs:subClassOf>
        <rdfs:subClassOf>
            <owl:Restriction>
                <owl:onProperty rdf:resource="http://purl.org/iot/vocab/m3-lite#hasDomainOfInterest"/>
                <owl:someValuesFrom rdf:resource="http://purl.org/iot/vocab/m3-lite#Weather"/>
            </owl:Restriction>
        </rdfs:subClassOf>
        <rdfs:comment xml:lang="en">Atmospheric Pressure Sensor, Barometer or Barometric Pressure Sensor is a scientific instrument used in meteorology to measure atmospheric pressure.</rdfs:comment>
        <rdfs:label xml:lang="en">Atmospheric Pressure Sensor</rdfs:label>
        <rdfs:seeAlso rdf:resource="http://archive.knoesis.org/research/semsci/application_domain/sem_sensor/ont/weather.owlPressure"/>
        <rdfs:seeAlso rdf:resource="http://casas.wsu.edu/owl/cose.owl#BarometricPressureSensor"/>
        <rdfs:seeAlso rdf:resource="http://purl.oclc.org/NET/ssnx/meteo/aws#AtmosphericPressureSensor"/>
    </owl:Class>
    


    <!-- http://purl.org/iot/vocab/m3-lite#AutomaticSensing -->

    <owl:Class rdf:about="http://purl.org/iot/vocab/m3-lite#AutomaticSensing">
        <rdfs:subClassOf rdf:resource="http://purl.org/iot/vocab/m3-lite#MeasurementType"/>
        <rdfs:comment xml:lang="en">When the devices are set to take the observations Automatically without any external aid.</rdfs:comment>
        <rdfs:label xml:lang="en">Automatic Measurement Type</rdfs:label>
    </owl:Class>
    


    <!-- http://purl.org/iot/vocab/m3-lite#Bar -->

    <owl:Class rdf:about="http://purl.org/iot/vocab/m3-lite#Bar">
        <rdfs:subClassOf rdf:resource="http://purl.org/NET/ssnx/qu/qu#Unit"/>
        <rdfs:comment xml:lang="en">Metric unit of atmospheric pressure equal to 14.50 pounds per square inch (lb/in2), 1.02 kilograms per square centimetre (kg/cm2), 29.53 inches of mercury (in Hg), or 0.9869 atmosphere.</rdfs:comment>
        <rdfs:label xml:lang="en">Bar</rdfs:label>
        <rdfs:seeAlso>http://qudt.org/vocab/unit#Bar</rdfs:seeAlso>
    </owl:Class>
    


    <!-- http://purl.org/iot/vocab/m3-lite#Barcode -->

    <owl:Class rdf:about="http://purl.org/iot/vocab/m3-lite#Barcode">
        <rdfs:subClassOf rdf:resource="http://purl.oclc.org/NET/UNIS/fiware/iot-lite#TagDevice"/>
        <rdfs:comment xml:lang="en">A tagging device can be Barcode.</rdfs:comment>
        <rdfs:label xml:lang="en">Barcode Tagging Device</rdfs:label>
    </owl:Class>
    


    <!-- http://purl.org/iot/vocab/m3-lite#BatteryLevel -->

    <owl:Class rdf:about="http://purl.org/iot/vocab/m3-lite#BatteryLevel">
        <rdfs:subClassOf rdf:resource="http://purl.org/NET/ssnx/qu/qu#QuantityKind"/>
        <rdfs:comment xml:lang="en">Measure of the percentage of the battery capacity that remains available.</rdfs:comment>
        <rdfs:label xml:lang="en">Battery Level Quantity Kind</rdfs:label>
        <rdfs:seeAlso>http://www.w3.org/2007/uwa/context/deliveryContext.owl#BatteryLevel</rdfs:seeAlso>
    </owl:Class>
    


    <!-- http://purl.org/iot/vocab/m3-lite#BeatPerMinute -->

    <owl:Class rdf:about="http://purl.org/iot/vocab/m3-lite#BeatPerMinute">
        <rdfs:subClassOf rdf:resource="http://purl.org/NET/ssnx/qu/qu#Unit"/>
        <rdfs:comment xml:lang="en">BeatPerMinute (bpm) is the unit to measure heart rate.</rdfs:comment>
        <rdfs:label xml:lang="en">Beat Per Minute (bpm)</rdfs:label>
    </owl:Class>
    


    <!-- http://purl.org/iot/vocab/m3-lite#Blind -->

    <owl:Class rdf:about="http://purl.org/iot/vocab/m3-lite#Blind">
        <rdfs:subClassOf rdf:resource="http://purl.oclc.org/NET/UNIS/fiware/iot-lite#ActuatingDevice"/>
        <rdfs:subClassOf>
            <owl:Restriction>
                <owl:onProperty rdf:resource="http://purl.org/iot/vocab/m3-lite#hasDomainOfInterest"/>
                <owl:someValuesFrom rdf:resource="http://purl.org/iot/vocab/m3-lite#BuildingAutomation"/>
            </owl:Restriction>
        </rdfs:subClassOf>
        <rdfs:comment xml:lang="en">An actuator to automatically switch on/off the window blinds.</rdfs:comment>
        <rdfs:label xml:lang="en">Blind Actuating Device</rdfs:label>
    </owl:Class>
    


    <!-- http://purl.org/iot/vocab/m3-lite#BloodGlucose -->

    <owl:Class rdf:about="http://purl.org/iot/vocab/m3-lite#BloodGlucose">
        <rdfs:subClassOf rdf:resource="http://purl.org/NET/ssnx/qu/qu#QuantityKind"/>
        <rdfs:comment xml:lang="en">Measure of Blood glucose level or blood sugar level.</rdfs:comment>
        <rdfs:label xml:lang="en">Blood Glucose Quantity Kind</rdfs:label>
    </owl:Class>
    


    <!-- http://purl.org/iot/vocab/m3-lite#BloodPressure -->

    <owl:Class rdf:about="http://purl.org/iot/vocab/m3-lite#BloodPressure">
        <rdfs:subClassOf rdf:resource="http://purl.org/iot/vocab/m3-lite#Pressure"/>
        <rdfs:comment xml:lang="en">Measure of the pressure in your blood vessels when your heart rests between beats.</rdfs:comment>
        <rdfs:label xml:lang="en">Blood Pressure</rdfs:label>
    </owl:Class>
    


    <!-- http://purl.org/iot/vocab/m3-lite#BloodPressureSensor -->

    <owl:Class rdf:about="http://purl.org/iot/vocab/m3-lite#BloodPressureSensor">
        <rdfs:subClassOf rdf:resource="http://purl.oclc.org/NET/ssnx/ssn#SensingDevice"/>
        <rdfs:subClassOf>
            <owl:Restriction>
                <owl:onProperty rdf:resource="http://purl.org/iot/vocab/m3-lite#hasDomainOfInterest"/>
                <owl:someValuesFrom rdf:resource="http://purl.org/iot/vocab/m3-lite#Health"/>
            </owl:Restriction>
        </rdfs:subClassOf>
        <rdfs:comment xml:lang="en">Device used to measure Blood Pressure.</rdfs:comment>
        <rdfs:label xml:lang="en">Blood Pressure Sensor</rdfs:label>
    </owl:Class>
    


    <!-- http://purl.org/iot/vocab/m3-lite#BoardTemperature -->

    <owl:Class rdf:about="http://purl.org/iot/vocab/m3-lite#BoardTemperature">
        <rdfs:subClassOf rdf:resource="http://purl.org/iot/vocab/m3-lite#Temperature"/>
        <rdfs:comment xml:lang="en">Measure of board temperature.</rdfs:comment>
        <rdfs:label xml:lang="en">Board Temperature</rdfs:label>
    </owl:Class>
    


    <!-- http://purl.org/iot/vocab/m3-lite#BoardThermometer -->

    <owl:Class rdf:about="http://purl.org/iot/vocab/m3-lite#BoardThermometer">
        <rdfs:subClassOf rdf:resource="http://purl.org/iot/vocab/m3-lite#Thermometer"/>
        <rdfs:comment xml:lang="en">Device used to measure board temperature.</rdfs:comment>
        <rdfs:label xml:lang="en">Board Thermometer</rdfs:label>
    </owl:Class>
    


    <!-- http://purl.org/iot/vocab/m3-lite#BoardVoltageSensor -->

    <owl:Class rdf:about="http://purl.org/iot/vocab/m3-lite#BoardVoltageSensor">
        <rdfs:subClassOf rdf:resource="http://purl.org/iot/vocab/m3-lite#VoltageSensor"/>
        <rdfs:comment xml:lang="en">Sensor used to measure board input voltage.</rdfs:comment>
        <rdfs:label xml:lang="en">Board Voltage Sensor</rdfs:label>
    </owl:Class>
    


    <!-- http://purl.org/iot/vocab/m3-lite#BodyTemperature -->

    <owl:Class rdf:about="http://purl.org/iot/vocab/m3-lite#BodyTemperature">
        <rdfs:subClassOf rdf:resource="http://purl.org/iot/vocab/m3-lite#Temperature"/>
        <rdfs:comment xml:lang="en">Measure of body temperature.</rdfs:comment>
        <rdfs:label xml:lang="en">Body Temperature</rdfs:label>
    </owl:Class>
    


    <!-- http://purl.org/iot/vocab/m3-lite#BodyThermometer -->

    <owl:Class rdf:about="http://purl.org/iot/vocab/m3-lite#BodyThermometer">
        <rdfs:subClassOf rdf:resource="http://purl.org/iot/vocab/m3-lite#Thermometer"/>
        <rdfs:subClassOf>
            <owl:Restriction>
                <owl:onProperty rdf:resource="http://purl.org/iot/vocab/m3-lite#hasDomainOfInterest"/>
                <owl:someValuesFrom rdf:resource="http://purl.org/iot/vocab/m3-lite#Health"/>
            </owl:Restriction>
        </rdfs:subClassOf>
        <rdfs:comment xml:lang="en">Device used to measure body temperature.</rdfs:comment>
        <rdfs:label xml:lang="en">Body Thermometer</rdfs:label>
    </owl:Class>
    


    <!-- http://purl.org/iot/vocab/m3-lite#Boiler -->

    <owl:Class rdf:about="http://purl.org/iot/vocab/m3-lite#Boiler">
        <rdfs:subClassOf rdf:resource="http://purl.oclc.org/NET/UNIS/fiware/iot-lite#ActuatingDevice"/>
        <rdfs:subClassOf>
            <owl:Restriction>
                <owl:onProperty rdf:resource="http://purl.org/iot/vocab/m3-lite#hasDomainOfInterest"/>
                <owl:someValuesFrom rdf:resource="http://purl.org/iot/vocab/m3-lite#BuildingAutomation"/>
            </owl:Restriction>
        </rdfs:subClassOf>
        <rdfs:comment xml:lang="en">An actuator to automatically switch on/off the boiler.</rdfs:comment>
        <rdfs:label xml:lang="en">Boiler Actuating Device</rdfs:label>
    </owl:Class>
    


    <!-- http://purl.org/iot/vocab/m3-lite#BuildingAutomation -->

    <owl:Class rdf:about="http://purl.org/iot/vocab/m3-lite#BuildingAutomation">
        <rdfs:subClassOf rdf:resource="http://purl.org/iot/vocab/m3-lite#DomainOfInterest"/>
        <rdfs:comment xml:lang="en">Smart Home/Building Automation as an Internet of Things (IoT) applicative domain.</rdfs:comment>
        <rdfs:label xml:lang="en">Smart Building DOI</rdfs:label>
        <rdfs:seeAlso rdf:resource="http://elite.polito.it/ontologies/dogont.owl#BuildingEnvironment"/>
    </owl:Class>
    


    <!-- http://purl.org/iot/vocab/m3-lite#BuildingTemperature -->

    <owl:Class rdf:about="http://purl.org/iot/vocab/m3-lite#BuildingTemperature">
        <rdfs:subClassOf rdf:resource="http://purl.org/iot/vocab/m3-lite#Temperature"/>
        <rdfs:comment xml:lang="en">Measure of building or room temperature.</rdfs:comment>
        <rdfs:label xml:lang="en">Building/Room Temperature</rdfs:label>
    </owl:Class>
    


    <!-- http://purl.org/iot/vocab/m3-lite#CO2 -->

    <owl:Class rdf:about="http://purl.org/iot/vocab/m3-lite#CO2">
        <rdfs:subClassOf rdf:resource="http://purl.org/NET/ssnx/qu/qu#QuantityKind"/>
        <rdfs:comment xml:lang="en">Carbon Dioxide (CO2) measure in the atmosphere.</rdfs:comment>
        <rdfs:label xml:lang="en">Carbon Dioxide (CO2) Quantity Kind</rdfs:label>
    </owl:Class>
    


    <!-- http://purl.org/iot/vocab/m3-lite#CO2Sensor -->

    <owl:Class rdf:about="http://purl.org/iot/vocab/m3-lite#CO2Sensor">
        <rdfs:subClassOf rdf:resource="http://purl.org/iot/vocab/m3-lite#GaseousPollutantSensor"/>
        <rdfs:subClassOf>
            <owl:Restriction>
                <owl:onProperty rdf:resource="http://purl.org/iot/vocab/m3-lite#hasDomainOfInterest"/>
                <owl:someValuesFrom rdf:resource="http://purl.org/iot/vocab/m3-lite#Agriculture"/>
            </owl:Restriction>
        </rdfs:subClassOf>
        <rdfs:subClassOf>
            <owl:Restriction>
                <owl:onProperty rdf:resource="http://purl.org/iot/vocab/m3-lite#hasDomainOfInterest"/>
                <owl:someValuesFrom rdf:resource="http://purl.org/iot/vocab/m3-lite#Environment"/>
            </owl:Restriction>
        </rdfs:subClassOf>
        <rdfs:comment xml:lang="en">Carbon Dioxide (CO2) Sensor used to measure level of CO2 in the atmosphere.</rdfs:comment>
        <rdfs:label xml:lang="en">Carbon Dioxide (CO2) Sensor</rdfs:label>
    </owl:Class>
    


    <!-- http://purl.org/iot/vocab/m3-lite#COSensor -->

    <owl:Class rdf:about="http://purl.org/iot/vocab/m3-lite#COSensor">
        <rdfs:subClassOf rdf:resource="http://purl.org/iot/vocab/m3-lite#GaseousPollutantSensor"/>
        <rdfs:comment xml:lang="en">Device to detect Carbon Monoxide (CO) in the environment.</rdfs:comment>
        <rdfs:label xml:lang="en">Carbon Monoxide (CO) Sensor</rdfs:label>
    </owl:Class>
    


    <!-- http://purl.org/iot/vocab/m3-lite#Calcium -->

    <owl:Class rdf:about="http://purl.org/iot/vocab/m3-lite#Calcium">
        <rdfs:subClassOf rdf:resource="http://purl.org/NET/ssnx/qu/qu#QuantityKind"/>
        <rdfs:comment xml:lang="en">Measure of blood calcium level.</rdfs:comment>
        <rdfs:label xml:lang="en">Calcium Quantity Kind</rdfs:label>
    </owl:Class>
    


    <!-- http://purl.org/iot/vocab/m3-lite#Calibration -->

    <owl:Class rdf:about="http://purl.org/iot/vocab/m3-lite#Calibration">
        <rdfs:subClassOf rdf:resource="http://purl.org/NET/ssnx/qu/qu#QuantityKind"/>
        <rdfs:comment xml:lang="en">Measure of blood calcium level.</rdfs:comment>
        <rdfs:label xml:lang="en">Calcium Quantity Kind</rdfs:label>
    </owl:Class>
    


    <!-- http://purl.org/iot/vocab/m3-lite#Candela -->

    <owl:Class rdf:about="http://purl.org/iot/vocab/m3-lite#Candela">
        <rdfs:subClassOf rdf:resource="http://purl.org/NET/ssnx/qu/qu#Unit"/>
        <rdfs:comment xml:lang="en">Candela is the luminous intensity, in a given direction, of a source that emits monochromatic radiation of frequency 540 x 10^12 hertz and that has a radiant intensity in that direction of 1/683 watt per steradian. (Source Wikipedia).</rdfs:comment>
        <rdfs:label xml:lang="en">Candela</rdfs:label>
        <rdfs:seeAlso rdf:resource="http://sweet.jpl.nasa.gov/ontology/units.owl#candela"/>
    </owl:Class>
    


    <!-- http://purl.org/iot/vocab/m3-lite#Capacitance -->

    <owl:Class rdf:about="http://purl.org/iot/vocab/m3-lite#Capacitance">
        <rdfs:subClassOf rdf:resource="http://purl.org/NET/ssnx/qu/qu#QuantityKind"/>
        <rdfs:comment xml:lang="en">Measure of the ability of a system to store an electric charge.</rdfs:comment>
        <rdfs:label xml:lang="en">Capacitance</rdfs:label>
    </owl:Class>
    


    <!-- http://purl.org/iot/vocab/m3-lite#Centibar -->

    <owl:Class rdf:about="http://purl.org/iot/vocab/m3-lite#Centibar">
        <rdfs:subClassOf rdf:resource="http://purl.org/iot/vocab/m3-lite#Bar"/>
        <rdfs:comment xml:lang="en">The centibar is a unit of pressure defined as 1e-2 bar.</rdfs:comment>
        <rdfs:label xml:lang="en">Centibar</rdfs:label>
    </owl:Class>
    


    <!-- http://purl.org/iot/vocab/m3-lite#Centimetre -->

    <owl:Class rdf:about="http://purl.org/iot/vocab/m3-lite#Centimetre">
        <rdfs:subClassOf rdf:resource="http://purl.org/iot/vocab/m3-lite#Metre"/>
        <rdfs:comment xml:lang="en">A metric unit of length, equal to one hundredth of a metre.</rdfs:comment>
        <rdfs:label xml:lang="en">Centimetre, Centimeter</rdfs:label>
    </owl:Class>
    


    <!-- http://purl.org/iot/vocab/m3-lite#ChemicalAgentAtmosphericConcentration -->

    <owl:Class rdf:about="http://purl.org/iot/vocab/m3-lite#ChemicalAgentAtmosphericConcentration">
        <rdfs:subClassOf rdf:resource="http://purl.org/iot/vocab/m3-lite#ChemicalAgentConcentration"/>
        <rdfs:comment xml:lang="en">Measure of Chemical Agent Atmospheric Concentration</rdfs:comment>
        <rdfs:label xml:lang="en">Chemical Agent Atmospheric Concentration Quantity Kind</rdfs:label>
    </owl:Class>
    


    <!-- http://purl.org/iot/vocab/m3-lite#ChemicalAgentAtmosphericConcentrationAirParticles -->

    <owl:Class rdf:about="http://purl.org/iot/vocab/m3-lite#ChemicalAgentAtmosphericConcentrationAirParticles">
        <rdfs:subClassOf rdf:resource="http://purl.org/iot/vocab/m3-lite#ChemicalAgentAtmosphericConcentration"/>
        <rdfs:comment xml:lang="en">Measure of the concentration of chemical particles suspended in the atmosphere.</rdfs:comment>
        <rdfs:label xml:lang="en">Air Particles Chemical Agent Atmospheric Concentration</rdfs:label>
    </owl:Class>
    


    <!-- http://purl.org/iot/vocab/m3-lite#ChemicalAgentAtmosphericConcentrationCO -->

    <owl:Class rdf:about="http://purl.org/iot/vocab/m3-lite#ChemicalAgentAtmosphericConcentrationCO">
        <rdfs:subClassOf rdf:resource="http://purl.org/iot/vocab/m3-lite#ChemicalAgentAtmosphericConcentration"/>
        <rdfs:comment xml:lang="en">Measure of the concentration of Carbon Monoxide (CO) gas suspended in the atmosphere.</rdfs:comment>
        <rdfs:label xml:lang="en">Carbon Monoxide (CO) Chemical Agent Atmospheric Concentration</rdfs:label>
    </owl:Class>
    


    <!-- http://purl.org/iot/vocab/m3-lite#ChemicalAgentAtmosphericConcentrationDust -->

    <owl:Class rdf:about="http://purl.org/iot/vocab/m3-lite#ChemicalAgentAtmosphericConcentrationDust">
        <rdfs:subClassOf rdf:resource="http://purl.org/iot/vocab/m3-lite#ChemicalAgentAtmosphericConcentration"/>
        <rdfs:comment xml:lang="en">Measure of the concentration of dust suspended in the air.</rdfs:comment>
        <rdfs:label xml:lang="en">Chemical Agent Atmospheric Concentration Dust</rdfs:label>
    </owl:Class>
    


    <!-- http://purl.org/iot/vocab/m3-lite#ChemicalAgentAtmosphericConcentrationNO -->

    <owl:Class rdf:about="http://purl.org/iot/vocab/m3-lite#ChemicalAgentAtmosphericConcentrationNO">
        <rdfs:subClassOf rdf:resource="http://purl.org/iot/vocab/m3-lite#ChemicalAgentAtmosphericConcentration"/>
        <rdfs:comment xml:lang="en">Measure of the concentration of Carbon Monoxide (CO) gas suspended in the atmosphere.</rdfs:comment>
        <rdfs:label xml:lang="en">Nitrogen Monoxide (NO) Chemical Agent Atmospheric Concentration</rdfs:label>
    </owl:Class>
    


    <!-- http://purl.org/iot/vocab/m3-lite#ChemicalAgentAtmosphericConcentrationNO2 -->

    <owl:Class rdf:about="http://purl.org/iot/vocab/m3-lite#ChemicalAgentAtmosphericConcentrationNO2">
        <rdfs:subClassOf rdf:resource="http://purl.org/iot/vocab/m3-lite#ChemicalAgentAtmosphericConcentration"/>
        <rdfs:comment xml:lang="en">Measure of the concentration of NO2 gas suspended in the atmosphere.</rdfs:comment>
        <rdfs:label xml:lang="en">NO2 Chemical Agent Atmospheric Concentration</rdfs:label>
    </owl:Class>
    


    <!-- http://purl.org/iot/vocab/m3-lite#ChemicalAgentAtmosphericConcentrationO3 -->

    <owl:Class rdf:about="http://purl.org/iot/vocab/m3-lite#ChemicalAgentAtmosphericConcentrationO3">
        <rdfs:subClassOf rdf:resource="http://purl.org/iot/vocab/m3-lite#ChemicalAgentAtmosphericConcentration"/>
        <rdfs:comment xml:lang="en">The concentration of ozone (O3) gas suspended in the atmosphere.</rdfs:comment>
        <rdfs:label xml:lang="en">Chemical Agent Atmospheric Concentration O3</rdfs:label>
    </owl:Class>
    


    <!-- http://purl.org/iot/vocab/m3-lite#ChemicalAgentAtmosphericConcentrationSO2 -->

    <owl:Class rdf:about="http://purl.org/iot/vocab/m3-lite#ChemicalAgentAtmosphericConcentrationSO2">
        <rdfs:subClassOf rdf:resource="http://purl.org/iot/vocab/m3-lite#ChemicalAgentAtmosphericConcentration"/>
        <rdfs:comment xml:lang="en">Measure of the concentration of Sulphur dioxide (SO2) gas suspended in the atmosphere.</rdfs:comment>
        <rdfs:label xml:lang="en">Sulphur dioxide (SO2) Chemical Agent Atmospheric Concentration</rdfs:label>
    </owl:Class>
    


    <!-- http://purl.org/iot/vocab/m3-lite#ChemicalAgentAtmosphericConcentrationVOC -->

    <owl:Class rdf:about="http://purl.org/iot/vocab/m3-lite#ChemicalAgentAtmosphericConcentrationVOC">
        <rdfs:subClassOf rdf:resource="http://purl.org/iot/vocab/m3-lite#ChemicalAgentAtmosphericConcentration"/>
        <rdfs:comment xml:lang="en">Measure of the concentration of Volatile Organic Compound gas suspended in the atmosphere.</rdfs:comment>
        <rdfs:label xml:lang="en">Volatile Organic Compound Chemical Agent Atmospheric Concentration</rdfs:label>
    </owl:Class>
    


    <!-- http://purl.org/iot/vocab/m3-lite#ChemicalAgentConcentration -->

    <owl:Class rdf:about="http://purl.org/iot/vocab/m3-lite#ChemicalAgentConcentration">
        <rdfs:subClassOf rdf:resource="http://purl.org/NET/ssnx/qu/qu#QuantityKind"/>
        <rdfs:comment xml:lang="en">Measure of Chemical Agent Concentration</rdfs:comment>
        <rdfs:label xml:lang="en">Chemical Agent Concentration Quantity Kind</rdfs:label>
    </owl:Class>
    


    <!-- http://purl.org/iot/vocab/m3-lite#ChemicalAgentWaterConcentration -->

    <owl:Class rdf:about="http://purl.org/iot/vocab/m3-lite#ChemicalAgentWaterConcentration">
        <rdfs:subClassOf rdf:resource="http://purl.org/iot/vocab/m3-lite#ChemicalAgentConcentration"/>
        <rdfs:comment xml:lang="en">Measure of Chemical Agent Concentration in Water </rdfs:comment>
        <rdfs:label xml:lang="en">Chemical Agent Water Concentration Quantity Kind</rdfs:label>
    </owl:Class>
    


    <!-- http://purl.org/iot/vocab/m3-lite#ChemicalAgentWaterConcentrationNH4Ion -->

    <owl:Class rdf:about="http://purl.org/iot/vocab/m3-lite#ChemicalAgentWaterConcentrationNH4Ion">
        <rdfs:subClassOf rdf:resource="http://purl.org/iot/vocab/m3-lite#ChemicalAgentWaterConcentration"/>
        <rdfs:comment xml:lang="en">Measure of NH4 ion concentration in Water </rdfs:comment>
        <rdfs:label xml:lang="en">Ammonium ion (NH4+) Chemical Agent Water Concentration</rdfs:label>
    </owl:Class>
    


    <!-- http://purl.org/iot/vocab/m3-lite#ChemicalAgentWaterConcentrationNO3Ion -->

    <owl:Class rdf:about="http://purl.org/iot/vocab/m3-lite#ChemicalAgentWaterConcentrationNO3Ion">
        <rdfs:subClassOf rdf:resource="http://purl.org/iot/vocab/m3-lite#ChemicalAgentWaterConcentration"/>
        <rdfs:comment xml:lang="en">Measure of NO3 ion concentration in Water </rdfs:comment>
        <rdfs:label xml:lang="en">Nitrate Ion (NO3-) Chemical Agent Water Concentration</rdfs:label>
    </owl:Class>
    


    <!-- http://purl.org/iot/vocab/m3-lite#ChemicalAgentWaterConcentrationO2 -->

    <owl:Class rdf:about="http://purl.org/iot/vocab/m3-lite#ChemicalAgentWaterConcentrationO2">
        <rdfs:subClassOf rdf:resource="http://purl.org/iot/vocab/m3-lite#ChemicalAgentWaterConcentration"/>
        <rdfs:comment xml:lang="en">Measure of O2 concentration in Water </rdfs:comment>
        <rdfs:label xml:lang="en">Oxygen (O2) Chemical Agent Water Concentration</rdfs:label>
    </owl:Class>
    


    <!-- http://purl.org/iot/vocab/m3-lite#Cholesterol -->

    <owl:Class rdf:about="http://purl.org/iot/vocab/m3-lite#Cholesterol">
        <rdfs:subClassOf rdf:resource="http://purl.org/NET/ssnx/qu/qu#QuantityKind"/>
        <rdfs:comment xml:lang="en">Measure of the cholesterol level in a system.</rdfs:comment>
        <rdfs:label xml:lang="en">Cholesterol Quantity Kind</rdfs:label>
    </owl:Class>
    


    <!-- http://purl.org/iot/vocab/m3-lite#CholesterolSensor -->

    <owl:Class rdf:about="http://purl.org/iot/vocab/m3-lite#CholesterolSensor">
        <rdfs:subClassOf rdf:resource="http://purl.oclc.org/NET/ssnx/ssn#SensingDevice"/>
        <rdfs:subClassOf>
            <owl:Restriction>
                <owl:onProperty rdf:resource="http://purl.org/iot/vocab/m3-lite#hasDomainOfInterest"/>
                <owl:someValuesFrom rdf:resource="http://purl.org/iot/vocab/m3-lite#Health"/>
            </owl:Restriction>
        </rdfs:subClassOf>
        <rdfs:comment xml:lang="en">Device used to measure the cholesterol level in a system.</rdfs:comment>
        <rdfs:label xml:lang="en">Cholesterol Sensor</rdfs:label>
    </owl:Class>
    


    <!-- http://purl.org/iot/vocab/m3-lite#City -->

    <owl:Class rdf:about="http://purl.org/iot/vocab/m3-lite#City">
        <rdfs:subClassOf rdf:resource="http://purl.org/iot/vocab/m3-lite#DomainOfInterest"/>
        <rdfs:comment xml:lang="en">Smart City as an Internet of Things (IoT) applicative domain.</rdfs:comment>
        <rdfs:label xml:lang="en">Smart City DOI</rdfs:label>
    </owl:Class>
    


    <!-- http://purl.org/iot/vocab/m3-lite#Clock -->

    <owl:Class rdf:about="http://purl.org/iot/vocab/m3-lite#Clock">
        <rdfs:subClassOf rdf:resource="http://purl.oclc.org/NET/ssnx/ssn#SensingDevice"/>
        <rdfs:comment xml:lang="en">sensor that measures time</rdfs:comment>
        <rdfs:label xml:lang="en">Clock</rdfs:label>
    </owl:Class>
    


    <!-- http://purl.org/iot/vocab/m3-lite#CloudCover -->

    <owl:Class rdf:about="http://purl.org/iot/vocab/m3-lite#CloudCover">
        <rdfs:subClassOf rdf:resource="http://purl.org/NET/ssnx/qu/qu#QuantityKind"/>
        <rdfs:comment xml:lang="en">Measure of cloud cover at a certain time. </rdfs:comment>
        <rdfs:label xml:lang="en">Cloud Cover Quantity Kind</rdfs:label>
    </owl:Class>
    


    <!-- http://purl.org/iot/vocab/m3-lite#CloudCoverSensor -->

    <owl:Class rdf:about="http://purl.org/iot/vocab/m3-lite#CloudCoverSensor">
        <rdfs:subClassOf rdf:resource="http://purl.oclc.org/NET/ssnx/ssn#SensingDevice"/>
        <rdfs:subClassOf>
            <owl:Restriction>
                <owl:onProperty rdf:resource="http://purl.org/iot/vocab/m3-lite#hasDomainOfInterest"/>
                <owl:someValuesFrom rdf:resource="http://purl.org/iot/vocab/m3-lite#Weather"/>
            </owl:Restriction>
        </rdfs:subClassOf>
        <rdfs:comment xml:lang="en">Cloud Cover Sensor is used to detect whether it is sunny, cloudy, etc.</rdfs:comment>
        <rdfs:label xml:lang="en">Cloud Cover Sensor</rdfs:label>
    </owl:Class>
    


    <!-- http://purl.org/iot/vocab/m3-lite#CoffeeMachine -->

    <owl:Class rdf:about="http://purl.org/iot/vocab/m3-lite#CoffeeMachine">
        <rdfs:subClassOf rdf:resource="http://purl.oclc.org/NET/UNIS/fiware/iot-lite#ActuatingDevice"/>
        <rdfs:subClassOf>
            <owl:Restriction>
                <owl:onProperty rdf:resource="http://purl.org/iot/vocab/m3-lite#hasDomainOfInterest"/>
                <owl:someValuesFrom rdf:resource="http://purl.org/iot/vocab/m3-lite#BuildingAutomation"/>
            </owl:Restriction>
        </rdfs:subClassOf>
        <rdfs:comment xml:lang="en">An actuator to automatically switch on/off the coffee machine.</rdfs:comment>
        <rdfs:label xml:lang="en">Coffee Machine, Coffee Maker Actuating Device</rdfs:label>
    </owl:Class>
    


    <!-- http://purl.org/iot/vocab/m3-lite#Communication -->

    <owl:Class rdf:about="http://purl.org/iot/vocab/m3-lite#Communication">
        <rdfs:subClassOf rdf:resource="http://purl.org/NET/ssnx/qu/qu#QuantityKind"/>
        <rdfs:comment xml:lang="en">Communication related properties.</rdfs:comment>
        <rdfs:label xml:lang="en">Communication Properties</rdfs:label>
    </owl:Class>
    


    <!-- http://purl.org/iot/vocab/m3-lite#Computer -->

    <owl:Class rdf:about="http://purl.org/iot/vocab/m3-lite#Computer">
        <rdfs:subClassOf rdf:resource="http://purl.oclc.org/NET/UNIS/fiware/iot-lite#ActuatingDevice"/>
        <rdfs:comment xml:lang="en">Actuating devices for Computer or PC.</rdfs:comment>
        <rdfs:label xml:lang="en">Computer, PC Actuating Device</rdfs:label>
    </owl:Class>
    


    <!-- http://purl.org/iot/vocab/m3-lite#Conductivity -->

    <owl:Class rdf:about="http://purl.org/iot/vocab/m3-lite#Conductivity">
        <rdfs:subClassOf rdf:resource="http://purl.org/NET/ssnx/qu/qu#QuantityKind"/>
        <rdfs:comment xml:lang="en">Measure of ability to conduct electricity. It is measured in siemens per metre (S/m).</rdfs:comment>
        <rdfs:label xml:lang="en">Conductivity</rdfs:label>
    </owl:Class>
    


    <!-- http://purl.org/iot/vocab/m3-lite#ConductivitySensor -->

    <owl:Class rdf:about="http://purl.org/iot/vocab/m3-lite#ConductivitySensor">
        <rdfs:subClassOf rdf:resource="http://purl.oclc.org/NET/ssnx/ssn#SensingDevice"/>
        <rdfs:comment xml:lang="en">Device used to measure the conductivity of a system.</rdfs:comment>
        <rdfs:label xml:lang="en">Conductivity Sensor</rdfs:label>
    </owl:Class>
    


    <!-- http://purl.org/iot/vocab/m3-lite#ConstructionWork -->

    <owl:Class rdf:about="http://purl.org/iot/vocab/m3-lite#ConstructionWork">
        <rdfs:subClassOf rdf:resource="http://purl.org/iot/vocab/m3-lite#SoundSource"/>
        <rdfs:comment xml:lang="en">When the source of the sound was a construction work.</rdfs:comment>
        <rdfs:label xml:lang="en">Construction Work Sound Source</rdfs:label>
    </owl:Class>
    


    <!-- http://purl.org/iot/vocab/m3-lite#Coordinates -->

    <owl:Class rdf:about="http://purl.org/iot/vocab/m3-lite#Coordinates">
        <rdfs:subClassOf rdf:resource="http://purl.org/NET/ssnx/qu/qu#Unit"/>
        <rdfs:comment xml:lang="en">Triples for location in the (Latitude, Longitude, Altitude) format.</rdfs:comment>
        <rdfs:label xml:lang="en">Coordinates</rdfs:label>
    </owl:Class>
    


    <!-- http://purl.org/iot/vocab/m3-lite#Coulomb -->

    <owl:Class rdf:about="http://purl.org/iot/vocab/m3-lite#Coulomb">
        <rdfs:subClassOf rdf:resource="http://purl.org/NET/ssnx/qu/qu#Unit"/>
        <rdfs:comment xml:lang="en">SI unit of electric charge.</rdfs:comment>
        <rdfs:label xml:lang="en">Coulomb</rdfs:label>
        <rdfs:seeAlso rdf:resource="http://sweet.jpl.nasa.gov/ontology/units.owl#coulomb"/>
    </owl:Class>
    


    <!-- http://purl.org/iot/vocab/m3-lite#Count -->

    <owl:Class rdf:about="http://purl.org/iot/vocab/m3-lite#Count">
        <rdfs:subClassOf rdf:resource="http://purl.org/NET/ssnx/qu/qu#QuantityKind"/>
        <rdfs:comment xml:lang="en">Number of available particular things.</rdfs:comment>
        <rdfs:label xml:lang="en">Count</rdfs:label>
    </owl:Class>
    


    <!-- http://purl.org/iot/vocab/m3-lite#CountAvailableBicycles -->

    <owl:Class rdf:about="http://purl.org/iot/vocab/m3-lite#CountAvailableBicycles">
        <rdfs:subClassOf rdf:resource="http://purl.org/iot/vocab/m3-lite#Count"/>
        <rdfs:comment xml:lang="en">Number of available bicycles at a particular bicycle docking station.</rdfs:comment>
        <rdfs:label xml:lang="en">Count Available Bicycles</rdfs:label>
    </owl:Class>
    


    <!-- http://purl.org/iot/vocab/m3-lite#CountAvailableTaxis -->

    <owl:Class rdf:about="http://purl.org/iot/vocab/m3-lite#CountAvailableTaxis">
        <rdfs:subClassOf rdf:resource="http://purl.org/iot/vocab/m3-lite#Count"/>
        <rdfs:comment xml:lang="en">Number of taxis available at a particular taxi stop.</rdfs:comment>
        <rdfs:label xml:lang="en">Count Available Taxis</rdfs:label>
    </owl:Class>
    


    <!-- http://purl.org/iot/vocab/m3-lite#CountEmptyDockingPoints -->

    <owl:Class rdf:about="http://purl.org/iot/vocab/m3-lite#CountEmptyDockingPoints">
        <rdfs:subClassOf rdf:resource="http://purl.org/iot/vocab/m3-lite#Count"/>
        <rdfs:comment xml:lang="en">Number of empty docking points at a particular bicycle docking station.</rdfs:comment>
        <rdfs:label xml:lang="en">Count Empty Docking Points</rdfs:label>
    </owl:Class>
    


    <!-- http://purl.org/iot/vocab/m3-lite#Counter -->

    <owl:Class rdf:about="http://purl.org/iot/vocab/m3-lite#Counter">
        <rdfs:subClassOf rdf:resource="http://purl.oclc.org/NET/ssnx/ssn#SensingDevice"/>
        <rdfs:comment xml:lang="en">Sensors that reckons occurrences or repetitions of physical objects, phenomena or events.</rdfs:comment>
        <rdfs:label xml:lang="en">Counter</rdfs:label>
    </owl:Class>
    


    <!-- http://purl.org/iot/vocab/m3-lite#Crowd -->

    <owl:Class rdf:about="http://purl.org/iot/vocab/m3-lite#Crowd">
        <rdfs:subClassOf rdf:resource="http://purl.org/iot/vocab/m3-lite#SoundSource"/>
        <rdfs:comment xml:lang="en">When the source of the sound was crowd.</rdfs:comment>
        <rdfs:label xml:lang="en">Crowd Sound Source</rdfs:label>
    </owl:Class>
    


    <!-- http://purl.org/iot/vocab/m3-lite#Cupboard -->

    <owl:Class rdf:about="http://purl.org/iot/vocab/m3-lite#Cupboard">
        <rdfs:subClassOf rdf:resource="http://purl.oclc.org/NET/UNIS/fiware/iot-lite#ActuatingDevice"/>
        <rdfs:subClassOf>
            <owl:Restriction>
                <owl:onProperty rdf:resource="http://purl.org/iot/vocab/m3-lite#hasDomainOfInterest"/>
                <owl:someValuesFrom rdf:resource="http://purl.org/iot/vocab/m3-lite#BuildingAutomation"/>
            </owl:Restriction>
        </rdfs:subClassOf>
        <rdfs:comment xml:lang="en">An actuator to automatically open/close the cupboard.</rdfs:comment>
        <rdfs:label xml:lang="en">Cupboard Actuating Device</rdfs:label>
    </owl:Class>
    


    <!-- http://purl.org/iot/vocab/m3-lite#Curtain -->

    <owl:Class rdf:about="http://purl.org/iot/vocab/m3-lite#Curtain">
        <rdfs:subClassOf rdf:resource="http://purl.oclc.org/NET/UNIS/fiware/iot-lite#ActuatingDevice"/>
        <rdfs:subClassOf>
            <owl:Restriction>
                <owl:onProperty rdf:resource="http://purl.org/iot/vocab/m3-lite#hasDomainOfInterest"/>
                <owl:someValuesFrom rdf:resource="http://purl.org/iot/vocab/m3-lite#BuildingAutomation"/>
            </owl:Restriction>
        </rdfs:subClassOf>
        <rdfs:comment xml:lang="en">An actuator to automatically open/close the curtain.</rdfs:comment>
        <rdfs:label xml:lang="en">Curtain Actuating Device</rdfs:label>
    </owl:Class>
    


    <!-- http://purl.org/iot/vocab/m3-lite#Day -->

    <owl:Class rdf:about="http://purl.org/iot/vocab/m3-lite#Day">
        <rdfs:subClassOf rdf:resource="http://purl.org/iot/vocab/m3-lite#SecondTime"/>
        <rdfs:comment xml:lang="en">Day is a unit of time.</rdfs:comment>
        <rdfs:label xml:lang="en">Day</rdfs:label>
    </owl:Class>
    


    <!-- http://purl.org/iot/vocab/m3-lite#Decibel -->

    <owl:Class rdf:about="http://purl.org/iot/vocab/m3-lite#Decibel">
        <rdfs:subClassOf rdf:resource="http://purl.org/NET/ssnx/qu/qu#Unit"/>
        <rdfs:comment xml:lang="en">Decibel is a logarithmic unit used to express the ratio of two values of a physical quantity. It is often used to measure sound level.</rdfs:comment>
        <rdfs:label xml:lang="en">Decibel (dB)</rdfs:label>
        <rdfs:seeAlso>http://purl.oclc.org/NET/ssnx/qu/unit#decibel</rdfs:seeAlso>
    </owl:Class>
    


    <!-- http://purl.org/iot/vocab/m3-lite#DecibelA -->

    <owl:Class rdf:about="http://purl.org/iot/vocab/m3-lite#DecibelA">
        <rdfs:subClassOf rdf:resource="http://purl.org/iot/vocab/m3-lite#Decibel"/>
        <rdfs:comment xml:lang="en">Sound pressure sensed by the human ear.</rdfs:comment>
        <rdfs:label xml:lang="en">DecibelA (dB(A))</rdfs:label>
    </owl:Class>
    


    <!-- http://purl.org/iot/vocab/m3-lite#DecibelMilliwatt -->

    <owl:Class rdf:about="http://purl.org/iot/vocab/m3-lite#DecibelMilliwatt">
        <rdfs:subClassOf rdf:resource="http://purl.org/iot/vocab/m3-lite#Decibel"/>
        <rdfs:comment xml:lang="en">It describes power ratio in decibels of the measured power referenced to one milliwatt.</rdfs:comment>
        <rdfs:label xml:lang="en">Decibel Milliwatt</rdfs:label>
    </owl:Class>
    


    <!-- http://purl.org/iot/vocab/m3-lite#Degree -->

    <owl:Class rdf:about="http://purl.org/iot/vocab/m3-lite#Degree">
        <rdfs:subClassOf rdf:resource="http://purl.org/NET/ssnx/qu/qu#Unit"/>
        <rdfs:comment xml:lang="en">Degree</rdfs:comment>
        <rdfs:label xml:lang="en">Degree</rdfs:label>
    </owl:Class>
    


    <!-- http://purl.org/iot/vocab/m3-lite#DegreeAngle -->

    <owl:Class rdf:about="http://purl.org/iot/vocab/m3-lite#DegreeAngle">
        <rdfs:subClassOf rdf:resource="http://purl.org/iot/vocab/m3-lite#Degree"/>
        <rdfs:comment xml:lang="en">A plane angle unit which is equal to 1/360 of a full rotation or pi/180 rad.</rdfs:comment>
        <rdfs:label xml:lang="en">Degree Angle</rdfs:label>
        <rdfs:seeAlso>http://qudt.org/vocab/unit#DegreeAngle</rdfs:seeAlso>
    </owl:Class>
    


    <!-- http://purl.org/iot/vocab/m3-lite#DegreeCelsius -->

    <owl:Class rdf:about="http://purl.org/iot/vocab/m3-lite#DegreeCelsius">
        <rdfs:subClassOf rdf:resource="http://purl.org/iot/vocab/m3-lite#Degree"/>
        <rdfs:comment xml:lang="en">A temperature unit which is equal to one kelvin degree. However, they have their zeros at different points. The centigrade scale has its zero at 273.15 K.</rdfs:comment>
        <rdfs:label xml:lang="en">Degree Celsius</rdfs:label>
        <rdfs:seeAlso rdf:resource="http://data.qudt.org/qudt/owl/1.0.0/unit.owl#DegreeCelsius"/>
        <rdfs:seeAlso rdf:resource="http://sweet.jpl.nasa.gov/ontology/units.owl#degreeC"/>
        <rdfs:seeAlso>http://purl.oclc.org/NET/ssnx/qu/unit#degreeCelsius</rdfs:seeAlso>
    </owl:Class>
    


    <!-- http://purl.org/iot/vocab/m3-lite#DegreeFahrenheit -->

    <owl:Class rdf:about="http://purl.org/iot/vocab/m3-lite#DegreeFahrenheit">
        <rdfs:subClassOf rdf:resource="http://purl.org/iot/vocab/m3-lite#Degree"/>
        <rdfs:comment xml:lang="en">Measurement Unit to represent temperature on the Fahrenheit scale.</rdfs:comment>
        <rdfs:label xml:lang="en">Degree Fahrenheit</rdfs:label>
        <rdfs:seeAlso rdf:resource="http://archive.knoesis.org/research/semsci/application_domain/sem_sensor/ont/weather.owlfahrenheit"/>
        <rdfs:seeAlso rdf:resource="http://sweet.jpl.nasa.gov/ontology/units.owl#degreeF"/>
    </owl:Class>
    


    <!-- http://purl.org/iot/vocab/m3-lite#DeltaDewPoint -->

    <owl:Class rdf:about="http://purl.org/iot/vocab/m3-lite#DeltaDewPoint">
        <rdfs:subClassOf rdf:resource="http://purl.org/iot/vocab/m3-lite#DewPoint"/>
        <rdfs:comment xml:lang="en">Difference between Dewpoint and surface temperatures.</rdfs:comment>
        <rdfs:label xml:lang="en">Delta Dew Point</rdfs:label>
    </owl:Class>
    


    <!-- http://purl.org/iot/vocab/m3-lite#DeltaDewPointSensor -->

    <owl:Class rdf:about="http://purl.org/iot/vocab/m3-lite#DeltaDewPointSensor">
        <rdfs:subClassOf rdf:resource="http://purl.oclc.org/NET/ssnx/ssn#SensingDevice"/>
        <rdfs:comment xml:lang="en">Device that measures the difference between Dewpoint and surface temperatures.</rdfs:comment>
        <rdfs:label xml:lang="en">Delta Dew Point Sensor</rdfs:label>
    </owl:Class>
    


    <!-- http://purl.org/iot/vocab/m3-lite#DeviceUptime -->

    <owl:Class rdf:about="http://purl.org/iot/vocab/m3-lite#DeviceUptime">
        <rdfs:subClassOf rdf:resource="http://purl.org/NET/ssnx/qu/qu#QuantityKind"/>
        <rdfs:comment xml:lang="en">Time a device is working and is available</rdfs:comment>
        <rdfs:label xml:lang="en">Device Uptime</rdfs:label>
    </owl:Class>
    


    <!-- http://purl.org/iot/vocab/m3-lite#DeviceUptimeClock -->

    <owl:Class rdf:about="http://purl.org/iot/vocab/m3-lite#DeviceUptimeClock">
        <rdfs:subClassOf rdf:resource="http://purl.org/iot/vocab/m3-lite#Clock"/>
        <rdfs:comment xml:lang="en">Sensor that measures time a device is working and is available.</rdfs:comment>
        <rdfs:label xml:lang="en">Device Uptime Clock</rdfs:label>
    </owl:Class>
    


    <!-- http://purl.org/iot/vocab/m3-lite#DewPoint -->

    <owl:Class rdf:about="http://purl.org/iot/vocab/m3-lite#DewPoint">
        <rdfs:subClassOf rdf:resource="http://purl.org/NET/ssnx/qu/qu#QuantityKind"/>
        <rdfs:comment xml:lang="en">It is the temperature to which air must be cooled at constant pressure to condense to form liquid.</rdfs:comment>
        <rdfs:label xml:lang="en">Dew Point</rdfs:label>
    </owl:Class>
    


    <!-- http://purl.org/iot/vocab/m3-lite#DewPointSensor -->

    <owl:Class rdf:about="http://purl.org/iot/vocab/m3-lite#DewPointSensor">
        <rdfs:subClassOf rdf:resource="http://purl.oclc.org/NET/ssnx/ssn#SensingDevice"/>
        <rdfs:comment xml:lang="en">Device that measures dew point.</rdfs:comment>
        <rdfs:label xml:lang="en">Dew Point Sensor</rdfs:label>
    </owl:Class>
    


    <!-- http://purl.org/iot/vocab/m3-lite#DewPointTemperature -->

    <owl:Class rdf:about="http://purl.org/iot/vocab/m3-lite#DewPointTemperature">
        <rdfs:subClassOf rdf:resource="http://purl.org/iot/vocab/m3-lite#DewPoint"/>
        <rdfs:comment xml:lang="en">The temperature at which dew forms and is a measure of atmospheric moisture. It is the temperature to which air must be cooled at constant pressure and water content to reach saturation. A higher dew point indicates more moisture in the air; a dew point greater than 20 Degree C (68 Degree F) is considered uncomfortable and greater than 22 Degree C (72 Degree F) is considered to be extremely humid.</rdfs:comment>
        <rdfs:label xml:lang="en">Dew Point Temperature</rdfs:label>
    </owl:Class>
    


    <!-- http://purl.org/iot/vocab/m3-lite#DiastolicBloodPressure -->

    <owl:Class rdf:about="http://purl.org/iot/vocab/m3-lite#DiastolicBloodPressure">
        <rdfs:subClassOf rdf:resource="http://purl.org/iot/vocab/m3-lite#BloodPressure"/>
        <rdfs:comment xml:lang="en"> Measure of the pressure in the arteries when the heart rests between beats.</rdfs:comment>
        <rdfs:label xml:lang="en">Diastolic Blood Pressure</rdfs:label>
    </owl:Class>
    


    <!-- http://purl.org/iot/vocab/m3-lite#Dimensionless -->

    <owl:Class rdf:about="http://purl.org/iot/vocab/m3-lite#Dimensionless">
        <rdfs:subClassOf rdf:resource="http://purl.org/NET/ssnx/qu/qu#Unit"/>
        <rdfs:comment xml:lang="en">Without dimensions; having no appreciable or noteworthy extent. Without physical meaning.</rdfs:comment>
        <rdfs:label xml:lang="en">Dimensionless</rdfs:label>
        <rdfs:seeAlso>http://purl.oclc.org/NET/ssnx/qu/dim#Dimensionless</rdfs:seeAlso>
    </owl:Class>
    


    <!-- http://purl.org/iot/vocab/m3-lite#Direction -->

    <owl:Class rdf:about="http://purl.org/iot/vocab/m3-lite#Direction">
        <rdfs:comment xml:lang="en">Measurements of sensors are affected by the direction of the sensing device. This concept is used to reflect it.</rdfs:comment>
        <rdfs:label xml:lang="en">Direction</rdfs:label>
    </owl:Class>
    


    <!-- http://purl.org/iot/vocab/m3-lite#DirectionAzimuth -->

    <owl:Class rdf:about="http://purl.org/iot/vocab/m3-lite#DirectionAzimuth">
        <rdfs:subClassOf rdf:resource="http://purl.org/iot/vocab/m3-lite#Direction"/>
        <rdfs:comment xml:lang="en">The geodetic azimuth of the direction towards which an object is point to.</rdfs:comment>
        <rdfs:label xml:lang="en">Direction Azimuth</rdfs:label>
    </owl:Class>
    


    <!-- http://purl.org/iot/vocab/m3-lite#DirectionHeading -->

    <owl:Class rdf:about="http://purl.org/iot/vocab/m3-lite#DirectionHeading">
        <rdfs:subClassOf rdf:resource="http://purl.org/iot/vocab/m3-lite#Direction"/>
        <rdfs:comment xml:lang="en">The course or direction in which a object (vehicle, person, ...) is moving.</rdfs:comment>
        <rdfs:label xml:lang="en">Direction Heading</rdfs:label>
    </owl:Class>
    


    <!-- http://purl.org/iot/vocab/m3-lite#DirectionOfArrival -->

    <owl:Class rdf:about="http://purl.org/iot/vocab/m3-lite#DirectionOfArrival">
        <rdfs:subClassOf rdf:resource="http://purl.org/NET/ssnx/qu/qu#QuantityKind"/>
        <rdfs:comment xml:lang="en">The azimuth direction of a  source relative to the azimuth direction of the DOA sensor.</rdfs:comment>
        <rdfs:label xml:lang="en">Direction Of Arrival</rdfs:label>
    </owl:Class>
    


    <!-- http://purl.org/iot/vocab/m3-lite#DirectionOfArrivalSensor -->

    <owl:Class rdf:about="http://purl.org/iot/vocab/m3-lite#DirectionOfArrivalSensor">
        <rdfs:subClassOf rdf:resource="http://purl.oclc.org/NET/ssnx/ssn#SensingDevice"/>
        <rdfs:comment xml:lang="en">Sensor that estimates the azimuth direction of sources relative to the sensors position.</rdfs:comment>
        <rdfs:label xml:lang="en">Direction Of Arrival (DOA) Sensor</rdfs:label>
    </owl:Class>
    


    <!-- http://purl.org/iot/vocab/m3-lite#DishWasher -->

    <owl:Class rdf:about="http://purl.org/iot/vocab/m3-lite#DishWasher">
        <rdfs:subClassOf rdf:resource="http://purl.oclc.org/NET/UNIS/fiware/iot-lite#ActuatingDevice"/>
        <rdfs:subClassOf>
            <owl:Restriction>
                <owl:onProperty rdf:resource="http://purl.org/iot/vocab/m3-lite#hasDomainOfInterest"/>
                <owl:someValuesFrom rdf:resource="http://purl.org/iot/vocab/m3-lite#BuildingAutomation"/>
            </owl:Restriction>
        </rdfs:subClassOf>
        <rdfs:comment xml:lang="en">An actuator to automatically switch on/off the dishwasher.</rdfs:comment>
        <rdfs:label xml:lang="en">Dish Washer Actuating Device</rdfs:label>
    </owl:Class>
    


    <!-- http://purl.org/iot/vocab/m3-lite#Distance -->

    <owl:Class rdf:about="http://purl.org/iot/vocab/m3-lite#Distance">
        <rdfs:subClassOf rdf:resource="http://purl.org/NET/ssnx/qu/qu#QuantityKind"/>
        <rdfs:comment xml:lang="en">Measure of how far apart objects are.</rdfs:comment>
        <rdfs:label xml:lang="en">Distance</rdfs:label>
    </owl:Class>
    


    <!-- http://purl.org/iot/vocab/m3-lite#DistanceSensor -->

    <owl:Class rdf:about="http://purl.org/iot/vocab/m3-lite#DistanceSensor">
        <rdfs:subClassOf rdf:resource="http://purl.oclc.org/NET/ssnx/ssn#SensingDevice"/>
        <rdfs:subClassOf>
            <owl:Restriction>
                <owl:onProperty rdf:resource="http://purl.org/iot/vocab/m3-lite#hasDomainOfInterest"/>
                <owl:someValuesFrom rdf:resource="http://purl.org/iot/vocab/m3-lite#Transportation"/>
            </owl:Restriction>
        </rdfs:subClassOf>
        <rdfs:comment xml:lang="en">Distance Sensor is used to detect distance between two objects for example:  the safety distance with other cars. Distance sensor can be a laser.</rdfs:comment>
        <rdfs:label xml:lang="en">Distance Sensor</rdfs:label>
    </owl:Class>
    


    <!-- http://purl.org/iot/vocab/m3-lite#DomainOfInterest -->

    <owl:Class rdf:about="http://purl.org/iot/vocab/m3-lite#DomainOfInterest">
        <rdfs:comment xml:lang="en">Application Domain for example: health, environment, etc.</rdfs:comment>
        <rdfs:label xml:lang="en">Domain Of Interest</rdfs:label>
    </owl:Class>
    


    <!-- http://purl.org/iot/vocab/m3-lite#Door -->

    <owl:Class rdf:about="http://purl.org/iot/vocab/m3-lite#Door">
        <rdfs:subClassOf rdf:resource="http://purl.oclc.org/NET/UNIS/fiware/iot-lite#ActuatingDevice"/>
        <rdfs:subClassOf>
            <owl:Restriction>
                <owl:onProperty rdf:resource="http://purl.org/iot/vocab/m3-lite#hasDomainOfInterest"/>
                <owl:someValuesFrom rdf:resource="http://purl.org/iot/vocab/m3-lite#BuildingAutomation"/>
            </owl:Restriction>
        </rdfs:subClassOf>
        <rdfs:comment xml:lang="en">An actuator to automatically open/close the door.</rdfs:comment>
        <rdfs:label xml:lang="en">Door Actuating Device</rdfs:label>
    </owl:Class>
    


    <!-- http://purl.org/iot/vocab/m3-lite#DoorStateSensor -->

    <owl:Class rdf:about="http://purl.org/iot/vocab/m3-lite#DoorStateSensor">
        <rdfs:subClassOf rdf:resource="http://purl.oclc.org/NET/ssnx/ssn#SensingDevice"/>
        <rdfs:comment xml:lang="en">This sensor detects if a door is in the state of OPEN or CLOSED.</rdfs:comment>
        <rdfs:label xml:lang="en">Door State Sensor</rdfs:label>
    </owl:Class>
    


    <!-- http://purl.org/iot/vocab/m3-lite#DoorStatus -->

    <owl:Class rdf:about="http://purl.org/iot/vocab/m3-lite#DoorStatus">
        <rdfs:subClassOf rdf:resource="http://purl.org/NET/ssnx/qu/qu#QuantityKind"/>
        <rdfs:comment xml:lang="en">Describes if a door is OPEN or CLOSED.</rdfs:comment>
        <rdfs:label xml:lang="en">Door Status</rdfs:label>
    </owl:Class>
    


    <!-- http://purl.org/iot/vocab/m3-lite#Drawer -->

    <owl:Class rdf:about="http://purl.org/iot/vocab/m3-lite#Drawer">
        <rdfs:subClassOf rdf:resource="http://purl.oclc.org/NET/UNIS/fiware/iot-lite#ActuatingDevice"/>
        <rdfs:subClassOf>
            <owl:Restriction>
                <owl:onProperty rdf:resource="http://purl.org/iot/vocab/m3-lite#hasDomainOfInterest"/>
                <owl:someValuesFrom rdf:resource="http://purl.org/iot/vocab/m3-lite#BuildingAutomation"/>
            </owl:Restriction>
        </rdfs:subClassOf>
        <rdfs:comment xml:lang="en">An actuator to automatically open/close the drawer.</rdfs:comment>
        <rdfs:label xml:lang="en">Drawer Actuating Device</rdfs:label>
    </owl:Class>
    


    <!-- http://purl.org/iot/vocab/m3-lite#DustSensor -->

    <owl:Class rdf:about="http://purl.org/iot/vocab/m3-lite#DustSensor">
        <rdfs:subClassOf rdf:resource="http://purl.oclc.org/NET/ssnx/ssn#SensingDevice"/>
        <rdfs:comment xml:lang="en">A sensing device that measures dust particle concentration.</rdfs:comment>
        <rdfs:label xml:lang="en">Dust Sensor</rdfs:label>
    </owl:Class>
    


    <!-- http://purl.org/iot/vocab/m3-lite#EAQI -->

    <owl:Class rdf:about="http://purl.org/iot/vocab/m3-lite#EAQI">
        <rdfs:subClassOf rdf:resource="http://purl.org/NET/ssnx/qu/qu#Unit"/>
        <rdfs:comment xml:lang="en">Unit to measure Air Quality in European cities.</rdfs:comment>
        <rdfs:label xml:lang="en">European Air Quality Index (EAQI)</rdfs:label>
    </owl:Class>
    


    <!-- http://purl.org/iot/vocab/m3-lite#ECG -->

    <owl:Class rdf:about="http://purl.org/iot/vocab/m3-lite#ECG">
        <rdfs:subClassOf rdf:resource="http://purl.oclc.org/NET/ssnx/ssn#SensingDevice"/>
        <rdfs:subClassOf>
            <owl:Restriction>
                <owl:onProperty rdf:resource="http://purl.org/iot/vocab/m3-lite#hasDomainOfInterest"/>
                <owl:someValuesFrom rdf:resource="http://purl.org/iot/vocab/m3-lite#Emotion"/>
            </owl:Restriction>
        </rdfs:subClassOf>
        <rdfs:subClassOf>
            <owl:Restriction>
                <owl:onProperty rdf:resource="http://purl.org/iot/vocab/m3-lite#hasDomainOfInterest"/>
                <owl:someValuesFrom rdf:resource="http://purl.org/iot/vocab/m3-lite#Health"/>
            </owl:Restriction>
        </rdfs:subClassOf>
        <rdfs:comment xml:lang="en">ECG or EKG (Electrocardiogram) device.</rdfs:comment>
        <rdfs:label xml:lang="en">ECG or EKG (Electrocardiogram)</rdfs:label>
    </owl:Class>
    


    <!-- http://purl.org/iot/vocab/m3-lite#ESP -->

    <owl:Class rdf:about="http://purl.org/iot/vocab/m3-lite#ESP">
        <rdfs:subClassOf rdf:resource="http://purl.oclc.org/NET/UNIS/fiware/iot-lite#ActuatingDevice"/>
        <rdfs:subClassOf>
            <owl:Restriction>
                <owl:onProperty rdf:resource="http://purl.org/iot/vocab/m3-lite#hasDomainOfInterest"/>
                <owl:someValuesFrom rdf:resource="http://purl.org/iot/vocab/m3-lite#Transportation"/>
            </owl:Restriction>
        </rdfs:subClassOf>
        <rdfs:comment xml:lang="en">The actuator for turning ESP on/off.</rdfs:comment>
        <rdfs:label xml:lang="en">ESP (Electronic Stability Program) Actuating device</rdfs:label>
    </owl:Class>
    


    <!-- http://purl.org/iot/vocab/m3-lite#ElectricCharge -->

    <owl:Class rdf:about="http://purl.org/iot/vocab/m3-lite#ElectricCharge">
        <rdfs:subClassOf rdf:resource="http://purl.org/NET/ssnx/qu/qu#QuantityKind"/>
        <rdfs:comment xml:lang="en">It is the physical property of matter that causes it to experience a force when placed in an electromagnetic field. (Source Wikipedia).</rdfs:comment>
        <rdfs:label xml:lang="en">Electric Charge</rdfs:label>
    </owl:Class>
    


    <!-- http://purl.org/iot/vocab/m3-lite#ElectricCurrent -->

    <owl:Class rdf:about="http://purl.org/iot/vocab/m3-lite#ElectricCurrent">
        <rdfs:subClassOf rdf:resource="http://purl.org/NET/ssnx/qu/qu#QuantityKind"/>
        <rdfs:comment xml:lang="en">Electric current is the flow of electric charge. It is a base quantity in the International System of Units. Electric current is electric charge divided by time. Electric Current is the flow (movement) of electric charge. The amount of electric current through some surface, e.g., a section through a copper conductor, is defined as the amount of electric charge flowing through that surface over time.</rdfs:comment>
        <rdfs:label xml:lang="en">Electric Current</rdfs:label>
        <rdfs:seeAlso>http://qudt.org/vocab/quantity#ElectricCurrent</rdfs:seeAlso>
    </owl:Class>
    


    <!-- http://purl.org/iot/vocab/m3-lite#ElectricField -->

    <owl:Class rdf:about="http://purl.org/iot/vocab/m3-lite#ElectricField">
        <rdfs:subClassOf rdf:resource="http://purl.org/NET/ssnx/qu/qu#QuantityKind"/>
        <rdfs:comment xml:lang="en">Electric field is the electric force per unit charge.</rdfs:comment>
        <rdfs:label xml:lang="en">Electric Field</rdfs:label>
        <rdfs:seeAlso>http://qudt.org/vocab/quantity#ElectricField</rdfs:seeAlso>
    </owl:Class>
    


    <!-- http://purl.org/iot/vocab/m3-lite#ElectricField1800MHz -->

    <owl:Class rdf:about="http://purl.org/iot/vocab/m3-lite#ElectricField1800MHz">
        <rdfs:subClassOf rdf:resource="http://purl.org/iot/vocab/m3-lite#ElectricField"/>
        <rdfs:comment xml:lang="en">A field of force associated with a moving electric charge equivalent to an electric field and a magnetic field at right angles to each other and to the direction of propagation. Applied to the 1800 MHz UHF band.</rdfs:comment>
        <rdfs:label xml:lang="en">Electric Field 1800 MHz</rdfs:label>
    </owl:Class>
    


    <!-- http://purl.org/iot/vocab/m3-lite#ElectricField2100MHz -->

    <owl:Class rdf:about="http://purl.org/iot/vocab/m3-lite#ElectricField2100MHz">
        <rdfs:subClassOf rdf:resource="http://purl.org/iot/vocab/m3-lite#ElectricField"/>
        <rdfs:comment xml:lang="en">A field of force associated with a moving electric charge equivalent to an electric field and a magnetic field at right angles to each other and to the direction of propagation. Applied to the 2100 MHz UHF band.</rdfs:comment>
        <rdfs:label xml:lang="en">Electric Field 2100 MHz</rdfs:label>
    </owl:Class>
    


    <!-- http://purl.org/iot/vocab/m3-lite#ElectricField2400MHz -->

    <owl:Class rdf:about="http://purl.org/iot/vocab/m3-lite#ElectricField2400MHz">
        <rdfs:subClassOf rdf:resource="http://purl.org/iot/vocab/m3-lite#ElectricField"/>
        <rdfs:comment xml:lang="en">A field of force associated with a moving electric charge equivalent to an electric field and a magnetic field at right angles to each other and to the direction of propagation. Applied to the 2400 MHz UHF band.</rdfs:comment>
        <rdfs:label xml:lang="en">Electric Field 2400 MHz</rdfs:label>
    </owl:Class>
    


    <!-- http://purl.org/iot/vocab/m3-lite#ElectricField900Mhz -->

    <owl:Class rdf:about="http://purl.org/iot/vocab/m3-lite#ElectricField900Mhz">
        <rdfs:subClassOf rdf:resource="http://purl.org/iot/vocab/m3-lite#ElectricField"/>
        <rdfs:comment xml:lang="en">A field of force associated with a moving electric charge equivalent to an electric field and a magnetic field at right angles to each other and to the direction of propagation. Applied to the 900 MHz UHF band.</rdfs:comment>
        <rdfs:label xml:lang="en">Electric Field 900 MHz</rdfs:label>
    </owl:Class>
    


    <!-- http://purl.org/iot/vocab/m3-lite#ElectricFieldSensor -->

    <owl:Class rdf:about="http://purl.org/iot/vocab/m3-lite#ElectricFieldSensor">
        <rdfs:subClassOf rdf:resource="http://purl.oclc.org/NET/ssnx/ssn#SensingDevice"/>
        <rdfs:comment xml:lang="en">Scientific instrument for measuring electromagnetic fields (EMF). Most of them measure the electromagnetic radiation flux density (DC fields) or the change in an electromagnetic field over time (AC fields).</rdfs:comment>
        <rdfs:label xml:lang="en">Electric Field Sensor</rdfs:label>
    </owl:Class>
    


    <!-- http://purl.org/iot/vocab/m3-lite#ElectricPotential -->

    <owl:Class rdf:about="http://purl.org/iot/vocab/m3-lite#ElectricPotential">
        <rdfs:subClassOf rdf:resource="http://purl.org/NET/ssnx/qu/qu#QuantityKind"/>
        <rdfs:comment xml:lang="en">Electric potential is the potential energy per unit charge associated with static (time-invariant) electric field.</rdfs:comment>
        <rdfs:label xml:lang="en">Electric Potential</rdfs:label>
        <rdfs:seeAlso>http://purl.oclc.org/NET/ssnx/qu/dim#ElectricPotential</rdfs:seeAlso>
    </owl:Class>
    


    <!-- http://purl.org/iot/vocab/m3-lite#ElectricalResistance -->

    <owl:Class rdf:about="http://purl.org/iot/vocab/m3-lite#ElectricalResistance">
        <rdfs:subClassOf rdf:resource="http://purl.org/NET/ssnx/qu/qu#QuantityKind"/>
        <rdfs:comment xml:lang="en">The electrical resistance of an electrical conductor is the opposition to the passage of an electric current through that conductor.</rdfs:comment>
        <rdfs:label xml:lang="en">Electrical Resistance</rdfs:label>
    </owl:Class>
    


    <!-- http://purl.org/iot/vocab/m3-lite#ElectricalSensor -->

    <owl:Class rdf:about="http://purl.org/iot/vocab/m3-lite#ElectricalSensor">
        <rdfs:subClassOf rdf:resource="http://purl.oclc.org/NET/ssnx/ssn#SensingDevice"/>
        <rdfs:comment xml:lang="en">Sensor that measures the changes in electrical or magnetic signals based on an environmental input.</rdfs:comment>
        <rdfs:label xml:lang="en">Electrical Sensor</rdfs:label>
    </owl:Class>
    


    <!-- http://purl.org/iot/vocab/m3-lite#Emotion -->

    <owl:Class rdf:about="http://purl.org/iot/vocab/m3-lite#Emotion">
        <rdfs:subClassOf rdf:resource="http://purl.org/iot/vocab/m3-lite#DomainOfInterest"/>
        <rdfs:comment xml:lang="en">Affective Science, Emotion, Mood, Emotional State, Brain Wave as an Internet of Things (IoT) applicative domain.</rdfs:comment>
        <rdfs:label xml:lang="en">Emotion DOI</rdfs:label>
        <rdfs:seeAlso rdf:resource="http://ns.inria.fr/emoca#Emotion"/>
        <rdfs:seeAlso rdf:resource="http://sensormeasurement.appspot.com/naturopathy#Emotion"/>
    </owl:Class>
    


    <!-- http://purl.org/iot/vocab/m3-lite#Energy -->

    <owl:Class rdf:about="http://purl.org/iot/vocab/m3-lite#Energy">
        <rdfs:subClassOf rdf:resource="http://purl.org/NET/ssnx/qu/qu#QuantityKind"/>
        <rdfs:comment xml:lang="en">Energy is the property that must be transferred to an object in order to perform work on. (Source Wikipedia).</rdfs:comment>
        <rdfs:label xml:lang="en">Energy</rdfs:label>
    </owl:Class>
    


    <!-- http://purl.org/iot/vocab/m3-lite#EnergyDOI -->

    <owl:Class rdf:about="http://purl.org/iot/vocab/m3-lite#EnergyDOI">
        <rdfs:subClassOf rdf:resource="http://purl.org/iot/vocab/m3-lite#DomainOfInterest"/>
        <rdfs:comment xml:lang="en">Energy or Smart Grid as an Internet of Things (IoT) applicative domain.</rdfs:comment>
        <rdfs:label xml:lang="en">Energy DOI</rdfs:label>
    </owl:Class>
    


    <!-- http://purl.org/iot/vocab/m3-lite#EnergyMeter -->

    <owl:Class rdf:about="http://purl.org/iot/vocab/m3-lite#EnergyMeter">
        <rdfs:subClassOf rdf:resource="http://purl.oclc.org/NET/ssnx/ssn#SensingDevice"/>
        <rdfs:subClassOf>
            <owl:Restriction>
                <owl:onProperty rdf:resource="http://purl.org/iot/vocab/m3-lite#hasDomainOfInterest"/>
                <owl:someValuesFrom rdf:resource="http://purl.org/iot/vocab/m3-lite#EnergyDOI"/>
            </owl:Restriction>
        </rdfs:subClassOf>
        <rdfs:comment xml:lang="en">Sensor to measure power or energy consumption.</rdfs:comment>
        <rdfs:label xml:lang="en">Energy Meter</rdfs:label>
    </owl:Class>
    


    <!-- http://purl.org/iot/vocab/m3-lite#Environment -->

    <owl:Class rdf:about="http://purl.org/iot/vocab/m3-lite#Environment">
        <rdfs:subClassOf rdf:resource="http://purl.org/iot/vocab/m3-lite#DomainOfInterest"/>
        <rdfs:comment xml:lang="en">Environment (earthquake, flooding, fire, pollution) as an Internet of Things (IoT) applicative domain.</rdfs:comment>
        <rdfs:label xml:lang="en">Environment DOI</rdfs:label>
    </owl:Class>
    


    <!-- http://purl.org/iot/vocab/m3-lite#Experiment -->

    <owl:Class rdf:about="http://purl.org/iot/vocab/m3-lite#Experiment">
        <rdfs:subClassOf rdf:resource="http://purl.org/iot/vocab/m3-lite#MeasurementType"/>
        <rdfs:comment xml:lang="en">Experiment based measurements.</rdfs:comment>
        <rdfs:label xml:lang="en">Experiment Measurement Type</rdfs:label>
    </owl:Class>
    


    <!-- http://purl.org/iot/vocab/m3-lite#FallDetector -->

    <owl:Class rdf:about="http://purl.org/iot/vocab/m3-lite#FallDetector">
        <rdfs:subClassOf rdf:resource="http://purl.oclc.org/NET/ssnx/ssn#SensingDevice"/>
        <rdfs:subClassOf>
            <owl:Restriction>
                <owl:onProperty rdf:resource="http://purl.org/iot/vocab/m3-lite#hasDomainOfInterest"/>
                <owl:someValuesFrom rdf:resource="http://purl.org/iot/vocab/m3-lite#BuildingAutomation"/>
            </owl:Restriction>
        </rdfs:subClassOf>
        <rdfs:comment xml:lang="en">Device to detect is a person has fallen.</rdfs:comment>
        <rdfs:label xml:lang="en">Fall Detector</rdfs:label>
    </owl:Class>
    


    <!-- http://purl.org/iot/vocab/m3-lite#Fan -->

    <owl:Class rdf:about="http://purl.org/iot/vocab/m3-lite#Fan">
        <rdfs:subClassOf rdf:resource="http://purl.org/iot/vocab/m3-lite#SoundSource"/>
        <rdfs:comment xml:lang="en">When the source of the sound was Fan.</rdfs:comment>
        <rdfs:label xml:lang="en">Fan Sound Source</rdfs:label>
    </owl:Class>
    


    <!-- http://purl.org/iot/vocab/m3-lite#Farad -->

    <owl:Class rdf:about="http://purl.org/iot/vocab/m3-lite#Farad">
        <rdfs:subClassOf rdf:resource="http://purl.org/NET/ssnx/qu/qu#Unit"/>
        <rdfs:comment xml:lang="en">SI unit of electrical capacitance.</rdfs:comment>
        <rdfs:label xml:lang="en">Farad</rdfs:label>
        <rdfs:seeAlso rdf:resource="http://sweet.jpl.nasa.gov/ontology/units.owl#farad"/>
    </owl:Class>
    


    <!-- http://purl.org/iot/vocab/m3-lite#FillLevel -->

    <owl:Class rdf:about="http://purl.org/iot/vocab/m3-lite#FillLevel">
        <rdfs:subClassOf rdf:resource="http://purl.org/NET/ssnx/qu/qu#QuantityKind"/>
        <rdfs:comment xml:lang="en">Property used to determine the level a certain object such as waste bin is filled upto.</rdfs:comment>
        <rdfs:label xml:lang="en">Fill Level</rdfs:label>
    </owl:Class>
    


    <!-- http://purl.org/iot/vocab/m3-lite#FillLevelGasTank -->

    <owl:Class rdf:about="http://purl.org/iot/vocab/m3-lite#FillLevelGasTank">
        <rdfs:subClassOf rdf:resource="http://purl.org/iot/vocab/m3-lite#FillLevel"/>
        <rdfs:comment xml:lang="en">Ratio of volume of combustible exhaust fluid to the total volume of diesel exhaust fluid storage container.</rdfs:comment>
        <rdfs:label xml:lang="en">Fill Level Gas Tank</rdfs:label>
    </owl:Class>
    


    <!-- http://purl.org/iot/vocab/m3-lite#FillLevelGasTank1 -->

    <owl:Class rdf:about="http://purl.org/iot/vocab/m3-lite#FillLevelGasTank1">
        <rdfs:subClassOf rdf:resource="http://purl.org/iot/vocab/m3-lite#FillLevelGasTank"/>
        <rdfs:comment xml:lang="en">Ratio of volume of combustible exhaust fluid to the total volume of diesel exhaust fluid storage container. This is the value for the primary tank of the vehicle.</rdfs:comment>
        <rdfs:label xml:lang="en">Fill Level Gas Tank 1</rdfs:label>
    </owl:Class>
    


    <!-- http://purl.org/iot/vocab/m3-lite#FillLevelGasTank2 -->

    <owl:Class rdf:about="http://purl.org/iot/vocab/m3-lite#FillLevelGasTank2">
        <rdfs:subClassOf rdf:resource="http://purl.org/iot/vocab/m3-lite#FillLevelGasTank"/>
        <rdfs:comment xml:lang="en">Ratio of volume of combustible exhaust fluid to the total volume of diesel exhaust fluid storage container. This is the value for the secondary tank of the vehicle.</rdfs:comment>
        <rdfs:label xml:lang="en">Fill Level Gas Tank 2</rdfs:label>
    </owl:Class>
    


    <!-- http://purl.org/iot/vocab/m3-lite#FillLevelWasteContainer -->

    <owl:Class rdf:about="http://purl.org/iot/vocab/m3-lite#FillLevelWasteContainer">
        <rdfs:subClassOf rdf:resource="http://purl.org/iot/vocab/m3-lite#FillLevel"/>
        <rdfs:comment xml:lang="en">Ratio between the current filleage level and the total capacity of a waste container.</rdfs:comment>
        <rdfs:label xml:lang="en">Fill Level Waste Container</rdfs:label>
    </owl:Class>
    


    <!-- http://purl.org/iot/vocab/m3-lite#FogLamp -->

    <owl:Class rdf:about="http://purl.org/iot/vocab/m3-lite#FogLamp">
        <rdfs:subClassOf rdf:resource="http://purl.oclc.org/NET/UNIS/fiware/iot-lite#ActuatingDevice"/>
        <rdfs:subClassOf>
            <owl:Restriction>
                <owl:onProperty rdf:resource="http://purl.org/iot/vocab/m3-lite#hasDomainOfInterest"/>
                <owl:someValuesFrom rdf:resource="http://purl.org/iot/vocab/m3-lite#Transportation"/>
            </owl:Restriction>
        </rdfs:subClassOf>
        <rdfs:comment xml:lang="en">The actuator for turning on or off the fog lamp.</rdfs:comment>
        <rdfs:label xml:lang="en">Fog Lamp Actuating Device</rdfs:label>
    </owl:Class>
    


    <!-- http://purl.org/iot/vocab/m3-lite#FoodTemperature -->

    <owl:Class rdf:about="http://purl.org/iot/vocab/m3-lite#FoodTemperature">
        <rdfs:subClassOf rdf:resource="http://purl.org/iot/vocab/m3-lite#Temperature"/>
        <rdfs:comment xml:lang="en">Measure of temperature of the food.</rdfs:comment>
        <rdfs:label xml:lang="en">Food Temperature</rdfs:label>
    </owl:Class>
    


    <!-- http://purl.org/iot/vocab/m3-lite#Freezer -->

    <owl:Class rdf:about="http://purl.org/iot/vocab/m3-lite#Freezer">
        <rdfs:subClassOf rdf:resource="http://purl.oclc.org/NET/UNIS/fiware/iot-lite#ActuatingDevice"/>
        <rdfs:subClassOf>
            <owl:Restriction>
                <owl:onProperty rdf:resource="http://purl.org/iot/vocab/m3-lite#hasDomainOfInterest"/>
                <owl:someValuesFrom rdf:resource="http://purl.org/iot/vocab/m3-lite#BuildingAutomation"/>
            </owl:Restriction>
        </rdfs:subClassOf>
        <rdfs:comment xml:lang="en">An actuator to automatically open/close the freezer.</rdfs:comment>
        <rdfs:label xml:lang="en">Freezer, Chiller Actuating Device</rdfs:label>
    </owl:Class>
    


    <!-- http://purl.org/iot/vocab/m3-lite#Frequency -->

    <owl:Class rdf:about="http://purl.org/iot/vocab/m3-lite#Frequency">
        <rdfs:subClassOf rdf:resource="http://purl.org/NET/ssnx/qu/qu#QuantityKind"/>
        <rdfs:comment xml:lang="en">Frequency is the number of occurrences of a repeating event per unit time.</rdfs:comment>
        <rdfs:label xml:lang="en">Frequency</rdfs:label>
    </owl:Class>
    


    <!-- http://purl.org/iot/vocab/m3-lite#FrequencySensor -->

    <owl:Class rdf:about="http://purl.org/iot/vocab/m3-lite#FrequencySensor">
        <rdfs:subClassOf rdf:resource="http://purl.oclc.org/NET/ssnx/ssn#SensingDevice"/>
        <rdfs:comment xml:lang="en">Device used to detect the frequency.</rdfs:comment>
        <rdfs:label xml:lang="en">Frequency Sensor</rdfs:label>
    </owl:Class>
    


    <!-- http://purl.org/iot/vocab/m3-lite#Fridge -->

    <owl:Class rdf:about="http://purl.org/iot/vocab/m3-lite#Fridge">
        <rdfs:subClassOf rdf:resource="http://purl.oclc.org/NET/UNIS/fiware/iot-lite#ActuatingDevice"/>
        <rdfs:subClassOf>
            <owl:Restriction>
                <owl:onProperty rdf:resource="http://purl.org/iot/vocab/m3-lite#hasDomainOfInterest"/>
                <owl:someValuesFrom rdf:resource="http://purl.org/iot/vocab/m3-lite#BuildingAutomation"/>
            </owl:Restriction>
        </rdfs:subClassOf>
        <rdfs:comment xml:lang="en">An actuator to automatically switch on/off the fridge.</rdfs:comment>
        <rdfs:label xml:lang="en">Fridge, Refrigerator Actuating Device</rdfs:label>
    </owl:Class>
    


    <!-- http://purl.org/iot/vocab/m3-lite#FuelConsumption -->

    <owl:Class rdf:about="http://purl.org/iot/vocab/m3-lite#FuelConsumption">
        <rdfs:subClassOf rdf:resource="http://purl.org/NET/ssnx/qu/qu#QuantityKind"/>
        <rdfs:comment xml:lang="en">The amount of fuel a vehicle uses to travel a particular distance at a particular speed.</rdfs:comment>
        <rdfs:label xml:lang="en">Fuel Consumption Quantity Kind</rdfs:label>
    </owl:Class>
    


    <!-- http://purl.org/iot/vocab/m3-lite#FuelConsumptionInstantaneous -->

    <owl:Class rdf:about="http://purl.org/iot/vocab/m3-lite#FuelConsumptionInstantaneous">
        <rdfs:subClassOf rdf:resource="http://purl.org/iot/vocab/m3-lite#FuelConsumption"/>
        <rdfs:comment xml:lang="en">A measure that displays the instantaneous fuel consumption of a vehicle during its operation.</rdfs:comment>
        <rdfs:label xml:lang="en">Fuel Consumption Instantaneous</rdfs:label>
    </owl:Class>
    


    <!-- http://purl.org/iot/vocab/m3-lite#FuelConsumptionTotal -->

    <owl:Class rdf:about="http://purl.org/iot/vocab/m3-lite#FuelConsumptionTotal">
        <rdfs:subClassOf rdf:resource="http://purl.org/iot/vocab/m3-lite#FuelConsumption"/>
        <rdfs:comment xml:lang="en">Accumulated amount of fuel used during vehicle operation.</rdfs:comment>
        <rdfs:label xml:lang="en">Fuel Consumption Total</rdfs:label>
    </owl:Class>
    


    <!-- http://purl.org/iot/vocab/m3-lite#FuelLevel -->

    <owl:Class rdf:about="http://purl.org/iot/vocab/m3-lite#FuelLevel">
        <rdfs:subClassOf rdf:resource="http://purl.oclc.org/NET/ssnx/ssn#SensingDevice"/>
        <rdfs:subClassOf>
            <owl:Restriction>
                <owl:onProperty rdf:resource="http://purl.org/iot/vocab/m3-lite#hasDomainOfInterest"/>
                <owl:someValuesFrom rdf:resource="http://purl.org/iot/vocab/m3-lite#Transportation"/>
            </owl:Restriction>
        </rdfs:subClassOf>
        <rdfs:comment xml:lang="en">Device used to detect fuel level in a system such a car.</rdfs:comment>
        <rdfs:label xml:lang="en">Fuel Level Sensor</rdfs:label>
    </owl:Class>
    


    <!-- http://purl.org/iot/vocab/m3-lite#GPSSensor -->

    <owl:Class rdf:about="http://purl.org/iot/vocab/m3-lite#GPSSensor">
        <rdfs:subClassOf rdf:resource="http://purl.oclc.org/NET/ssnx/ssn#SensingDevice"/>
        <rdfs:comment xml:lang="en">Device that allows an object to localize itself.</rdfs:comment>
        <rdfs:label xml:lang="en">GPS Sensor</rdfs:label>
    </owl:Class>
    


    <!-- http://purl.org/iot/vocab/m3-lite#GasDetector -->

    <owl:Class rdf:about="http://purl.org/iot/vocab/m3-lite#GasDetector">
        <rdfs:subClassOf rdf:resource="http://purl.oclc.org/NET/ssnx/ssn#SensingDevice"/>
        <rdfs:comment xml:lang="en">Device that detects the presence of gases in an area, often as part of a safety system.</rdfs:comment>
        <rdfs:label xml:lang="en">Gas Detector</rdfs:label>
    </owl:Class>
    


    <!-- http://purl.org/iot/vocab/m3-lite#GaseousPollutantSensor -->

    <owl:Class rdf:about="http://purl.org/iot/vocab/m3-lite#GaseousPollutantSensor">
        <rdfs:subClassOf rdf:resource="http://purl.org/iot/vocab/m3-lite#AirPollutantSensor"/>
        <rdfs:comment xml:lang="en">Device used to detect poisonous gaseous in the environment.</rdfs:comment>
        <rdfs:label xml:lang="en">Gaseous Pollutant Sensor</rdfs:label>
    </owl:Class>
    


    <!-- http://purl.org/iot/vocab/m3-lite#Gauss -->

    <owl:Class rdf:about="http://purl.org/iot/vocab/m3-lite#Gauss">
        <rdfs:subClassOf rdf:resource="http://purl.org/NET/ssnx/qu/qu#Unit"/>
        <rdfs:comment xml:lang="en">Gauss is the CGS unit of measurement of magnetic flux density (or magnetic induction) (B) (Source Wikipedia)</rdfs:comment>
        <rdfs:label xml:lang="en">Gauss</rdfs:label>
    </owl:Class>
    


    <!-- http://purl.org/iot/vocab/m3-lite#Glucometer -->

    <owl:Class rdf:about="http://purl.org/iot/vocab/m3-lite#Glucometer">
        <rdfs:subClassOf rdf:resource="http://purl.oclc.org/NET/ssnx/ssn#SensingDevice"/>
        <rdfs:subClassOf>
            <owl:Restriction>
                <owl:onProperty rdf:resource="http://purl.org/iot/vocab/m3-lite#hasDomainOfInterest"/>
                <owl:someValuesFrom rdf:resource="http://purl.org/iot/vocab/m3-lite#Health"/>
            </owl:Restriction>
        </rdfs:subClassOf>
        <rdfs:comment xml:lang="en">Device used to detect glucometer, blood sugar, blood glucose level</rdfs:comment>
        <rdfs:label xml:lang="en">Glucometer Sensor</rdfs:label>
    </owl:Class>
    


    <!-- http://purl.org/iot/vocab/m3-lite#Gram -->

    <owl:Class rdf:about="http://purl.org/iot/vocab/m3-lite#Gram">
        <rdfs:subClassOf rdf:resource="http://purl.org/NET/ssnx/qu/qu#Unit"/>
        <rdfs:comment>It is a metric system unit of mass</rdfs:comment>
        <rdfs:label>Gram (g)</rdfs:label>
    </owl:Class>
    


    <!-- http://purl.org/iot/vocab/m3-lite#GramPerCubicMetre -->

    <owl:Class rdf:about="http://purl.org/iot/vocab/m3-lite#GramPerCubicMetre">
        <rdfs:subClassOf rdf:resource="http://purl.org/NET/ssnx/qu/qu#Unit"/>
        <rdfs:comment xml:lang="en">It is defined by mass in grams divided by volume in cubic metres.</rdfs:comment>
        <rdfs:label xml:lang="en">Gram Per Cubic Metre, Gram Per Cubic Meter</rdfs:label>
    </owl:Class>
    


    <!-- http://purl.org/iot/vocab/m3-lite#GramPerLitre -->

    <owl:Class rdf:about="http://purl.org/iot/vocab/m3-lite#GramPerLitre">
        <rdfs:subClassOf rdf:resource="http://purl.org/NET/ssnx/qu/qu#Unit"/>
        <rdfs:comment xml:lang="en">It shows how many grams of a certain substance are present in one litre of a usually liquid or gaseous mixture.</rdfs:comment>
        <rdfs:label xml:lang="en">Gram Per Litre, Gram Per Liter (g/L)</rdfs:label>
    </owl:Class>
    


    <!-- http://purl.org/iot/vocab/m3-lite#GyrometerSensor -->

    <owl:Class rdf:about="http://purl.org/iot/vocab/m3-lite#GyrometerSensor">
        <rdfs:subClassOf rdf:resource="http://purl.oclc.org/NET/ssnx/ssn#SensingDevice"/>
        <rdfs:subClassOf>
            <owl:Restriction>
                <owl:onProperty rdf:resource="http://purl.org/iot/vocab/m3-lite#hasDomainOfInterest"/>
                <owl:someValuesFrom rdf:resource="http://purl.org/iot/vocab/m3-lite#Transportation"/>
            </owl:Restriction>
        </rdfs:subClassOf>
        <rdfs:comment xml:lang="en">A gyrometer is an instrument which measures an angular speed.</rdfs:comment>
        <rdfs:label xml:lang="en">Gyrometer Sensor</rdfs:label>
    </owl:Class>
    


    <!-- http://purl.org/iot/vocab/m3-lite#GyroscopeSensor -->

    <owl:Class rdf:about="http://purl.org/iot/vocab/m3-lite#GyroscopeSensor">
        <rdfs:subClassOf rdf:resource="http://purl.oclc.org/NET/ssnx/ssn#SensingDevice"/>
        <rdfs:subClassOf>
            <owl:Restriction>
                <owl:onProperty rdf:resource="http://purl.org/iot/vocab/m3-lite#hasDomainOfInterest"/>
                <owl:someValuesFrom rdf:resource="http://purl.org/iot/vocab/m3-lite#BuildingAutomation"/>
            </owl:Restriction>
        </rdfs:subClassOf>
        <rdfs:subClassOf>
            <owl:Restriction>
                <owl:onProperty rdf:resource="http://purl.org/iot/vocab/m3-lite#hasDomainOfInterest"/>
                <owl:someValuesFrom rdf:resource="http://purl.org/iot/vocab/m3-lite#Transportation"/>
            </owl:Restriction>
        </rdfs:subClassOf>
        <rdfs:comment xml:lang="en">A gyroscope is a device for measuring or maintaining orientation.</rdfs:comment>
        <rdfs:label xml:lang="en">Gyroscope Sensor</rdfs:label>
        <rdfs:seeAlso rdf:resource="http://casas.wsu.edu/owl/cose.owl#Gyroscope"/>
    </owl:Class>
    


    <!-- http://purl.org/iot/vocab/m3-lite#H2SSensor -->

    <owl:Class rdf:about="http://purl.org/iot/vocab/m3-lite#H2SSensor">
        <rdfs:subClassOf rdf:resource="http://purl.org/iot/vocab/m3-lite#GaseousPollutantSensor"/>
        <rdfs:comment xml:lang="en">Device used to measure of hydrogen sulphide in the environment.</rdfs:comment>
        <rdfs:label xml:lang="en">H2S Sensor</rdfs:label>
    </owl:Class>
    


    <!-- http://purl.org/iot/vocab/m3-lite#Health -->

    <owl:Class rdf:about="http://purl.org/iot/vocab/m3-lite#Health">
        <rdfs:subClassOf rdf:resource="http://purl.org/iot/vocab/m3-lite#DomainOfInterest"/>
        <rdfs:comment xml:lang="en">Healthcare as an Internet of Things (IoT) applicative domain.</rdfs:comment>
        <rdfs:label xml:lang="en">Health Care DOI</rdfs:label>
    </owl:Class>
    


    <!-- http://purl.org/iot/vocab/m3-lite#HeartBeat -->

    <owl:Class rdf:about="http://purl.org/iot/vocab/m3-lite#HeartBeat">
        <rdfs:subClassOf rdf:resource="http://purl.org/NET/ssnx/qu/qu#QuantityKind"/>
        <rdfs:comment xml:lang="en">The number of times your heart beats each minute (bpm).</rdfs:comment>
        <rdfs:label xml:lang="en">Heart Beat</rdfs:label>
    </owl:Class>
    


    <!-- http://purl.org/iot/vocab/m3-lite#HeartBeatSensor -->

    <owl:Class rdf:about="http://purl.org/iot/vocab/m3-lite#HeartBeatSensor">
        <rdfs:subClassOf rdf:resource="http://purl.oclc.org/NET/ssnx/ssn#SensingDevice"/>
        <rdfs:subClassOf>
            <owl:Restriction>
                <owl:onProperty rdf:resource="http://purl.org/iot/vocab/m3-lite#hasDomainOfInterest"/>
                <owl:someValuesFrom rdf:resource="http://purl.org/iot/vocab/m3-lite#Health"/>
            </owl:Restriction>
        </rdfs:subClassOf>
        <rdfs:comment xml:lang="en">Device to count heart beats per minute.</rdfs:comment>
        <rdfs:label xml:lang="en">Heart Beat Sensor</rdfs:label>
    </owl:Class>
    


    <!-- http://purl.org/iot/vocab/m3-lite#Heating -->

    <owl:Class rdf:about="http://purl.org/iot/vocab/m3-lite#Heating">
        <rdfs:subClassOf rdf:resource="http://purl.oclc.org/NET/UNIS/fiware/iot-lite#ActuatingDevice"/>
        <rdfs:subClassOf>
            <owl:Restriction>
                <owl:onProperty rdf:resource="http://purl.org/iot/vocab/m3-lite#hasDomainOfInterest"/>
                <owl:someValuesFrom rdf:resource="http://purl.org/iot/vocab/m3-lite#BuildingAutomation"/>
            </owl:Restriction>
        </rdfs:subClassOf>
        <rdfs:comment xml:lang="en">An actuator to automatically switch on/off the heating.</rdfs:comment>
        <rdfs:label xml:lang="en">Heating Actuating Device</rdfs:label>
    </owl:Class>
    


    <!-- http://purl.org/iot/vocab/m3-lite#Hertz -->

    <owl:Class rdf:about="http://purl.org/iot/vocab/m3-lite#Hertz">
        <rdfs:subClassOf rdf:resource="http://purl.org/NET/ssnx/qu/qu#Unit"/>
        <rdfs:comment xml:lang="en">The SI unit of frequency, equal to one cycle per second.</rdfs:comment>
        <rdfs:label xml:lang="en">Hertz</rdfs:label>
    </owl:Class>
    


    <!-- http://purl.org/iot/vocab/m3-lite#Hour -->

    <owl:Class rdf:about="http://purl.org/iot/vocab/m3-lite#Hour">
        <rdfs:subClassOf rdf:resource="http://purl.org/iot/vocab/m3-lite#SecondTime"/>
        <rdfs:comment xml:lang="en">Hour of the day.</rdfs:comment>
        <rdfs:label xml:lang="en">Hour</rdfs:label>
        <rdfs:seeAlso rdf:resource="http://sweet.jpl.nasa.gov/ontology/units.owl#hour"/>
    </owl:Class>
    


    <!-- http://purl.org/iot/vocab/m3-lite#HouseholdApplianceTemperature -->

    <owl:Class rdf:about="http://purl.org/iot/vocab/m3-lite#HouseholdApplianceTemperature">
        <rdfs:subClassOf rdf:resource="http://purl.org/iot/vocab/m3-lite#Temperature"/>
        <rdfs:comment xml:lang="en">Measure of Household Appliance Temperature.</rdfs:comment>
        <rdfs:label xml:lang="en">Household Appliance Temperature</rdfs:label>
    </owl:Class>
    


    <!-- http://purl.org/iot/vocab/m3-lite#HumanPresenceDetector -->

    <owl:Class rdf:about="http://purl.org/iot/vocab/m3-lite#HumanPresenceDetector">
        <rdfs:subClassOf rdf:resource="http://purl.org/iot/vocab/m3-lite#PresenceDetector"/>
        <rdfs:comment xml:lang="en">Device used to detect if an object (vehicle, room, place, etc.) is occupied by Human.</rdfs:comment>
        <rdfs:label xml:lang="en"> Human Presence Detector</rdfs:label>
    </owl:Class>
    


    <!-- http://purl.org/iot/vocab/m3-lite#Humidity -->

    <owl:Class rdf:about="http://purl.org/iot/vocab/m3-lite#Humidity">
        <rdfs:subClassOf rdf:resource="http://purl.org/NET/ssnx/qu/qu#QuantityKind"/>
        <rdfs:comment xml:lang="en">A quantity representing the amount of water vapour in the atmosphere or in a gas.</rdfs:comment>
        <rdfs:label xml:lang="en">Humidity</rdfs:label>
        <rdfs:seeAlso rdf:resource="http://elite.polito.it/ontologies/dogont.owl#HumidityMeasurementMNotification"/>
        <rdfs:seeAlso rdf:resource="http://openiot.eu/ontology/ns/AtmosphereHumidity"/>
        <rdfs:seeAlso rdf:resource="http://paul.staroch.name/thesis/SmartHomeWeather.owl#Humidity"/>
    </owl:Class>
    


    <!-- http://purl.org/iot/vocab/m3-lite#HumiditySensor -->

    <owl:Class rdf:about="http://purl.org/iot/vocab/m3-lite#HumiditySensor">
        <rdfs:subClassOf rdf:resource="http://purl.oclc.org/NET/ssnx/ssn#SensingDevice"/>
        <rdfs:subClassOf>
            <owl:Restriction>
                <owl:onProperty rdf:resource="http://purl.org/iot/vocab/m3-lite#hasDomainOfInterest"/>
                <owl:someValuesFrom rdf:resource="http://purl.org/iot/vocab/m3-lite#Agriculture"/>
            </owl:Restriction>
        </rdfs:subClassOf>
        <rdfs:subClassOf>
            <owl:Restriction>
                <owl:onProperty rdf:resource="http://purl.org/iot/vocab/m3-lite#hasDomainOfInterest"/>
                <owl:someValuesFrom rdf:resource="http://purl.org/iot/vocab/m3-lite#Environment"/>
            </owl:Restriction>
        </rdfs:subClassOf>
        <rdfs:subClassOf>
            <owl:Restriction>
                <owl:onProperty rdf:resource="http://purl.org/iot/vocab/m3-lite#hasDomainOfInterest"/>
                <owl:someValuesFrom rdf:resource="http://purl.org/iot/vocab/m3-lite#Weather"/>
            </owl:Restriction>
        </rdfs:subClassOf>
        <rdfs:comment xml:lang="en">Humidity sensor or hygrometer is an instrument used for measuring the moisture concent in the environment.</rdfs:comment>
        <rdfs:label xml:lang="en">Humidity Sensor</rdfs:label>
        <rdfs:seeAlso rdf:resource="http://purl.oclc.org/NET/ssnx/meteo/aws#HumiditySensor"/>
    </owl:Class>
    


    <!-- http://purl.org/iot/vocab/m3-lite#Hydrophone -->

    <owl:Class rdf:about="http://purl.org/iot/vocab/m3-lite#Hydrophone">
        <rdfs:subClassOf rdf:resource="http://purl.oclc.org/NET/ssnx/ssn#SensingDevice"/>
        <rdfs:comment xml:lang="en">A hydrophone is a microphone designed to be used underwater for recording or listening to underwater sound.</rdfs:comment>
        <rdfs:label xml:lang="en">Hydrophone</rdfs:label>
    </owl:Class>
    


    <!-- http://purl.org/iot/vocab/m3-lite#IEEE802154InterfaceEnergyMeter -->

    <owl:Class rdf:about="http://purl.org/iot/vocab/m3-lite#IEEE802154InterfaceEnergyMeter">
        <rdfs:subClassOf rdf:resource="http://purl.org/iot/vocab/m3-lite#EnergyMeter"/>
        <rdfs:comment xml:lang="en">Sensor that measures the power consumption of the IEEE802.15.4 interface nodes.</rdfs:comment>
        <rdfs:label xml:lang="en">IEEE802.15.4 Interface Energy Meter</rdfs:label>
    </owl:Class>
    


    <!-- http://purl.org/iot/vocab/m3-lite#Illuminance -->

    <owl:Class rdf:about="http://purl.org/iot/vocab/m3-lite#Illuminance">
        <rdfs:subClassOf rdf:resource="http://purl.org/NET/ssnx/qu/qu#QuantityKind"/>
        <rdfs:comment xml:lang="en">Illuminance is the total luminous flux incident on a surface, per unit area.</rdfs:comment>
        <rdfs:label xml:lang="en">Illuminance</rdfs:label>
    </owl:Class>
    


    <!-- http://purl.org/iot/vocab/m3-lite#ImageSensor -->

    <owl:Class rdf:about="http://purl.org/iot/vocab/m3-lite#ImageSensor">
        <rdfs:subClassOf rdf:resource="http://purl.oclc.org/NET/ssnx/ssn#SensingDevice"/>
        <rdfs:comment xml:lang="en">Sensor that detects and conveys the information that constitutes an image.</rdfs:comment>
        <rdfs:label xml:lang="en">Image Sensor</rdfs:label>
    </owl:Class>
    


    <!-- http://purl.org/iot/vocab/m3-lite#Inch -->

    <owl:Class rdf:about="http://purl.org/iot/vocab/m3-lite#Inch">
        <rdfs:subClassOf rdf:resource="http://purl.org/iot/vocab/m3-lite#Metre"/>
        <rdfs:comment xml:lang="en">Length in inches.</rdfs:comment>
        <rdfs:label xml:lang="en">Inch</rdfs:label>
    </owl:Class>
    


    <!-- http://purl.org/iot/vocab/m3-lite#Index -->

    <owl:Class rdf:about="http://purl.org/iot/vocab/m3-lite#Index">
        <rdfs:subClassOf rdf:resource="http://purl.org/NET/ssnx/qu/qu#Unit"/>
        <rdfs:comment>Arbitrary indirect reference which should be translated into meaningful measurements by using the corresponding decoding algorithm detailed in the resource description. In this case the returned values can only take certain values from a finite set.</rdfs:comment>
        <rdfs:label xml:lang="en">Index</rdfs:label>
    </owl:Class>
    


    <!-- http://purl.org/iot/vocab/m3-lite#IntDlLatency -->

    <owl:Class rdf:about="http://purl.org/iot/vocab/m3-lite#IntDlLatency">
        <rdfs:subClassOf rdf:resource="http://purl.org/iot/vocab/m3-lite#Communication"/>
        <rdfs:comment xml:lang="en">Downlink Latency.</rdfs:comment>
        <rdfs:label xml:lang="en">Downlink Latency</rdfs:label>
    </owl:Class>
    


    <!-- http://purl.org/iot/vocab/m3-lite#IntDlThroughputKbps -->

    <owl:Class rdf:about="http://purl.org/iot/vocab/m3-lite#IntDlThroughputKbps">
        <rdfs:subClassOf rdf:resource="http://purl.org/iot/vocab/m3-lite#Communication"/>
        <rdfs:comment xml:lang="en">Downlink Throughput.</rdfs:comment>
        <rdfs:label xml:lang="en">Downlink Throughput</rdfs:label>
    </owl:Class>
    


    <!-- http://purl.org/iot/vocab/m3-lite#IntUlPacketLoss -->

    <owl:Class rdf:about="http://purl.org/iot/vocab/m3-lite#IntUlPacketLoss">
        <rdfs:subClassOf rdf:resource="http://purl.org/iot/vocab/m3-lite#Communication"/>
        <rdfs:comment xml:lang="en">Uplink Packet Loss.</rdfs:comment>
        <rdfs:label xml:lang="en">Uplink Packet Loss</rdfs:label>
    </owl:Class>
    


    <!-- http://purl.org/iot/vocab/m3-lite#IntUlThroughputKbps -->

    <owl:Class rdf:about="http://purl.org/iot/vocab/m3-lite#IntUlThroughputKbps">
        <rdfs:subClassOf rdf:resource="http://purl.org/iot/vocab/m3-lite#Communication"/>
        <rdfs:comment xml:lang="en">Uplink Throughput.</rdfs:comment>
        <rdfs:label xml:lang="en">Uplink Throughput</rdfs:label>
    </owl:Class>
    


    <!-- http://purl.org/iot/vocab/m3-lite#Invalid -->

    <owl:Class rdf:about="http://purl.org/iot/vocab/m3-lite#Invalid">
        <rdfs:subClassOf rdf:resource="http://purl.org/iot/vocab/m3-lite#MeasurementType"/>
        <rdfs:comment xml:lang="en">If the measurement was tagged invalid.</rdfs:comment>
        <rdfs:label xml:lang="en">Invalid Measurement Type</rdfs:label>
    </owl:Class>
    


    <!-- http://purl.org/iot/vocab/m3-lite#IonisingRadiation -->

    <owl:Class rdf:about="http://purl.org/iot/vocab/m3-lite#IonisingRadiation">
        <rdfs:subClassOf rdf:resource="http://purl.org/NET/ssnx/qu/qu#QuantityKind"/>
        <rdfs:comment xml:lang="en">Ionising radiation is radiation that carries enough energy to free electrons from atoms or molecules, thereby ionizing them. Gamma rays, X-rays, and the higher ultraviolet part of the electromagnetic spectrum are ionizing, whereas the lower ultraviolet part of the electromagnetic spectrum, and also the lower part of the spectrum below UV, including visible light (including nearly all types of laser light), infrared, microwaves, and radio waves are all considered non-ionizing radiation.</rdfs:comment>
        <rdfs:label xml:lang="en">Ionising Radiation</rdfs:label>
    </owl:Class>
    


    <!-- http://purl.org/iot/vocab/m3-lite#Irrigation -->

    <owl:Class rdf:about="http://purl.org/iot/vocab/m3-lite#Irrigation">
        <rdfs:subClassOf rdf:resource="http://purl.oclc.org/NET/UNIS/fiware/iot-lite#ActuatingDevice"/>
        <rdfs:subClassOf>
            <owl:Restriction>
                <owl:onProperty rdf:resource="http://purl.org/iot/vocab/m3-lite#hasDomainOfInterest"/>
                <owl:someValuesFrom rdf:resource="http://purl.org/iot/vocab/m3-lite#Agriculture"/>
            </owl:Restriction>
        </rdfs:subClassOf>
        <rdfs:comment xml:lang="en">An actuator to automatically irrigate.</rdfs:comment>
        <rdfs:label xml:lang="en">Irrigation Actuation Device</rdfs:label>
    </owl:Class>
    


    <!-- http://purl.org/iot/vocab/m3-lite#Item -->

    <owl:Class rdf:about="http://purl.org/iot/vocab/m3-lite#Item">
        <rdfs:subClassOf rdf:resource="http://purl.org/NET/ssnx/qu/qu#Unit"/>
        <rdfs:comment xml:lang="en">Each of the accountable elements within a group.</rdfs:comment>
        <rdfs:label xml:lang="en">Item</rdfs:label>
    </owl:Class>
    


    <!-- http://purl.org/iot/vocab/m3-lite#Kelvin -->

    <owl:Class rdf:about="http://purl.org/iot/vocab/m3-lite#Kelvin">
        <rdfs:subClassOf rdf:resource="http://purl.org/NET/ssnx/qu/qu#Unit"/>
        <rdfs:comment xml:lang="en">Kelvin is a unit of measurement for temperature.</rdfs:comment>
        <rdfs:label xml:lang="en">Kelvin, Degree Kelvin</rdfs:label>
        <rdfs:seeAlso rdf:resource="http://sweet.jpl.nasa.gov/ontology/units.owl#kelvin"/>
    </owl:Class>
    


    <!-- http://purl.org/iot/vocab/m3-lite#KiloWattHour -->

    <owl:Class rdf:about="http://purl.org/iot/vocab/m3-lite#KiloWattHour">
        <rdfs:subClassOf rdf:resource="http://purl.org/NET/ssnx/qu/qu#Unit"/>
        <rdfs:comment xml:lang="en">Measure of electrical energy equivalent to a power consumption of one thousand watts for one hour.</rdfs:comment>
        <rdfs:label xml:lang="en">Kilo Watt Hour</rdfs:label>
        <rdfs:seeAlso rdf:resource="http://data.qudt.org/qudt/owl/1.0.0/unit.owl#KiloWatthour"/>
    </owl:Class>
    


    <!-- http://purl.org/iot/vocab/m3-lite#KilobitsPerSecond -->

    <owl:Class rdf:about="http://purl.org/iot/vocab/m3-lite#KilobitsPerSecond">
        <rdfs:subClassOf rdf:resource="http://purl.org/NET/ssnx/qu/qu#Unit"/>
        <rdfs:comment xml:lang="en">It is a unit of data transfer rate equal to: 1,000 bits per second.</rdfs:comment>
        <rdfs:label xml:lang="en">Kilobits Per Second</rdfs:label>
    </owl:Class>
    


    <!-- http://purl.org/iot/vocab/m3-lite#Kilogram -->

    <owl:Class rdf:about="http://purl.org/iot/vocab/m3-lite#Kilogram">
        <rdfs:subClassOf rdf:resource="http://purl.org/iot/vocab/m3-lite#Gram"/>
        <rdfs:comment xml:lang="en">The SI unit of mass, it is equal to the mass of the international prototype of the kilogram.</rdfs:comment>
        <rdfs:label xml:lang="en">Kilogram (kg)</rdfs:label>
        <rdfs:seeAlso>http://purl.oclc.org/NET/ssnx/qu/unit#kilogram</rdfs:seeAlso>
    </owl:Class>
    


    <!-- http://purl.org/iot/vocab/m3-lite#KilogramPerCubicMetre -->

    <owl:Class rdf:about="http://purl.org/iot/vocab/m3-lite#KilogramPerCubicMetre">
        <rdfs:subClassOf rdf:resource="http://purl.org/iot/vocab/m3-lite#GramPerCubicMetre"/>
        <rdfs:comment xml:lang="en">It is SI derived unit of density, defined by mass in kilograms divided by volume in cubic metres.</rdfs:comment>
        <rdfs:label xml:lang="en">Kilogram Per Cubic Metre, Kilogram Per Cubic Meter</rdfs:label>
    </owl:Class>
    


    <!-- http://purl.org/iot/vocab/m3-lite#Kilometre -->

    <owl:Class rdf:about="http://purl.org/iot/vocab/m3-lite#Kilometre">
        <rdfs:subClassOf rdf:resource="http://purl.org/iot/vocab/m3-lite#Metre"/>
        <rdfs:comment xml:lang="en">A metric unit of measurement equal to 1,000 metres (approx 0.62 miles).</rdfs:comment>
        <rdfs:label xml:lang="en">Kilometre, Kilometer</rdfs:label>
    </owl:Class>
    


    <!-- http://purl.org/iot/vocab/m3-lite#KilometrePerHour -->

    <owl:Class rdf:about="http://purl.org/iot/vocab/m3-lite#KilometrePerHour">
        <rdfs:subClassOf rdf:resource="http://purl.org/iot/vocab/m3-lite#MetrePerSecond"/>
        <rdfs:comment xml:lang="en">It is a unit of speed, expressing the number of kilometres travelled in one hour.</rdfs:comment>
        <rdfs:label xml:lang="en">Kilometre Per Hour, Kilometer Per Hour</rdfs:label>
        <rdfs:seeAlso>http://data.qudt.org/qudt/owl/1.0.0/unit.owl#KilometerPerHour</rdfs:seeAlso>
    </owl:Class>
    


    <!-- http://purl.org/iot/vocab/m3-lite#Lamp -->

    <owl:Class rdf:about="http://purl.org/iot/vocab/m3-lite#Lamp">
        <rdfs:subClassOf rdf:resource="http://purl.oclc.org/NET/UNIS/fiware/iot-lite#ActuatingDevice"/>
        <rdfs:subClassOf>
            <owl:Restriction>
                <owl:onProperty rdf:resource="http://purl.org/iot/vocab/m3-lite#hasDomainOfInterest"/>
                <owl:someValuesFrom rdf:resource="http://purl.org/iot/vocab/m3-lite#BuildingAutomation"/>
            </owl:Restriction>
        </rdfs:subClassOf>
        <rdfs:comment xml:lang="en">An actuator to automatically switch on/off the lamp.</rdfs:comment>
        <rdfs:label xml:lang="en">Lamp Actuating Device</rdfs:label>
    </owl:Class>
    


    <!-- http://purl.org/iot/vocab/m3-lite#Lavatory -->

    <owl:Class rdf:about="http://purl.org/iot/vocab/m3-lite#Lavatory">
        <rdfs:subClassOf rdf:resource="http://purl.oclc.org/NET/UNIS/fiware/iot-lite#ActuatingDevice"/>
        <rdfs:subClassOf>
            <owl:Restriction>
                <owl:onProperty rdf:resource="http://purl.org/iot/vocab/m3-lite#hasDomainOfInterest"/>
                <owl:someValuesFrom rdf:resource="http://purl.org/iot/vocab/m3-lite#BuildingAutomation"/>
            </owl:Restriction>
        </rdfs:subClassOf>
        <rdfs:comment xml:lang="en">An actuator to automatically switch on/off the lavatory.</rdfs:comment>
        <rdfs:label xml:lang="en">Lavatory</rdfs:label>
    </owl:Class>
    


    <!-- http://purl.org/iot/vocab/m3-lite#LeafWetness -->

    <owl:Class rdf:about="http://purl.org/iot/vocab/m3-lite#LeafWetness">
        <rdfs:subClassOf rdf:resource="http://purl.org/NET/ssnx/qu/qu#QuantityKind"/>
        <rdfs:comment xml:lang="en">Leaf wetness is a meteorological parameter that describes the amount of dew and precipitation left on surfaces. It is used for monitoring leaf moisture for agricultural purposes, such as fungus and disease control, for control of irrigation systems, and for detection of fog and dew conditions, and early detection of rainfall. (Source Wikipedia).</rdfs:comment>
        <rdfs:label xml:lang="en">Leaf Wetness</rdfs:label>
    </owl:Class>
    


    <!-- http://purl.org/iot/vocab/m3-lite#LeafWetnessSensor -->

    <owl:Class rdf:about="http://purl.org/iot/vocab/m3-lite#LeafWetnessSensor">
        <rdfs:subClassOf rdf:resource="http://purl.oclc.org/NET/ssnx/ssn#SensingDevice"/>
        <rdfs:subClassOf>
            <owl:Restriction>
                <owl:onProperty rdf:resource="http://purl.org/iot/vocab/m3-lite#hasDomainOfInterest"/>
                <owl:someValuesFrom rdf:resource="http://purl.org/iot/vocab/m3-lite#Agriculture"/>
            </owl:Restriction>
        </rdfs:subClassOf>
        <rdfs:comment xml:lang="en">Leaf Wetness Sensor is used in agriculture to check whether the plants need to be watered.</rdfs:comment>
        <rdfs:label xml:lang="en">Leaf Wetness Sensor</rdfs:label>
    </owl:Class>
    


    <!-- http://purl.org/iot/vocab/m3-lite#LightSensor -->

    <owl:Class rdf:about="http://purl.org/iot/vocab/m3-lite#LightSensor">
        <rdfs:subClassOf rdf:resource="http://purl.oclc.org/NET/ssnx/ssn#SensingDevice"/>
        <rdfs:subClassOf>
            <owl:Restriction>
                <owl:onProperty rdf:resource="http://purl.org/iot/vocab/m3-lite#hasDomainOfInterest"/>
                <owl:someValuesFrom rdf:resource="http://purl.org/iot/vocab/m3-lite#BuildingAutomation"/>
            </owl:Restriction>
        </rdfs:subClassOf>
        <rdfs:subClassOf>
            <owl:Restriction>
                <owl:onProperty rdf:resource="http://purl.org/iot/vocab/m3-lite#hasDomainOfInterest"/>
                <owl:someValuesFrom rdf:resource="http://purl.org/iot/vocab/m3-lite#Transportation"/>
            </owl:Restriction>
        </rdfs:subClassOf>
        <rdfs:subClassOf>
            <owl:Restriction>
                <owl:onProperty rdf:resource="http://purl.org/iot/vocab/m3-lite#hasDomainOfInterest"/>
                <owl:someValuesFrom rdf:resource="http://purl.org/iot/vocab/m3-lite#Weather"/>
            </owl:Restriction>
        </rdfs:subClassOf>
        <rdfs:comment xml:lang="en">Light/Illuminance Sensor is used to adjust the brightness of the surface.</rdfs:comment>
        <rdfs:label xml:lang="en">Light Sensor</rdfs:label>
    </owl:Class>
    


    <!-- http://purl.org/iot/vocab/m3-lite#Litre -->

    <owl:Class rdf:about="http://purl.org/iot/vocab/m3-lite#Litre">
        <rdfs:subClassOf rdf:resource="http://purl.org/NET/ssnx/qu/qu#Unit"/>
        <rdfs:comment xml:lang="en">A metric unit of capacity defined as the volume of one kilogram of water under standard conditions. It is equal to 1,000 cubic centimetres.</rdfs:comment>
        <rdfs:label xml:lang="en">Litre, Liter</rdfs:label>
        <rdfs:seeAlso>http://purl.oclc.org/NET/ssnx/qu/unit#litre</rdfs:seeAlso>
    </owl:Class>
    


    <!-- http://purl.org/iot/vocab/m3-lite#LitrePer100Kilometres -->

    <owl:Class rdf:about="http://purl.org/iot/vocab/m3-lite#LitrePer100Kilometres">
        <rdfs:subClassOf rdf:resource="http://purl.org/NET/ssnx/qu/qu#Unit"/>
        <rdfs:comment xml:lang="en">A consumption unit which is equal to the one of a vehicle which needs 1 fuel litre in order to traverse 100 kilometres.</rdfs:comment>
        <rdfs:label xml:lang="en">Litre Per 100 Kilometres, Liter Per 100 Kilometers</rdfs:label>
    </owl:Class>
    


    <!-- http://purl.org/iot/vocab/m3-lite#LoRaInterfaceEnergyMeter -->

    <owl:Class rdf:about="http://purl.org/iot/vocab/m3-lite#LoRaInterfaceEnergyMeter">
        <rdfs:subClassOf rdf:resource="http://purl.org/iot/vocab/m3-lite#EnergyMeter"/>
        <rdfs:comment xml:lang="en">Measure the average power consumption of the LoRa interface nodes.</rdfs:comment>
        <rdfs:label xml:lang="en">LoRa Interface Energy Meter</rdfs:label>
    </owl:Class>
    


    <!-- http://purl.org/iot/vocab/m3-lite#LocationQK -->

    <owl:Class rdf:about="http://purl.org/iot/vocab/m3-lite#LocationQK">
        <rdfs:subClassOf rdf:resource="http://purl.org/NET/ssnx/qu/qu#QuantityKind"/>
        <rdfs:comment xml:lang="en">A particular place or position.</rdfs:comment>
        <rdfs:label xml:lang="en">Location Quantity Kind</rdfs:label>
        <rdfs:seeAlso rdf:resource="http://www.w3.org/2003/01/geo/wgs84_pos#SpatialThing"/>
    </owl:Class>
    


    <!-- http://purl.org/iot/vocab/m3-lite#Lumen -->

    <owl:Class rdf:about="http://purl.org/iot/vocab/m3-lite#Lumen">
        <rdfs:subClassOf rdf:resource="http://purl.org/NET/ssnx/qu/qu#Unit"/>
        <rdfs:comment xml:lang="en">The SI unit of luminous flux, equal to the amount of light emitted per second in a unit solid angle of one steradian from a uniform source of one candela.</rdfs:comment>
        <rdfs:label xml:lang="en">Lumen (lm)</rdfs:label>
        <rdfs:seeAlso>http://purl.oclc.org/NET/ssnx/qu/unit#lumen</rdfs:seeAlso>
    </owl:Class>
    


    <!-- http://purl.org/iot/vocab/m3-lite#LuminousFlux -->

    <owl:Class rdf:about="http://purl.org/iot/vocab/m3-lite#LuminousFlux">
        <rdfs:subClassOf rdf:resource="http://purl.org/NET/ssnx/qu/qu#QuantityKind"/>
        <rdfs:comment xml:lang="en">Luminous Flux is the measure of the perceived power of light.</rdfs:comment>
        <rdfs:label xml:lang="en">Luminous Flux</rdfs:label>
    </owl:Class>
    


    <!-- http://purl.org/iot/vocab/m3-lite#LuminousIntensity -->

    <owl:Class rdf:about="http://purl.org/iot/vocab/m3-lite#LuminousIntensity">
        <rdfs:subClassOf rdf:resource="http://purl.org/NET/ssnx/qu/qu#QuantityKind"/>
        <rdfs:comment xml:lang="en"> It is a measure of the wavelength-weighted power emitted by a light source in a particular direction per unit solid angle, based on the luminosity function, a standardized model of the sensitivity of the human eye. The SI unit of luminous intensity is the candela (cd), an SI base unit. (Source Wikipedia)</rdfs:comment>
        <rdfs:label xml:lang="en">Luminous Intensity</rdfs:label>
    </owl:Class>
    


    <!-- http://purl.org/iot/vocab/m3-lite#Lux -->

    <owl:Class rdf:about="http://purl.org/iot/vocab/m3-lite#Lux">
        <rdfs:subClassOf rdf:resource="http://purl.org/NET/ssnx/qu/qu#Unit"/>
        <rdfs:comment xml:lang="en">The SI unit of illuminance, equal to one lumen per square metre.</rdfs:comment>
        <rdfs:label xml:lang="en">Lux (lx)</rdfs:label>
        <rdfs:seeAlso rdf:resource="http://data.qudt.org/qudt/owl/1.0.0/unit.owl#Lux"/>
        <rdfs:seeAlso rdf:resource="http://sweet.jpl.nasa.gov/ontology/units.owl#lux"/>
        <rdfs:seeAlso>http://purl.oclc.org/NET/ssnx/qu/unit#lux</rdfs:seeAlso>
    </owl:Class>
    


    <!-- http://purl.org/iot/vocab/m3-lite#MagneticField -->

    <owl:Class rdf:about="http://purl.org/iot/vocab/m3-lite#MagneticField">
        <rdfs:subClassOf rdf:resource="http://purl.org/NET/ssnx/qu/qu#QuantityKind"/>
        <rdfs:comment xml:lang="en">A region around a magnetic material or a moving electric charge within which the force of magnetism acts.</rdfs:comment>
        <rdfs:label xml:lang="en">Magnetic Field</rdfs:label>
    </owl:Class>
    


    <!-- http://purl.org/iot/vocab/m3-lite#MagneticFluxDensity -->

    <owl:Class rdf:about="http://purl.org/iot/vocab/m3-lite#MagneticFluxDensity">
        <rdfs:subClassOf rdf:resource="http://purl.org/NET/ssnx/qu/qu#QuantityKind"/>
        <rdfs:comment xml:lang="en">It is the magnetic flux  through a surface is the surface integral of the normal component of the magnetic field (B) passing through that surface. The SI unit of magnetic flux is the weber (Wb). (Source Wikipedia).</rdfs:comment>
        <rdfs:label xml:lang="en">Magnetic Flux Density</rdfs:label>
    </owl:Class>
    


    <!-- http://purl.org/iot/vocab/m3-lite#Magnetometer -->

    <owl:Class rdf:about="http://purl.org/iot/vocab/m3-lite#Magnetometer">
        <rdfs:subClassOf rdf:resource="http://purl.oclc.org/NET/ssnx/ssn#SensingDevice"/>
        <rdfs:subClassOf>
            <owl:Restriction>
                <owl:onProperty rdf:resource="http://purl.org/iot/vocab/m3-lite#hasDomainOfInterest"/>
                <owl:someValuesFrom rdf:resource="http://purl.org/iot/vocab/m3-lite#BuildingAutomation"/>
            </owl:Restriction>
        </rdfs:subClassOf>
        <rdfs:comment xml:lang="en">A magnetometer is an device that measures magnetismeither magnetization of magnetic material like a ferromagnet, or the strength and, in some cases, direction of the magnetic field at a point in space. (Source Wikipedia).</rdfs:comment>
        <rdfs:label xml:lang="en">Magnetometer</rdfs:label>
    </owl:Class>
    


    <!-- http://purl.org/iot/vocab/m3-lite#Manual -->

    <owl:Class rdf:about="http://purl.org/iot/vocab/m3-lite#Manual">
        <rdfs:subClassOf rdf:resource="http://purl.org/iot/vocab/m3-lite#MeasurementType"/>
        <rdfs:comment xml:lang="en">If the measurement was taken when human effort was involved.</rdfs:comment>
        <rdfs:label xml:lang="en">Manual Measurement Type</rdfs:label>
    </owl:Class>
    


    <!-- http://purl.org/iot/vocab/m3-lite#Mass -->

    <owl:Class rdf:about="http://purl.org/iot/vocab/m3-lite#Mass">
        <rdfs:subClassOf rdf:resource="http://purl.org/NET/ssnx/qu/qu#QuantityKind"/>
        <rdfs:comment xml:lang="en">Mass is a property of a physical body. It is the measure of an object&apos;s resistance to acceleration when a net force is applied.</rdfs:comment>
        <rdfs:label xml:lang="en">Mass</rdfs:label>
        <rdfs:seeAlso>http://purl.oclc.org/NET/ssnx/qu/quantity#mass</rdfs:seeAlso>
    </owl:Class>
    


    <!-- http://purl.org/iot/vocab/m3-lite#MeasurementType -->

    <owl:Class rdf:about="http://purl.org/iot/vocab/m3-lite#MeasurementType">
        <rdfs:comment xml:lang="en">Type of Measurement done using a device.</rdfs:comment>
        <rdfs:label xml:lang="en">Measurement Type</rdfs:label>
    </owl:Class>
    


    <!-- http://purl.org/iot/vocab/m3-lite#MethaneSensor -->

    <owl:Class rdf:about="http://purl.org/iot/vocab/m3-lite#MethaneSensor">
        <rdfs:subClassOf rdf:resource="http://purl.org/iot/vocab/m3-lite#GaseousPollutantSensor"/>
        <rdfs:comment xml:lang="en">Device used to detect Methane in the environment.</rdfs:comment>
        <rdfs:label xml:lang="en">Methane (CH4) Sensor</rdfs:label>
    </owl:Class>
    


    <!-- http://purl.org/iot/vocab/m3-lite#Metre -->

    <owl:Class rdf:about="http://purl.org/iot/vocab/m3-lite#Metre">
        <rdfs:subClassOf rdf:resource="http://purl.org/NET/ssnx/qu/qu#Unit"/>
        <rdfs:comment xml:lang="en">It is the unit of length.</rdfs:comment>
        <rdfs:label xml:lang="en">Metre, Meter</rdfs:label>
        <rdfs:seeAlso rdf:resource="http://data.qudt.org/qudt/owl/1.0.0/unit.owl#Meter"/>
        <rdfs:seeAlso rdf:resource="http://sweet.jpl.nasa.gov/ontology/units.owl#meter"/>
    </owl:Class>
    


    <!-- http://purl.org/iot/vocab/m3-lite#MetrePerSecond -->

    <owl:Class rdf:about="http://purl.org/iot/vocab/m3-lite#MetrePerSecond">
        <rdfs:subClassOf rdf:resource="http://purl.org/NET/ssnx/qu/qu#Unit"/>
        <rdfs:comment xml:lang="en">A speed/velocity unit which is equal to the speed of an object traveling 1 metre distance in one second.</rdfs:comment>
        <rdfs:label xml:lang="en">Metre Per Second, Meter Per Second  (m/s)</rdfs:label>
        <rdfs:seeAlso rdf:resource="http://data.qudt.org/qudt/owl/1.0.0/unit.owl#MeterPerSecond"/>
        <rdfs:seeAlso>http://purl.oclc.org/NET/ssnx/qu/unit#metrePerSecond</rdfs:seeAlso>
    </owl:Class>
    


    <!-- http://purl.org/iot/vocab/m3-lite#MetrePerSecondSquare -->

    <owl:Class rdf:about="http://purl.org/iot/vocab/m3-lite#MetrePerSecondSquare">
        <rdfs:subClassOf rdf:resource="http://purl.org/NET/ssnx/qu/qu#Unit"/>
        <rdfs:comment xml:lang="en">It is the unit of acceleration.</rdfs:comment>
        <rdfs:label xml:lang="en">Metre Per Second Square, Meter Per Second Square</rdfs:label>
        <rdfs:seeAlso rdf:resource="http://purl.oclc.org/NET/ssnx/qu/unit#metrePerSecondSquared"/>
    </owl:Class>
    


    <!-- http://purl.org/iot/vocab/m3-lite#Microampere -->

    <owl:Class rdf:about="http://purl.org/iot/vocab/m3-lite#Microampere">
        <rdfs:subClassOf rdf:resource="http://purl.org/iot/vocab/m3-lite#Ampere"/>
        <rdfs:comment xml:lang="en">It is a unit of electric current, or amount of electric charge per second.</rdfs:comment>
        <rdfs:label xml:lang="en">Microampere (uA)</rdfs:label>
    </owl:Class>
    


    <!-- http://purl.org/iot/vocab/m3-lite#Microgram -->

    <owl:Class rdf:about="http://purl.org/iot/vocab/m3-lite#Microgram">
        <rdfs:subClassOf rdf:resource="http://purl.org/iot/vocab/m3-lite#Gram"/>
        <rdfs:comment xml:lang="en">It is a unit of mass equal to one billionth (110^9) of a kilogram.</rdfs:comment>
        <rdfs:label xml:lang="en">Microgram (ug)</rdfs:label>
    </owl:Class>
    


    <!-- http://purl.org/iot/vocab/m3-lite#MicrogramPerCubicMetre -->

    <owl:Class rdf:about="http://purl.org/iot/vocab/m3-lite#MicrogramPerCubicMetre">
        <rdfs:subClassOf rdf:resource="http://purl.org/iot/vocab/m3-lite#GramPerCubicMetre"/>
        <rdfs:comment xml:lang="en">Microgram per cubic metre is a unit of density defined as microgram divided by cubic metre. Milligram per cubic metre is a derived unit in the International System of Units.</rdfs:comment>
        <rdfs:label xml:lang="en">Microgram Per Cubic Metre, Microgram Per Cubic Meter</rdfs:label>
        <rdfs:seeAlso>http://purl.oclc.org/NET/ssnx/qu/unit#microgramPerCubicMetre</rdfs:seeAlso>
    </owl:Class>
    


    <!-- http://purl.org/iot/vocab/m3-lite#Microvolt -->

    <owl:Class rdf:about="http://purl.org/iot/vocab/m3-lite#Microvolt">
        <rdfs:subClassOf rdf:resource="http://purl.org/iot/vocab/m3-lite#Volt"/>
        <rdfs:comment xml:lang="en">It is a unit of electromotive force or potential difference equal to one millionth of a volt. </rdfs:comment>
        <rdfs:label xml:lang="en">Microvolt (uV)</rdfs:label>
    </owl:Class>
    


    <!-- http://purl.org/iot/vocab/m3-lite#Microwatt -->

    <owl:Class rdf:about="http://purl.org/iot/vocab/m3-lite#Microwatt">
        <rdfs:subClassOf rdf:resource="http://purl.org/iot/vocab/m3-lite#Watt"/>
        <rdfs:comment xml:lang="en">It is a unit of power.</rdfs:comment>
        <rdfs:label xml:lang="en">Microwatt (uW)</rdfs:label>
    </owl:Class>
    


    <!-- http://purl.org/iot/vocab/m3-lite#MicrowattPerSquareCentimetre -->

    <owl:Class rdf:about="http://purl.org/iot/vocab/m3-lite#MicrowattPerSquareCentimetre">
        <rdfs:subClassOf rdf:resource="http://purl.org/iot/vocab/m3-lite#WattPerSquareMetre"/>
        <rdfs:comment xml:lang="en">It is one of the unit for radiative and other energy fluxes.</rdfs:comment>
        <rdfs:label xml:lang="en">Microwatt Per Square Centimetre, Microwatt Per Square Centimeter</rdfs:label>
    </owl:Class>
    


    <!-- http://purl.org/iot/vocab/m3-lite#Microwave -->

    <owl:Class rdf:about="http://purl.org/iot/vocab/m3-lite#Microwave">
        <rdfs:subClassOf rdf:resource="http://purl.oclc.org/NET/UNIS/fiware/iot-lite#ActuatingDevice"/>
        <rdfs:subClassOf>
            <owl:Restriction>
                <owl:onProperty rdf:resource="http://purl.org/iot/vocab/m3-lite#hasDomainOfInterest"/>
                <owl:someValuesFrom rdf:resource="http://purl.org/iot/vocab/m3-lite#BuildingAutomation"/>
            </owl:Restriction>
        </rdfs:subClassOf>
        <rdfs:comment xml:lang="en">An actuator to automatically switch on/off the Microwave.</rdfs:comment>
        <rdfs:label xml:lang="en">Microwave Actuating Device</rdfs:label>
    </owl:Class>
    


    <!-- http://purl.org/iot/vocab/m3-lite#Mileage -->

    <owl:Class rdf:about="http://purl.org/iot/vocab/m3-lite#Mileage">
        <rdfs:subClassOf rdf:resource="http://purl.org/NET/ssnx/qu/qu#QuantityKind"/>
        <rdfs:comment xml:lang="en">Measure of the number of miles or the average distance that a vehicle can travel on a specified quantity of fuel</rdfs:comment>
        <rdfs:label xml:lang="en">Mileage</rdfs:label>
    </owl:Class>
    


    <!-- http://purl.org/iot/vocab/m3-lite#MileageDistanceToService -->

    <owl:Class rdf:about="http://purl.org/iot/vocab/m3-lite#MileageDistanceToService">
        <rdfs:subClassOf rdf:resource="http://purl.org/iot/vocab/m3-lite#Mileage"/>
        <rdfs:comment xml:lang="en">The distance which can be travelled by the vehicle before the next service inspection is required.  A negative distance is transmitted if the service inspection has been passed.</rdfs:comment>
        <rdfs:label xml:lang="en">Mileage Distance To Service</rdfs:label>
    </owl:Class>
    


    <!-- http://purl.org/iot/vocab/m3-lite#MileageTotal -->

    <owl:Class rdf:about="http://purl.org/iot/vocab/m3-lite#MileageTotal">
        <rdfs:subClassOf rdf:resource="http://purl.org/iot/vocab/m3-lite#Mileage"/>
        <rdfs:comment xml:lang="en">The total distance travelled by the particular vehicle since its initial production.</rdfs:comment>
        <rdfs:label xml:lang="en">Mileage Total</rdfs:label>
    </owl:Class>
    


    <!-- http://purl.org/iot/vocab/m3-lite#Miles -->

    <owl:Class rdf:about="http://purl.org/iot/vocab/m3-lite#Miles">
        <rdfs:subClassOf rdf:resource="http://purl.org/iot/vocab/m3-lite#Metre"/>
        <rdfs:comment xml:lang="en">It is a unit of length that is equal to 1,760 yards (approx. 1.609 kilometres).</rdfs:comment>
        <rdfs:label xml:lang="en">Miles</rdfs:label>
    </owl:Class>
    


    <!-- http://purl.org/iot/vocab/m3-lite#Milliampere -->

    <owl:Class rdf:about="http://purl.org/iot/vocab/m3-lite#Milliampere">
        <rdfs:subClassOf rdf:resource="http://purl.org/iot/vocab/m3-lite#Ampere"/>
        <rdfs:comment xml:lang="en">One thousandth of an ampere.</rdfs:comment>
        <rdfs:label xml:lang="en">Milliampere (mA)</rdfs:label>
    </owl:Class>
    


    <!-- http://purl.org/iot/vocab/m3-lite#Millibar -->

    <owl:Class rdf:about="http://purl.org/iot/vocab/m3-lite#Millibar">
        <rdfs:subClassOf rdf:resource="http://purl.org/iot/vocab/m3-lite#Bar"/>
        <rdfs:comment xml:lang="en">One thousandth of a bar.</rdfs:comment>
        <rdfs:label xml:lang="en">Millibar</rdfs:label>
    </owl:Class>
    


    <!-- http://purl.org/iot/vocab/m3-lite#Milligram -->

    <owl:Class rdf:about="http://purl.org/iot/vocab/m3-lite#Milligram">
        <rdfs:subClassOf rdf:resource="http://purl.org/iot/vocab/m3-lite#Gram"/>
        <rdfs:comment xml:lang="en">One thousandth of a gram.</rdfs:comment>
        <rdfs:label xml:lang="en">Milligram (mg)</rdfs:label>
    </owl:Class>
    


    <!-- http://purl.org/iot/vocab/m3-lite#MilligramPerCubicMetre -->

    <owl:Class rdf:about="http://purl.org/iot/vocab/m3-lite#MilligramPerCubicMetre">
        <rdfs:subClassOf rdf:resource="http://purl.org/iot/vocab/m3-lite#GramPerCubicMetre"/>
        <rdfs:comment xml:lang="en">It is a density measurement unit.</rdfs:comment>
        <rdfs:label xml:lang="en">Milligram Per Cubic Metre, Milligram Per Cubic Meter</rdfs:label>
    </owl:Class>
    


    <!-- http://purl.org/iot/vocab/m3-lite#MilligramPerLitre -->

    <owl:Class rdf:about="http://purl.org/iot/vocab/m3-lite#MilligramPerLitre">
        <rdfs:subClassOf rdf:resource="http://purl.org/iot/vocab/m3-lite#GramPerLitre"/>
        <rdfs:comment xml:lang="en">Level of Dissolved substance in liquid measured in mg per litre.</rdfs:comment>
        <rdfs:label xml:lang="en">Milligram Per Litre, Milligram Per Liter</rdfs:label>
    </owl:Class>
    


    <!-- http://purl.org/iot/vocab/m3-lite#MilligramPerSquareMetre -->

    <owl:Class rdf:about="http://purl.org/iot/vocab/m3-lite#MilligramPerSquareMetre">
        <rdfs:subClassOf rdf:resource="http://purl.org/NET/ssnx/qu/qu#Unit"/>
        <rdfs:comment xml:lang="en">A dose unit which is equal to 1 milligram of a substance per square metre of surface area of the recipient subject.</rdfs:comment>
        <rdfs:label xml:lang="en">Milligram Per Square Metre, Milligram Per Square Meter</rdfs:label>
        <rdfs:seeAlso>http://purl.oclc.org/NET/ssnx/qu/unit#milligramPerSquareMetre</rdfs:seeAlso>
    </owl:Class>
    


    <!-- http://purl.org/iot/vocab/m3-lite#Millilitre -->

    <owl:Class rdf:about="http://purl.org/iot/vocab/m3-lite#Millilitre">
        <rdfs:subClassOf rdf:resource="http://purl.org/iot/vocab/m3-lite#Litre"/>
        <rdfs:comment xml:lang="en">One thousandth of a litre (0.002 pint).</rdfs:comment>
        <rdfs:label xml:lang="en">Millilitre, Milliliter</rdfs:label>
    </owl:Class>
    


    <!-- http://purl.org/iot/vocab/m3-lite#Millimetre -->

    <owl:Class rdf:about="http://purl.org/iot/vocab/m3-lite#Millimetre">
        <rdfs:subClassOf rdf:resource="http://purl.org/iot/vocab/m3-lite#Metre"/>
        <rdfs:comment xml:lang="en">One thousandth of a metre (0.039 in).</rdfs:comment>
        <rdfs:label xml:lang="en">Millimetre, Millimeter</rdfs:label>
    </owl:Class>
    


    <!-- http://purl.org/iot/vocab/m3-lite#MillimetrePerHour -->

    <owl:Class rdf:about="http://purl.org/iot/vocab/m3-lite#MillimetrePerHour">
        <rdfs:subClassOf rdf:resource="http://purl.org/NET/ssnx/qu/qu#Unit"/>
        <rdfs:comment xml:lang="en">A unit of both speed (scalar) and velocity (vector), defined as the distance of one millimetre travelled per unit hour.</rdfs:comment>
        <rdfs:label xml:lang="en">Millimetre Per Hour, Millimeter Per Hour</rdfs:label>
        <rdfs:seeAlso>http://purl.oclc.org/NET/ssnx/qu/unit#millimetrePerHour</rdfs:seeAlso>
    </owl:Class>
    


    <!-- http://purl.org/iot/vocab/m3-lite#Millisecond -->

    <owl:Class rdf:about="http://purl.org/iot/vocab/m3-lite#Millisecond">
        <rdfs:subClassOf rdf:resource="http://purl.org/iot/vocab/m3-lite#SecondTime"/>
        <rdfs:comment xml:lang="en">One thousandth of a second.</rdfs:comment>
        <rdfs:label xml:lang="en">Millisecond</rdfs:label>
    </owl:Class>
    


    <!-- http://purl.org/iot/vocab/m3-lite#Millivolt -->

    <owl:Class rdf:about="http://purl.org/iot/vocab/m3-lite#Millivolt">
        <rdfs:subClassOf rdf:resource="http://purl.org/iot/vocab/m3-lite#Volt"/>
        <rdfs:comment xml:lang="en">One thousandth of a volt.</rdfs:comment>
        <rdfs:label xml:lang="en">Millivolt (mV)</rdfs:label>
    </owl:Class>
    


    <!-- http://purl.org/iot/vocab/m3-lite#MillivoltPerMetre -->

    <owl:Class rdf:about="http://purl.org/iot/vocab/m3-lite#MillivoltPerMetre">
        <rdfs:subClassOf rdf:resource="http://purl.org/NET/ssnx/qu/qu#Unit"/>
        <rdfs:comment xml:lang="en">It is a measure of the intensity of the signal of a radio transmitter.</rdfs:comment>
        <rdfs:label xml:lang="en">Millivolt Per Metre, Millivolt Per Meter</rdfs:label>
    </owl:Class>
    


    <!-- http://purl.org/iot/vocab/m3-lite#Milliwatt -->

    <owl:Class rdf:about="http://purl.org/iot/vocab/m3-lite#Milliwatt">
        <rdfs:subClassOf rdf:resource="http://purl.org/iot/vocab/m3-lite#Watt"/>
        <rdfs:comment xml:lang="en">A unit of power equal to one thousandth of a watt.</rdfs:comment>
        <rdfs:label xml:lang="en">Milliwatt (mW)</rdfs:label>
    </owl:Class>
    


    <!-- http://purl.org/iot/vocab/m3-lite#MinuteAngle -->

    <owl:Class rdf:about="http://purl.org/iot/vocab/m3-lite#MinuteAngle">
        <rdfs:subClassOf rdf:resource="http://purl.org/NET/ssnx/qu/qu#Unit"/>
        <rdfs:comment xml:lang="en">A Minute of Angle (MOA) is an angular measurement. A MOA is 1/60th of a degree.</rdfs:comment>
        <rdfs:label xml:lang="en">Minute Angle</rdfs:label>
    </owl:Class>
    


    <!-- http://purl.org/iot/vocab/m3-lite#MinuteTime -->

    <owl:Class rdf:about="http://purl.org/iot/vocab/m3-lite#MinuteTime">
        <rdfs:subClassOf rdf:resource="http://purl.org/iot/vocab/m3-lite#SecondTime"/>
        <rdfs:comment xml:lang="en">A unit of time equal to 60 seconds or 1/60th of an hour.</rdfs:comment>
        <rdfs:label xml:lang="en">Minute Time</rdfs:label>
    </owl:Class>
    


    <!-- http://purl.org/iot/vocab/m3-lite#MmHg -->

    <owl:Class rdf:about="http://purl.org/iot/vocab/m3-lite#MmHg">
        <rdfs:subClassOf rdf:resource="http://purl.org/NET/ssnx/qu/qu#Unit"/>
        <rdfs:comment xml:lang="en">A millimetre of mercury is a manometric unit of pressure, formerly defined as the extra pressure generated by a column of mercury one millimetre high and now defined as precisely 133.322387415 pascals. It is denoted by the symbol mmHg. It  is used to measure blood pressure measurements (systolic and diastolic).</rdfs:comment>
        <rdfs:label xml:lang="en">MmHg</rdfs:label>
    </owl:Class>
    


    <!-- http://purl.org/iot/vocab/m3-lite#MmolPerLitre -->

    <owl:Class rdf:about="http://purl.org/iot/vocab/m3-lite#MmolPerLitre">
        <rdfs:subClassOf rdf:resource="http://purl.org/NET/ssnx/qu/qu#Unit"/>
        <rdfs:comment xml:lang="en">It is the amount of a substance that corresponds to its formula mass in milligrams. MmolPerLitre is used to measure cholesterol.</rdfs:comment>
        <rdfs:label xml:lang="en">Mmol Per Litre, Mmol Per Liter</rdfs:label>
    </owl:Class>
    


    <!-- http://purl.org/iot/vocab/m3-lite#MobHoExecSuccRate -->

    <owl:Class rdf:about="http://purl.org/iot/vocab/m3-lite#MobHoExecSuccRate">
        <rdfs:subClassOf rdf:resource="http://purl.org/iot/vocab/m3-lite#Communication"/>
        <rdfs:comment xml:lang="en">Handover Execution.</rdfs:comment>
        <rdfs:label xml:lang="en">Handover Execution</rdfs:label>
    </owl:Class>
    


    <!-- http://purl.org/iot/vocab/m3-lite#MobHoPrepSuccRate -->

    <owl:Class rdf:about="http://purl.org/iot/vocab/m3-lite#MobHoPrepSuccRate">
        <rdfs:subClassOf rdf:resource="http://purl.org/iot/vocab/m3-lite#Communication"/>
        <rdfs:comment xml:lang="en">Handover Preparation Success Rate.</rdfs:comment>
        <rdfs:label xml:lang="en">Handover Preparation Success Rate</rdfs:label>
    </owl:Class>
    


    <!-- http://purl.org/iot/vocab/m3-lite#MobMobilitySuccRate -->

    <owl:Class rdf:about="http://purl.org/iot/vocab/m3-lite#MobMobilitySuccRate">
        <rdfs:subClassOf rdf:resource="http://purl.org/iot/vocab/m3-lite#Communication"/>
        <rdfs:comment xml:lang="en">Handover Mobility Success Rate.</rdfs:comment>
        <rdfs:label xml:lang="en">Handover Mobility Success Rate</rdfs:label>
    </owl:Class>
    


    <!-- http://purl.org/iot/vocab/m3-lite#Motion -->

    <owl:Class rdf:about="http://purl.org/iot/vocab/m3-lite#Motion">
        <rdfs:subClassOf rdf:resource="http://purl.org/NET/ssnx/qu/qu#QuantityKind"/>
        <rdfs:comment xml:lang="en">It is the action or process of moving or being moved.</rdfs:comment>
        <rdfs:label xml:lang="en">Motion</rdfs:label>
        <rdfs:seeAlso rdf:resource="http://spitfire-project.eu/ontology/ns/Motion"/>
    </owl:Class>
    


    <!-- http://purl.org/iot/vocab/m3-lite#MotionState -->

    <owl:Class rdf:about="http://purl.org/iot/vocab/m3-lite#MotionState">
        <rdfs:subClassOf rdf:resource="http://purl.org/NET/ssnx/qu/qu#QuantityKind"/>
        <rdfs:comment xml:lang="en">Indicator of whether a person (or object) is detected upon his/her/its movement.</rdfs:comment>
        <rdfs:label xml:lang="en">Motion State</rdfs:label>
    </owl:Class>
    


    <!-- http://purl.org/iot/vocab/m3-lite#MotionStateVehicle -->

    <owl:Class rdf:about="http://purl.org/iot/vocab/m3-lite#MotionStateVehicle">
        <rdfs:subClassOf rdf:resource="http://purl.org/iot/vocab/m3-lite#MotionState"/>
        <rdfs:comment>Indicates whether motion of the vehicle is detected or not.</rdfs:comment>
        <rdfs:label xml:lang="en">Motion State Vehicle</rdfs:label>
    </owl:Class>
    


    <!-- http://purl.org/iot/vocab/m3-lite#NFC -->

    <owl:Class rdf:about="http://purl.org/iot/vocab/m3-lite#NFC">
        <rdfs:subClassOf rdf:resource="http://purl.oclc.org/NET/UNIS/fiware/iot-lite#TagDevice"/>
        <rdfs:comment xml:lang="en">A tagging device can be NFC (Near Field Communication).</rdfs:comment>
        <rdfs:label xml:lang="en">NFC Tagging Device</rdfs:label>
    </owl:Class>
    


    <!-- http://purl.org/iot/vocab/m3-lite#NH3Sensor -->

    <owl:Class rdf:about="http://purl.org/iot/vocab/m3-lite#NH3Sensor">
        <rdfs:subClassOf rdf:resource="http://purl.org/iot/vocab/m3-lite#GaseousPollutantSensor"/>
        <rdfs:comment xml:lang="en">Device used to detect NH3 level in the environment.</rdfs:comment>
        <rdfs:label xml:lang="en">NH3 Sensor</rdfs:label>
    </owl:Class>
    


    <!-- http://purl.org/iot/vocab/m3-lite#NO2Sensor -->

    <owl:Class rdf:about="http://purl.org/iot/vocab/m3-lite#NO2Sensor">
        <rdfs:subClassOf rdf:resource="http://purl.org/iot/vocab/m3-lite#GaseousPollutantSensor"/>
        <rdfs:subClassOf>
            <owl:Restriction>
                <owl:onProperty rdf:resource="http://purl.org/iot/vocab/m3-lite#hasDomainOfInterest"/>
                <owl:someValuesFrom rdf:resource="http://purl.org/iot/vocab/m3-lite#Environment"/>
            </owl:Restriction>
        </rdfs:subClassOf>
        <rdfs:comment xml:lang="en">Sensor detecting levels of Nitrogen Dioxide (NO2) in the environment.</rdfs:comment>
        <rdfs:label xml:lang="en">Nitrogen Dioxide (NO2) Sensor</rdfs:label>
    </owl:Class>
    


    <!-- http://purl.org/iot/vocab/m3-lite#NOSensor -->

    <owl:Class rdf:about="http://purl.org/iot/vocab/m3-lite#NOSensor">
        <rdfs:subClassOf rdf:resource="http://purl.org/iot/vocab/m3-lite#GaseousPollutantSensor"/>
        <rdfs:comment xml:lang="en">Device used to detect Nitrogen Oxide (NO) in the environment.</rdfs:comment>
        <rdfs:label xml:lang="en">Nitrogen Oxide (NO) Sensor</rdfs:label>
    </owl:Class>
    


    <!-- http://purl.org/iot/vocab/m3-lite#Neighbours -->

    <owl:Class rdf:about="http://purl.org/iot/vocab/m3-lite#Neighbours">
        <rdfs:subClassOf rdf:resource="http://purl.org/iot/vocab/m3-lite#SoundSource"/>
        <rdfs:comment xml:lang="en">When the source of the sound were noisy neighbours.</rdfs:comment>
        <rdfs:label xml:lang="en">Neighbours Sound Source</rdfs:label>
    </owl:Class>
    


    <!-- http://purl.org/iot/vocab/m3-lite#O3Sensor -->

    <owl:Class rdf:about="http://purl.org/iot/vocab/m3-lite#O3Sensor">
        <rdfs:subClassOf rdf:resource="http://purl.org/iot/vocab/m3-lite#GaseousPollutantSensor"/>
        <rdfs:comment xml:lang="en">Device used to detect Ozone (O3) in the environment.</rdfs:comment>
        <rdfs:label xml:lang="en">Ozone (O3) Sensor</rdfs:label>
    </owl:Class>
    


    <!-- http://purl.org/iot/vocab/m3-lite#Odometer -->

    <owl:Class rdf:about="http://purl.org/iot/vocab/m3-lite#Odometer">
        <rdfs:subClassOf rdf:resource="http://purl.oclc.org/NET/ssnx/ssn#SensingDevice"/>
        <rdfs:comment xml:lang="en">An odometer or odograph is an instrument that indicates distance travelled by a vehicle, such as bicycle or automobile.</rdfs:comment>
        <rdfs:label xml:lang="en">Odometer</rdfs:label>
    </owl:Class>
    


    <!-- http://purl.org/iot/vocab/m3-lite#Ohm -->

    <owl:Class rdf:about="http://purl.org/iot/vocab/m3-lite#Ohm">
        <rdfs:subClassOf rdf:resource="http://purl.org/NET/ssnx/qu/qu#Unit"/>
        <rdfs:comment xml:lang="en">Ohm is the unit of electrical resistance.</rdfs:comment>
        <rdfs:label xml:lang="en">Ohm</rdfs:label>
        <rdfs:seeAlso rdf:resource="http://sweet.jpl.nasa.gov/ontology/units.owl#ohm"/>
    </owl:Class>
    


    <!-- http://purl.org/iot/vocab/m3-lite#Okta -->

    <owl:Class rdf:about="http://purl.org/iot/vocab/m3-lite#Okta">
        <rdfs:subClassOf rdf:resource="http://purl.org/NET/ssnx/qu/qu#Unit"/>
        <rdfs:comment xml:lang="en">Okta is the unit to measure the cloud cover.</rdfs:comment>
        <rdfs:label xml:lang="en">Okta</rdfs:label>
    </owl:Class>
    


    <!-- http://purl.org/iot/vocab/m3-lite#OpticalDustSensor -->

    <owl:Class rdf:about="http://purl.org/iot/vocab/m3-lite#OpticalDustSensor">
        <rdfs:subClassOf rdf:resource="http://purl.org/iot/vocab/m3-lite#DustSensor"/>
        <rdfs:comment xml:lang="en">A sensing device that measures dust particle concentration using optical sensing mean.</rdfs:comment>
        <rdfs:label xml:lang="en">Optical Dust Sensor</rdfs:label>
    </owl:Class>
    


    <!-- http://purl.org/iot/vocab/m3-lite#Others -->

    <owl:Class rdf:about="http://purl.org/iot/vocab/m3-lite#Others">
        <rdfs:subClassOf rdf:resource="http://purl.org/NET/ssnx/qu/qu#QuantityKind"/>
        <rdfs:subClassOf rdf:resource="http://purl.org/NET/ssnx/qu/qu#Unit"/>
        <rdfs:subClassOf rdf:resource="http://purl.org/iot/vocab/m3-lite#MeasurementType"/>
        <rdfs:subClassOf rdf:resource="http://purl.org/iot/vocab/m3-lite#SoundSource"/>
        <rdfs:subClassOf rdf:resource="http://purl.org/iot/vocab/m3-lite#Source"/>
        <rdfs:comment xml:lang="en">Relates to phenomenon and unit that are not available currently in the current version of Taxonomy.</rdfs:comment>
        <rdfs:label xml:lang="en">Others</rdfs:label>
    </owl:Class>
    


    <!-- http://purl.org/iot/vocab/m3-lite#OxygenSensor -->

    <owl:Class rdf:about="http://purl.org/iot/vocab/m3-lite#OxygenSensor">
        <rdfs:subClassOf rdf:resource="http://purl.org/iot/vocab/m3-lite#GaseousPollutantSensor"/>
        <rdfs:comment xml:lang="en">Device used to detect Oxygen (O2) in the environment.</rdfs:comment>
        <rdfs:label xml:lang="en">Oxygen Sensor</rdfs:label>
    </owl:Class>
    


    <!-- http://purl.org/iot/vocab/m3-lite#PH -->

    <owl:Class rdf:about="http://purl.org/iot/vocab/m3-lite#PH">
        <rdfs:subClassOf rdf:resource="http://purl.org/NET/ssnx/qu/qu#QuantityKind"/>
        <rdfs:comment xml:lang="en">It is a numeric scale used to specify the acidity or basicity of an aqueous solution.</rdfs:comment>
        <rdfs:label xml:lang="en">PH</rdfs:label>
    </owl:Class>
    


    <!-- http://purl.org/iot/vocab/m3-lite#PHSensor -->

    <owl:Class rdf:about="http://purl.org/iot/vocab/m3-lite#PHSensor">
        <rdfs:subClassOf rdf:resource="http://purl.oclc.org/NET/ssnx/ssn#SensingDevice"/>
        <rdfs:subClassOf>
            <owl:Restriction>
                <owl:onProperty rdf:resource="http://purl.org/iot/vocab/m3-lite#hasDomainOfInterest"/>
                <owl:someValuesFrom rdf:resource="http://purl.org/iot/vocab/m3-lite#Agriculture"/>
            </owl:Restriction>
        </rdfs:subClassOf>
        <rdfs:subClassOf>
            <owl:Restriction>
                <owl:onProperty rdf:resource="http://purl.org/iot/vocab/m3-lite#hasDomainOfInterest"/>
                <owl:someValuesFrom rdf:resource="http://purl.org/iot/vocab/m3-lite#Environment"/>
            </owl:Restriction>
        </rdfs:subClassOf>
        <rdfs:comment xml:lang="en">Device used to detect PH level.</rdfs:comment>
        <rdfs:label xml:lang="en">PH Sensor</rdfs:label>
    </owl:Class>
    


    <!-- http://purl.org/iot/vocab/m3-lite#PPM -->

    <owl:Class rdf:about="http://purl.org/iot/vocab/m3-lite#PPM">
        <rdfs:subClassOf rdf:resource="http://purl.org/NET/ssnx/qu/qu#Unit"/>
        <rdfs:comment xml:lang="en">It describes the concentration of something in water or soil.</rdfs:comment>
        <rdfs:label xml:lang="en">PPM (parts per million)</rdfs:label>
    </owl:Class>
    


    <!-- http://purl.org/iot/vocab/m3-lite#PartsPerBillion -->

    <owl:Class rdf:about="http://purl.org/iot/vocab/m3-lite#PartsPerBillion">
        <rdfs:subClassOf rdf:resource="http://purl.org/iot/vocab/m3-lite#PPM"/>
        <rdfs:comment xml:lang="en">It describes the concentration of something in parts per billion parts of water or soil, expressed in any (but common) unit of measurement.</rdfs:comment>
        <rdfs:label xml:lang="en">Parts Per Billion</rdfs:label>
    </owl:Class>
    


    <!-- http://purl.org/iot/vocab/m3-lite#Pascal -->

    <owl:Class rdf:about="http://purl.org/iot/vocab/m3-lite#Pascal">
        <rdfs:subClassOf rdf:resource="http://purl.org/NET/ssnx/qu/qu#Unit"/>
        <rdfs:comment xml:lang="en">Unit for pressure (e.g., atmospheric pressure).</rdfs:comment>
        <rdfs:label xml:lang="en">Pascal</rdfs:label>
    </owl:Class>
    


    <!-- http://purl.org/iot/vocab/m3-lite#Pedometer -->

    <owl:Class rdf:about="http://purl.org/iot/vocab/m3-lite#Pedometer">
        <rdfs:subClassOf rdf:resource="http://purl.oclc.org/NET/ssnx/ssn#SensingDevice"/>
        <rdfs:subClassOf>
            <owl:Restriction>
                <owl:onProperty rdf:resource="http://purl.org/iot/vocab/m3-lite#hasDomainOfInterest"/>
                <owl:someValuesFrom rdf:resource="http://purl.org/iot/vocab/m3-lite#Health"/>
            </owl:Restriction>
        </rdfs:subClassOf>
        <rdfs:comment xml:lang="en">Pedometer is used to count the number of steps when walking, running, etc.</rdfs:comment>
        <rdfs:label xml:lang="en">Pedometer</rdfs:label>
    </owl:Class>
    


    <!-- http://purl.org/iot/vocab/m3-lite#Percent -->

    <owl:Class rdf:about="http://purl.org/iot/vocab/m3-lite#Percent">
        <rdfs:subClassOf rdf:resource="http://purl.org/NET/ssnx/qu/qu#Unit"/>
        <rdfs:comment xml:lang="en">It is the amount in or for every hundred.</rdfs:comment>
        <rdfs:label xml:lang="en">Percent</rdfs:label>
        <rdfs:seeAlso rdf:resource="http://data.qudt.org/qudt/owl/1.0.0/unit.owl#Percent"/>
        <rdfs:seeAlso rdf:resource="http://sweet.jpl.nasa.gov/ontology/units.owl#percent"/>
    </owl:Class>
    


    <!-- http://purl.org/iot/vocab/m3-lite#Place -->

    <owl:Class rdf:about="http://purl.org/iot/vocab/m3-lite#Place">
        <rdfs:subClassOf rdf:resource="http://purl.org/iot/vocab/m3-lite#DomainOfInterest"/>
        <rdfs:comment xml:lang="en">Location, Place, GPS coordinates as an Internet of Things (IoT) applicative domain.</rdfs:comment>
        <rdfs:label xml:lang="en">Place DOI</rdfs:label>
    </owl:Class>
    


    <!-- http://purl.org/iot/vocab/m3-lite#Potassium -->

    <owl:Class rdf:about="http://purl.org/iot/vocab/m3-lite#Potassium">
        <rdfs:subClassOf rdf:resource="http://purl.org/NET/ssnx/qu/qu#QuantityKind"/>
        <rdfs:comment xml:lang="en">It is the measure of Blood Potassium Level.</rdfs:comment>
        <rdfs:label xml:lang="en">Potassium</rdfs:label>
    </owl:Class>
    


    <!-- http://purl.org/iot/vocab/m3-lite#Pound -->

    <owl:Class rdf:about="http://purl.org/iot/vocab/m3-lite#Pound">
        <rdfs:subClassOf rdf:resource="http://purl.org/iot/vocab/m3-lite#Gram"/>
        <rdfs:comment xml:lang="en">A unit of weight equal to 16 oz. 1 pound= 453.592 grams</rdfs:comment>
        <rdfs:label xml:lang="en">Pound</rdfs:label>
    </owl:Class>
    


    <!-- http://purl.org/iot/vocab/m3-lite#Power -->

    <owl:Class rdf:about="http://purl.org/iot/vocab/m3-lite#Power">
        <rdfs:subClassOf rdf:resource="http://purl.org/NET/ssnx/qu/qu#QuantityKind"/>
        <rdfs:comment xml:lang="en">It is the rate, per unit time, at which electrical energy is transferred by an electric circuit.</rdfs:comment>
        <rdfs:label xml:lang="en">Power</rdfs:label>
    </owl:Class>
    


    <!-- http://purl.org/iot/vocab/m3-lite#Precipitation -->

    <owl:Class rdf:about="http://purl.org/iot/vocab/m3-lite#Precipitation">
        <rdfs:subClassOf rdf:resource="http://purl.org/NET/ssnx/qu/qu#QuantityKind"/>
        <rdfs:comment xml:lang="en">It is any product of the condensation of atmospheric water vapour that falls under gravity.</rdfs:comment>
        <rdfs:label xml:lang="en">Precipitation</rdfs:label>
        <rdfs:seeAlso rdf:resource="http://archive.knoesis.org/research/semsci/application_domain/sem_sensor/ont/sensor-observation.owlPrecipitationProperty"/>
        <rdfs:seeAlso rdf:resource="http://paul.staroch.name/thesis/SmartHomeWeather.owl#Precipitation"/>
    </owl:Class>
    


    <!-- http://purl.org/iot/vocab/m3-lite#PrecipitationSensor -->

    <owl:Class rdf:about="http://purl.org/iot/vocab/m3-lite#PrecipitationSensor">
        <rdfs:subClassOf rdf:resource="http://purl.oclc.org/NET/ssnx/ssn#SensingDevice"/>
        <rdfs:subClassOf>
            <owl:Restriction>
                <owl:onProperty rdf:resource="http://purl.org/iot/vocab/m3-lite#hasDomainOfInterest"/>
                <owl:someValuesFrom rdf:resource="http://purl.org/iot/vocab/m3-lite#Agriculture"/>
            </owl:Restriction>
        </rdfs:subClassOf>
        <rdfs:subClassOf>
            <owl:Restriction>
                <owl:onProperty rdf:resource="http://purl.org/iot/vocab/m3-lite#hasDomainOfInterest"/>
                <owl:someValuesFrom rdf:resource="http://purl.org/iot/vocab/m3-lite#Weather"/>
            </owl:Restriction>
        </rdfs:subClassOf>
        <rdfs:comment xml:lang="en">It is a device measuring the amount of precipitation.</rdfs:comment>
        <rdfs:label xml:lang="en">Precipitation Sensor</rdfs:label>
        <rdfs:seeAlso rdf:resource="http://purl.oclc.org/NET/ssnx/meteo/aws#PrecipitationSensor"/>
    </owl:Class>
    


    <!-- http://purl.org/iot/vocab/m3-lite#Presence -->

    <owl:Class rdf:about="http://purl.org/iot/vocab/m3-lite#Presence">
        <rdfs:subClassOf rdf:resource="http://purl.org/NET/ssnx/qu/qu#QuantityKind"/>
        <rdfs:comment xml:lang="en">Measure to know if an object is present. It is usually boolean.</rdfs:comment>
        <rdfs:label xml:lang="en">Presence</rdfs:label>
    </owl:Class>
    


    <!-- http://purl.org/iot/vocab/m3-lite#PresenceDetector -->

    <owl:Class rdf:about="http://purl.org/iot/vocab/m3-lite#PresenceDetector">
        <rdfs:subClassOf rdf:resource="http://purl.oclc.org/NET/ssnx/ssn#SensingDevice"/>
        <rdfs:comment xml:lang="en">Device used to detect if on object is occupied or not.</rdfs:comment>
        <rdfs:label xml:lang="en">Presence Detector</rdfs:label>
        <rdfs:seeAlso rdf:resource="http://casas.wsu.edu/owl/cose.owl#PassiveInfraredSensor"/>
    </owl:Class>
    


    <!-- http://purl.org/iot/vocab/m3-lite#PresenceStateDriverCard -->

    <owl:Class rdf:about="http://purl.org/iot/vocab/m3-lite#PresenceStateDriverCard">
        <rdfs:subClassOf rdf:resource="http://purl.org/iot/vocab/m3-lite#Presence"/>
        <rdfs:comment xml:lang="en">Indicates the presence of the first driver card.</rdfs:comment>
        <rdfs:label xml:lang="en">Presence State Driver Card</rdfs:label>
    </owl:Class>
    


    <!-- http://purl.org/iot/vocab/m3-lite#PresenceStateDriverCard1 -->

    <owl:Class rdf:about="http://purl.org/iot/vocab/m3-lite#PresenceStateDriverCard1">
        <rdfs:subClassOf rdf:resource="http://purl.org/iot/vocab/m3-lite#PresenceStateDriverCard"/>
        <rdfs:comment xml:lang="en">Indicates the presence of the first driver card.</rdfs:comment>
        <rdfs:label xml:lang="en">Presence State Driver Card 1</rdfs:label>
    </owl:Class>
    


    <!-- http://purl.org/iot/vocab/m3-lite#PresenceStateDriverCard2 -->

    <owl:Class rdf:about="http://purl.org/iot/vocab/m3-lite#PresenceStateDriverCard2">
        <rdfs:subClassOf rdf:resource="http://purl.org/iot/vocab/m3-lite#PresenceStateDriverCard"/>
        <rdfs:comment xml:lang="en">Indicates the presence of the second driver card.</rdfs:comment>
        <rdfs:label xml:lang="en">Presence State Driver Card 2</rdfs:label>
    </owl:Class>
    


    <!-- http://purl.org/iot/vocab/m3-lite#PresenceStateEmergencyVehicle -->

    <owl:Class rdf:about="http://purl.org/iot/vocab/m3-lite#PresenceStateEmergencyVehicle">
        <rdfs:subClassOf rdf:resource="http://purl.org/iot/vocab/m3-lite#Presence"/>
        <rdfs:comment>The presence or absence of an emergency vehicle (ambulance, fire fighters, etc.).</rdfs:comment>
        <rdfs:label xml:lang="en">Presence State Emergency Vehicle</rdfs:label>
    </owl:Class>
    


    <!-- http://purl.org/iot/vocab/m3-lite#PresenceStateParking -->

    <owl:Class rdf:about="http://purl.org/iot/vocab/m3-lite#PresenceStateParking">
        <rdfs:subClassOf rdf:resource="http://purl.org/iot/vocab/m3-lite#Presence"/>
        <rdfs:comment>The presence or absence of a vehicle parked.</rdfs:comment>
        <rdfs:label xml:lang="en">Presence State Parking</rdfs:label>
    </owl:Class>
    


    <!-- http://purl.org/iot/vocab/m3-lite#PresenceStatePeople -->

    <owl:Class rdf:about="http://purl.org/iot/vocab/m3-lite#PresenceStatePeople">
        <rdfs:subClassOf rdf:resource="http://purl.org/iot/vocab/m3-lite#Presence"/>
        <rdfs:comment>The presence or absence of people passing.</rdfs:comment>
        <rdfs:label xml:lang="en">Presence State People</rdfs:label>
    </owl:Class>
    


    <!-- http://purl.org/iot/vocab/m3-lite#Pressure -->

    <owl:Class rdf:about="http://purl.org/iot/vocab/m3-lite#Pressure">
        <rdfs:subClassOf rdf:resource="http://purl.org/NET/ssnx/qu/qu#QuantityKind"/>
        <rdfs:comment xml:lang="en">It is the physical force exerted on or against an object by something in contact with it.</rdfs:comment>
        <rdfs:label xml:lang="en">Pressure</rdfs:label>
        <rdfs:seeAlso rdf:resource="http://archive.knoesis.org/research/semsci/application_domain/sem_sensor/ont/sensor-observation.owlPressureProperty"/>
    </owl:Class>
    


    <!-- http://purl.org/iot/vocab/m3-lite#PressureSensor -->

    <owl:Class rdf:about="http://purl.org/iot/vocab/m3-lite#PressureSensor">
        <rdfs:subClassOf rdf:resource="http://purl.oclc.org/NET/ssnx/ssn#SensingDevice"/>
        <rdfs:subClassOf>
            <owl:Restriction>
                <owl:onProperty rdf:resource="http://purl.org/iot/vocab/m3-lite#hasDomainOfInterest"/>
                <owl:someValuesFrom rdf:resource="http://purl.org/iot/vocab/m3-lite#BuildingAutomation"/>
            </owl:Restriction>
        </rdfs:subClassOf>
        <rdfs:comment xml:lang="en">A device used to detect pressure. For example, it can be attached on the bed to infer if the user is lying, sleeping, sitting, bed occupancy, etc.</rdfs:comment>
        <rdfs:label xml:lang="en">Pressure Sensor</rdfs:label>
    </owl:Class>
    


    <!-- http://purl.org/iot/vocab/m3-lite#Proximity -->

    <owl:Class rdf:about="http://purl.org/iot/vocab/m3-lite#Proximity">
        <rdfs:subClassOf rdf:resource="http://purl.org/NET/ssnx/qu/qu#QuantityKind"/>
        <rdfs:comment xml:lang="en">Measure to detect proximity.</rdfs:comment>
        <rdfs:label xml:lang="en">Proximity</rdfs:label>
    </owl:Class>
    


    <!-- http://purl.org/iot/vocab/m3-lite#ProximitySensor -->

    <owl:Class rdf:about="http://purl.org/iot/vocab/m3-lite#ProximitySensor">
        <rdfs:subClassOf rdf:resource="http://purl.oclc.org/NET/ssnx/ssn#SensingDevice"/>
        <rdfs:comment xml:lang="en">Detect if something is within proximity of a sensor.</rdfs:comment>
        <rdfs:label xml:lang="en">Proximity Sensor</rdfs:label>
    </owl:Class>
    


    <!-- http://purl.org/iot/vocab/m3-lite#PublicTransit -->

    <owl:Class rdf:about="http://purl.org/iot/vocab/m3-lite#PublicTransit">
        <rdfs:subClassOf rdf:resource="http://purl.org/iot/vocab/m3-lite#SoundSource"/>
        <rdfs:comment xml:lang="en">When the source of the sound was Public transit.</rdfs:comment>
        <rdfs:label xml:lang="en">Public Transit</rdfs:label>
    </owl:Class>
    


    <!-- http://purl.org/iot/vocab/m3-lite#PulseOxymeter -->

    <owl:Class rdf:about="http://purl.org/iot/vocab/m3-lite#PulseOxymeter">
        <rdfs:subClassOf rdf:resource="http://purl.oclc.org/NET/ssnx/ssn#SensingDevice"/>
        <rdfs:subClassOf>
            <owl:Restriction>
                <owl:onProperty rdf:resource="http://purl.org/iot/vocab/m3-lite#hasDomainOfInterest"/>
                <owl:someValuesFrom rdf:resource="http://purl.org/iot/vocab/m3-lite#Health"/>
            </owl:Restriction>
        </rdfs:subClassOf>
        <rdfs:comment xml:lang="en">Pulse Oxymeter, SpO2, Blood Oxygen Saturation Sensor are used to measure the concentration of oxygen in the blood.</rdfs:comment>
        <rdfs:label xml:lang="en">Pulse Oxymeter</rdfs:label>
    </owl:Class>
    


    <!-- http://purl.org/iot/vocab/m3-lite#QRCode -->

    <owl:Class rdf:about="http://purl.org/iot/vocab/m3-lite#QRCode">
        <rdfs:subClassOf rdf:resource="http://purl.oclc.org/NET/UNIS/fiware/iot-lite#TagDevice"/>
        <rdfs:comment xml:lang="en">A tagging device can be QRCode.</rdfs:comment>
        <rdfs:label xml:lang="en">QR Code tagging Device</rdfs:label>
    </owl:Class>
    


    <!-- http://purl.org/iot/vocab/m3-lite#RFID -->

    <owl:Class rdf:about="http://purl.org/iot/vocab/m3-lite#RFID">
        <rdfs:subClassOf rdf:resource="http://purl.oclc.org/NET/UNIS/fiware/iot-lite#TagDevice"/>
        <rdfs:comment xml:lang="en">A tagging device can be RFID.</rdfs:comment>
        <rdfs:label xml:lang="en">RFID Tagging Device</rdfs:label>
    </owl:Class>
    


    <!-- http://purl.org/iot/vocab/m3-lite#Radian -->

    <owl:Class rdf:about="http://purl.org/iot/vocab/m3-lite#Radian">
        <rdfs:subClassOf rdf:resource="http://purl.org/NET/ssnx/qu/qu#Unit"/>
        <rdfs:comment xml:lang="en">The radian is a unit of angular measure defined such that an angle of one radian subtended from the centre of a unit circle produces an arc with arc length 1.</rdfs:comment>
        <rdfs:label xml:lang="en">Radian</rdfs:label>
        <rdfs:seeAlso rdf:resource="http://sweet.jpl.nasa.gov/ontology/units.owl#radian"/>
    </owl:Class>
    


    <!-- http://purl.org/iot/vocab/m3-lite#RadianPerSecond -->

    <owl:Class rdf:about="http://purl.org/iot/vocab/m3-lite#RadianPerSecond">
        <rdfs:subClassOf rdf:resource="http://purl.org/NET/ssnx/qu/qu#Unit"/>
        <rdfs:comment xml:lang="en">The radian per second is defined as the change in the orientation of an object, in radians, every second. The radian per second is the SI unit of angular (rotational) speed.</rdfs:comment>
        <rdfs:label xml:lang="en">Radian Per Second</rdfs:label>
        <rdfs:seeAlso>http://purl.oclc.org/NET/ssnx/qu/unit#radianPerSecond</rdfs:seeAlso>
    </owl:Class>
    


    <!-- http://purl.org/iot/vocab/m3-lite#RadiationParticleDetector -->

    <owl:Class rdf:about="http://purl.org/iot/vocab/m3-lite#RadiationParticleDetector">
        <rdfs:subClassOf rdf:resource="http://purl.oclc.org/NET/ssnx/ssn#SensingDevice"/>
        <rdfs:comment xml:lang="en">A particle detector, also known as a radiation detector or Geiger counter, is a device used to detect, track, and/or identify ionising particles, such as those produced by nuclear decay, cosmic radiation, or reactions in a particle accelerator.</rdfs:comment>
        <rdfs:label xml:lang="en">Radiation Particle Detector</rdfs:label>
    </owl:Class>
    


    <!-- http://purl.org/iot/vocab/m3-lite#RadiationParticlesPerMinute -->

    <owl:Class rdf:about="http://purl.org/iot/vocab/m3-lite#RadiationParticlesPerMinute">
        <rdfs:subClassOf rdf:resource="http://purl.org/NET/ssnx/qu/qu#Unit"/>
        <rdfs:comment xml:lang="en">The number of ionizing events detected in one minute.</rdfs:comment>
        <rdfs:label xml:lang="en">Radiation Particles Per Minute</rdfs:label>
    </owl:Class>
    


    <!-- http://purl.org/iot/vocab/m3-lite#Rainfall -->

    <owl:Class rdf:about="http://purl.org/iot/vocab/m3-lite#Rainfall">
        <rdfs:subClassOf rdf:resource="http://purl.org/NET/ssnx/qu/qu#QuantityKind"/>
        <rdfs:comment xml:lang="en">The depth of precipitation (water-equivalent) that accumulated over a measurement time quantity.</rdfs:comment>
        <rdfs:label xml:lang="en">Rainfall</rdfs:label>
        <rdfs:seeAlso>http://sweet.jpl.nasa.gov/ontology/property.owl#Rainfall</rdfs:seeAlso>
    </owl:Class>
    


    <!-- http://purl.org/iot/vocab/m3-lite#ReactivePower -->

    <owl:Class rdf:about="http://purl.org/iot/vocab/m3-lite#ReactivePower">
        <rdfs:subClassOf rdf:resource="http://purl.org/iot/vocab/m3-lite#Power"/>
        <rdfs:comment xml:lang="en">The portion of electricity that establishes and sustains the electric and magnetic fields of alternating-current equipment.</rdfs:comment>
        <rdfs:label xml:lang="en">Reactive Power</rdfs:label>
        <rdfs:seeAlso>http://purl.oclc.org/NET/ssnx/qu/dim#ReactivePower</rdfs:seeAlso>
    </owl:Class>
    


    <!-- http://purl.org/iot/vocab/m3-lite#RecognizedActivity -->

    <owl:Class rdf:about="http://purl.org/iot/vocab/m3-lite#RecognizedActivity">
        <rdfs:subClassOf rdf:resource="http://purl.org/NET/ssnx/qu/qu#QuantityKind"/>
        <rdfs:comment xml:lang="en">Activity Recognized. This is usually made available as a part of analysis done by Google. The available activities recognized are IN_VEHICLE, ON_BICYCLE, ON_FOOT, RUNNING, STILL, TILTING, UNKNOWN, and WALKING.</rdfs:comment>
        <rdfs:label xml:lang="en">Recognized Activity</rdfs:label>
    </owl:Class>
    


    <!-- http://purl.org/iot/vocab/m3-lite#RelativeHumidity -->

    <owl:Class rdf:about="http://purl.org/iot/vocab/m3-lite#RelativeHumidity">
        <rdfs:subClassOf rdf:resource="http://purl.org/NET/ssnx/qu/qu#QuantityKind"/>
        <rdfs:comment xml:lang="en">The ratio of vapour pressure to saturation vapour pressure, where vapour pressure is the pressure exerted by the molecules of water vapour and saturation vapour pressure is the pressure exerted by molecules of water vapour in AIR that has attained saturation.</rdfs:comment>
        <rdfs:label xml:lang="en">Relative Humidity</rdfs:label>
        <rdfs:seeAlso>http://sweet.jpl.nasa.gov/ontology/property.owl#RelativeHumidity</rdfs:seeAlso>
    </owl:Class>
    


    <!-- http://purl.org/iot/vocab/m3-lite#ResAverageLicConnectedUsers -->

    <owl:Class rdf:about="http://purl.org/iot/vocab/m3-lite#ResAverageLicConnectedUsers">
        <rdfs:subClassOf rdf:resource="http://purl.org/iot/vocab/m3-lite#Communication"/>
        <rdfs:comment xml:lang="en">Connected Users to a communication channel/platform</rdfs:comment>
        <rdfs:label xml:lang="en">Connected Users</rdfs:label>
    </owl:Class>
    


    <!-- http://purl.org/iot/vocab/m3-lite#RetERabDrop -->

    <owl:Class rdf:about="http://purl.org/iot/vocab/m3-lite#RetERabDrop">
        <rdfs:subClassOf rdf:resource="http://purl.org/iot/vocab/m3-lite#Communication"/>
        <rdfs:comment xml:lang="en">ERAB Drop.</rdfs:comment>
        <rdfs:label xml:lang="en">ERAB Drop</rdfs:label>
    </owl:Class>
    


    <!-- http://purl.org/iot/vocab/m3-lite#RevolutionsPerMinute -->

    <owl:Class rdf:about="http://purl.org/iot/vocab/m3-lite#RevolutionsPerMinute">
        <rdfs:subClassOf rdf:resource="http://purl.org/NET/ssnx/qu/qu#Unit"/>
        <rdfs:comment>Revolutions per minute (abbreviated rpm, RPM, rev/min, r/min) is a measure of the frequency of rotation, specifically the number of rotations around a fixed axis in one minute. It is used as a measure of rotational speed of a mechanical component.</rdfs:comment>
        <rdfs:label xml:lang="en">Revolutions Per Minute</rdfs:label>
    </owl:Class>
    


    <!-- http://purl.org/iot/vocab/m3-lite#RoadOccupancy -->

    <owl:Class rdf:about="http://purl.org/iot/vocab/m3-lite#RoadOccupancy">
        <rdfs:subClassOf rdf:resource="http://purl.org/NET/ssnx/qu/qu#QuantityKind"/>
        <rdfs:comment>Ratio of time on which a road lane section is occupied by vehicles within a given period of time.</rdfs:comment>
        <rdfs:label xml:lang="en">Road Occupancy</rdfs:label>
    </owl:Class>
    


    <!-- http://purl.org/iot/vocab/m3-lite#RoadSurfaceThermometer -->

    <owl:Class rdf:about="http://purl.org/iot/vocab/m3-lite#RoadSurfaceThermometer">
        <rdfs:subClassOf rdf:resource="http://purl.org/iot/vocab/m3-lite#Thermometer"/>
        <rdfs:subClassOf>
            <owl:Restriction>
                <owl:onProperty rdf:resource="http://purl.org/iot/vocab/m3-lite#hasDomainOfInterest"/>
                <owl:someValuesFrom rdf:resource="http://purl.org/iot/vocab/m3-lite#Transportation"/>
            </owl:Restriction>
        </rdfs:subClassOf>
        <rdfs:comment xml:lang="en">Device used to measure the road Surface temperature.</rdfs:comment>
        <rdfs:label xml:lang="en">Road Surface Thermometer</rdfs:label>
    </owl:Class>
    


    <!-- http://purl.org/iot/vocab/m3-lite#RoadTemperature -->

    <owl:Class rdf:about="http://purl.org/iot/vocab/m3-lite#RoadTemperature">
        <rdfs:subClassOf rdf:resource="http://purl.org/iot/vocab/m3-lite#Temperature"/>
        <rdfs:comment xml:lang="en">Temperature of the road.</rdfs:comment>
        <rdfs:label xml:lang="en">Road Temperature</rdfs:label>
    </owl:Class>
    


    <!-- http://purl.org/iot/vocab/m3-lite#RoomTemperature -->

    <owl:Class rdf:about="http://purl.org/iot/vocab/m3-lite#RoomTemperature">
        <rdfs:subClassOf rdf:resource="http://purl.org/iot/vocab/m3-lite#BuildingTemperature"/>
        <rdfs:comment xml:lang="en">Temperature of a room.</rdfs:comment>
        <rdfs:label xml:lang="en">Room Temperature</rdfs:label>
        <rdfs:seeAlso rdf:resource="http://elite.polito.it/ontologies/dogont.owl#TemperatureMeasurementMNotification"/>
        <rdfs:seeAlso rdf:resource="http://sensormeasurement.appspot.com/home#RoomTemperature"/>
    </owl:Class>
    


    <!-- http://purl.org/iot/vocab/m3-lite#RotationalSpeed -->

    <owl:Class rdf:about="http://purl.org/iot/vocab/m3-lite#RotationalSpeed">
        <rdfs:subClassOf rdf:resource="http://purl.org/NET/ssnx/qu/qu#QuantityKind"/>
        <rdfs:comment xml:lang="en">Rotational speed (or speed of revolution) of an object rotating around an axis is the number of turns of the object divided by time, specified as revolutions per minute (rpm), revolutions per second (rev/s), or radians per second (rad/s). (Source Wikipedia)</rdfs:comment>
        <rdfs:label xml:lang="en">Rotational Speed</rdfs:label>
    </owl:Class>
    


    <!-- http://purl.org/iot/vocab/m3-lite#RotationalSpeedEngine -->

    <owl:Class rdf:about="http://purl.org/iot/vocab/m3-lite#RotationalSpeedEngine">
        <rdfs:subClassOf rdf:resource="http://purl.org/iot/vocab/m3-lite#RotationalSpeed"/>
        <rdfs:comment xml:lang="en">Rotational speed is a property that is the rate of rotation of a material around an axis, in this case the engine cylinders.</rdfs:comment>
        <rdfs:label xml:lang="en">Rotational Speed Engine</rdfs:label>
        <rdfs:seeAlso>http://purl.oclc.org/NET/ssnx/qu/quantity#rotationalSpeed</rdfs:seeAlso>
    </owl:Class>
    


    <!-- http://purl.org/iot/vocab/m3-lite#SO2Sensor -->

    <owl:Class rdf:about="http://purl.org/iot/vocab/m3-lite#SO2Sensor">
        <rdfs:subClassOf rdf:resource="http://purl.org/iot/vocab/m3-lite#GaseousPollutantSensor"/>
        <rdfs:comment xml:lang="en">Device use to detect Sulphur Dioxide (SO2) level in the environment.</rdfs:comment>
        <rdfs:label xml:lang="en">Sulphur Dioxide (SO2) Sensor</rdfs:label>
    </owl:Class>
    


    <!-- http://purl.org/iot/vocab/m3-lite#SPO2 -->

    <owl:Class rdf:about="http://purl.org/iot/vocab/m3-lite#SPO2">
        <rdfs:subClassOf rdf:resource="http://purl.org/NET/ssnx/qu/qu#QuantityKind"/>
        <rdfs:comment xml:lang="en">It is a measure of the amount of oxygenated haemoglobin in the blood.</rdfs:comment>
        <rdfs:label xml:lang="en">SPO2</rdfs:label>
    </owl:Class>
    


    <!-- http://purl.org/iot/vocab/m3-lite#Salinity -->

    <owl:Class rdf:about="http://purl.org/iot/vocab/m3-lite#Salinity">
        <rdfs:subClassOf rdf:resource="http://purl.org/NET/ssnx/qu/qu#QuantityKind"/>
        <rdfs:comment xml:lang="en">It is the measure of all the salts dissolved in water.</rdfs:comment>
        <rdfs:label xml:lang="en">Salinity</rdfs:label>
    </owl:Class>
    


    <!-- http://purl.org/iot/vocab/m3-lite#SaltMeter -->

    <owl:Class rdf:about="http://purl.org/iot/vocab/m3-lite#SaltMeter">
        <rdfs:subClassOf rdf:resource="http://purl.oclc.org/NET/ssnx/ssn#SensingDevice"/>
        <rdfs:subClassOf>
            <owl:Restriction>
                <owl:onProperty rdf:resource="http://purl.org/iot/vocab/m3-lite#hasDomainOfInterest"/>
                <owl:someValuesFrom rdf:resource="http://purl.org/iot/vocab/m3-lite#Environment"/>
            </owl:Restriction>
        </rdfs:subClassOf>
        <rdfs:comment xml:lang="en">Device use to detect salinity of water.</rdfs:comment>
        <rdfs:label xml:lang="en">Salt Meter</rdfs:label>
    </owl:Class>
    


    <!-- http://purl.org/iot/vocab/m3-lite#Scale -->

    <owl:Class rdf:about="http://purl.org/iot/vocab/m3-lite#Scale">
        <rdfs:subClassOf rdf:resource="http://purl.org/NET/ssnx/qu/qu#Unit"/>
        <rdfs:comment xml:lang="en">Arbitrary indirect reference which should be translated into meaningful measurements by using the corresponding decoding algorithm detailed in the resource description. In this case the returned values are part of a continuous variable which can take any numeric value.</rdfs:comment>
        <rdfs:label xml:lang="en">Scale</rdfs:label>
    </owl:Class>
    


    <!-- http://purl.org/iot/vocab/m3-lite#SeatBeltTensionSensor -->

    <owl:Class rdf:about="http://purl.org/iot/vocab/m3-lite#SeatBeltTensionSensor">
        <rdfs:subClassOf rdf:resource="http://purl.oclc.org/NET/UNIS/fiware/iot-lite#ActuatingDevice"/>
        <rdfs:subClassOf>
            <owl:Restriction>
                <owl:onProperty rdf:resource="http://purl.org/iot/vocab/m3-lite#hasDomainOfInterest"/>
                <owl:someValuesFrom rdf:resource="http://purl.org/iot/vocab/m3-lite#Transportation"/>
            </owl:Restriction>
        </rdfs:subClassOf>
        <rdfs:comment xml:lang="en"> Actuator used to turn Seat Belt Tension Actuator on or off. </rdfs:comment>
        <rdfs:label xml:lang="en">Seat Belt Tension Actuating Device</rdfs:label>
    </owl:Class>
    


    <!-- http://purl.org/iot/vocab/m3-lite#SecondAngle -->

    <owl:Class rdf:about="http://purl.org/iot/vocab/m3-lite#SecondAngle">
        <rdfs:subClassOf rdf:resource="http://purl.org/NET/ssnx/qu/qu#Unit"/>
        <rdfs:comment xml:lang="en">It is a unit of angular measurement equal to 1/60 of one degree.</rdfs:comment>
        <rdfs:label xml:lang="en">Second Angle</rdfs:label>
    </owl:Class>
    


    <!-- http://purl.org/iot/vocab/m3-lite#SecondTime -->

    <owl:Class rdf:about="http://purl.org/iot/vocab/m3-lite#SecondTime">
        <rdfs:subClassOf rdf:resource="http://purl.org/NET/ssnx/qu/qu#Unit"/>
        <rdfs:comment xml:lang="en">Qualitatively defined as the second division of the hour by sixty, the first division by sixty being the minute. SI definition of second is &quot;the duration of 9 192 631 770 periods of the radiation corresponding to the transition between the two hyperfine levels of the ground state of the cesium 133 atom.</rdfs:comment>
        <rdfs:label xml:lang="en">Second Time</rdfs:label>
    </owl:Class>
    


    <!-- http://purl.org/iot/vocab/m3-lite#Seismometer -->

    <owl:Class rdf:about="http://purl.org/iot/vocab/m3-lite#Seismometer">
        <rdfs:subClassOf rdf:resource="http://purl.oclc.org/NET/ssnx/ssn#SensingDevice"/>
        <rdfs:comment xml:lang="en">Seismometers are instruments that measure motions of the ground, including those of seismic waves generated by earthquakes, volcanic eruptions, and other seismic sources.</rdfs:comment>
        <rdfs:label xml:lang="en">Seismometer</rdfs:label>
    </owl:Class>
    


    <!-- http://purl.org/iot/vocab/m3-lite#ShakeSensor -->

    <owl:Class rdf:about="http://purl.org/iot/vocab/m3-lite#ShakeSensor">
        <rdfs:subClassOf rdf:resource="http://purl.oclc.org/NET/ssnx/ssn#SensingDevice"/>
        <rdfs:subClassOf>
            <owl:Restriction>
                <owl:onProperty rdf:resource="http://purl.org/iot/vocab/m3-lite#hasDomainOfInterest"/>
                <owl:someValuesFrom rdf:resource="http://purl.org/iot/vocab/m3-lite#Environment"/>
            </owl:Restriction>
        </rdfs:subClassOf>
        <rdfs:subClassOf>
            <owl:Restriction>
                <owl:onProperty rdf:resource="http://purl.org/iot/vocab/m3-lite#hasDomainOfInterest"/>
                <owl:someValuesFrom rdf:resource="http://purl.org/iot/vocab/m3-lite#Transportation"/>
            </owl:Restriction>
        </rdfs:subClassOf>
        <rdfs:comment xml:lang="en">Shake sensor is used to deduce the quality of the road, earthquakes.</rdfs:comment>
        <rdfs:label xml:lang="en">Shake Sensor</rdfs:label>
        <rdfs:seeAlso rdf:resource="http://casas.wsu.edu/owl/cose.owl#ShakeSensor"/>
    </owl:Class>
    


    <!-- http://purl.org/iot/vocab/m3-lite#Shower -->

    <owl:Class rdf:about="http://purl.org/iot/vocab/m3-lite#Shower">
        <rdfs:subClassOf rdf:resource="http://purl.oclc.org/NET/UNIS/fiware/iot-lite#ActuatingDevice"/>
        <rdfs:subClassOf>
            <owl:Restriction>
                <owl:onProperty rdf:resource="http://purl.org/iot/vocab/m3-lite#hasDomainOfInterest"/>
                <owl:someValuesFrom rdf:resource="http://purl.org/iot/vocab/m3-lite#BuildingAutomation"/>
            </owl:Restriction>
        </rdfs:subClassOf>
        <rdfs:comment xml:lang="en">An actuator to automatically switch on/off the shower.</rdfs:comment>
        <rdfs:label xml:lang="en">Shower Actuating Device</rdfs:label>
    </owl:Class>
    


    <!-- http://purl.org/iot/vocab/m3-lite#SiemensPerMetre -->

    <owl:Class rdf:about="http://purl.org/iot/vocab/m3-lite#SiemensPerMetre">
        <rdfs:subClassOf rdf:resource="http://purl.org/NET/ssnx/qu/qu#Unit"/>
        <rdfs:comment xml:lang="en">Conductivity is measured in Siemens per metre (S/m).</rdfs:comment>
        <rdfs:label xml:lang="en">Siemens Per Metre, Siemens Per Meter</rdfs:label>
    </owl:Class>
    


    <!-- http://purl.org/iot/vocab/m3-lite#Sink -->

    <owl:Class rdf:about="http://purl.org/iot/vocab/m3-lite#Sink">
        <rdfs:subClassOf rdf:resource="http://purl.oclc.org/NET/UNIS/fiware/iot-lite#ActuatingDevice"/>
        <rdfs:subClassOf>
            <owl:Restriction>
                <owl:onProperty rdf:resource="http://purl.org/iot/vocab/m3-lite#hasDomainOfInterest"/>
                <owl:someValuesFrom rdf:resource="http://purl.org/iot/vocab/m3-lite#BuildingAutomation"/>
            </owl:Restriction>
        </rdfs:subClassOf>
        <rdfs:comment xml:lang="en">An actuator to automatically switch on/off the sink.</rdfs:comment>
        <rdfs:label xml:lang="en">Sink Actuating Device</rdfs:label>
    </owl:Class>
    


    <!-- http://purl.org/iot/vocab/m3-lite#Sirens -->

    <owl:Class rdf:about="http://purl.org/iot/vocab/m3-lite#Sirens">
        <rdfs:subClassOf rdf:resource="http://purl.org/iot/vocab/m3-lite#SoundSource"/>
        <rdfs:comment xml:lang="en">When source of the sound were sirens either from ambulance, police car or factory etc.</rdfs:comment>
        <rdfs:label xml:lang="en">Sirens Sound Source</rdfs:label>
    </owl:Class>
    


    <!-- http://purl.org/iot/vocab/m3-lite#SkinConductance -->

    <owl:Class rdf:about="http://purl.org/iot/vocab/m3-lite#SkinConductance">
        <rdfs:subClassOf rdf:resource="http://purl.org/NET/ssnx/qu/qu#QuantityKind"/>
        <rdfs:comment xml:lang="en">Electroderal activity (also known as skin conductance or galvanic skin response) directly correlates to the sympathetic nervous system activity and thus provides a powerful tool for monitoring arousal and certain aspects of autonomic regulation.</rdfs:comment>
        <rdfs:label xml:lang="en">Skin conductance, GSR</rdfs:label>
    </owl:Class>
    


    <!-- http://purl.org/iot/vocab/m3-lite#SkinConductanceSensor -->

    <owl:Class rdf:about="http://purl.org/iot/vocab/m3-lite#SkinConductanceSensor">
        <rdfs:subClassOf rdf:resource="http://purl.oclc.org/NET/ssnx/ssn#SensingDevice"/>
        <rdfs:subClassOf>
            <owl:Restriction>
                <owl:onProperty rdf:resource="http://purl.org/iot/vocab/m3-lite#hasDomainOfInterest"/>
                <owl:someValuesFrom rdf:resource="http://purl.org/iot/vocab/m3-lite#Emotion"/>
            </owl:Restriction>
        </rdfs:subClassOf>
        <rdfs:subClassOf>
            <owl:Restriction>
                <owl:onProperty rdf:resource="http://purl.org/iot/vocab/m3-lite#hasDomainOfInterest"/>
                <owl:someValuesFrom rdf:resource="http://purl.org/iot/vocab/m3-lite#Health"/>
            </owl:Restriction>
        </rdfs:subClassOf>
        <rdfs:comment xml:lang="en">Device used to detect Skin Conductance.</rdfs:comment>
        <rdfs:label xml:lang="en">Skin Conductance Sensor</rdfs:label>
    </owl:Class>
    


    <!-- http://purl.org/iot/vocab/m3-lite#SmokeDetector -->

    <owl:Class rdf:about="http://purl.org/iot/vocab/m3-lite#SmokeDetector">
        <rdfs:subClassOf rdf:resource="http://purl.oclc.org/NET/ssnx/ssn#SensingDevice"/>
        <rdfs:subClassOf>
            <owl:Restriction>
                <owl:onProperty rdf:resource="http://purl.org/iot/vocab/m3-lite#hasDomainOfInterest"/>
                <owl:someValuesFrom rdf:resource="http://purl.org/iot/vocab/m3-lite#BuildingAutomation"/>
            </owl:Restriction>
        </rdfs:subClassOf>
        <rdfs:comment xml:lang="en">Device used to detect if there is a fire or the smoke.</rdfs:comment>
        <rdfs:label xml:lang="en">Smoke Detector</rdfs:label>
        <rdfs:seeAlso rdf:resource="http://casas.wsu.edu/owl/cose.owl#SmokeAlarm"/>
    </owl:Class>
    


    <!-- http://purl.org/iot/vocab/m3-lite#SnowChains -->

    <owl:Class rdf:about="http://purl.org/iot/vocab/m3-lite#SnowChains">
        <rdfs:subClassOf rdf:resource="http://purl.oclc.org/NET/UNIS/fiware/iot-lite#ActuatingDevice"/>
        <rdfs:subClassOf>
            <owl:Restriction>
                <owl:onProperty rdf:resource="http://purl.org/iot/vocab/m3-lite#hasDomainOfInterest"/>
                <owl:someValuesFrom rdf:resource="http://purl.org/iot/vocab/m3-lite#Transportation"/>
            </owl:Restriction>
        </rdfs:subClassOf>
        <rdfs:comment xml:lang="en">The actuator that turn Snow chains on/off.</rdfs:comment>
        <rdfs:label xml:lang="en">Snow Chains Actuating Device</rdfs:label>
    </owl:Class>
    


    <!-- http://purl.org/iot/vocab/m3-lite#Sodium -->

    <owl:Class rdf:about="http://purl.org/iot/vocab/m3-lite#Sodium">
        <rdfs:subClassOf rdf:resource="http://purl.org/NET/ssnx/qu/qu#QuantityKind"/>
        <rdfs:comment xml:lang="en">Measure of Blood Sodium level.</rdfs:comment>
        <rdfs:label xml:lang="en">Sodium</rdfs:label>
    </owl:Class>
    


    <!-- http://purl.org/iot/vocab/m3-lite#SoilHumidity -->

    <owl:Class rdf:about="http://purl.org/iot/vocab/m3-lite#SoilHumidity">
        <rdfs:subClassOf rdf:resource="http://purl.org/NET/ssnx/qu/qu#QuantityKind"/>
        <rdfs:comment xml:lang="en">It is the quantity of water contained in a material, such as soil. </rdfs:comment>
        <rdfs:label xml:lang="en">Soil Humidity</rdfs:label>
    </owl:Class>
    


    <!-- http://purl.org/iot/vocab/m3-lite#SoilHumiditySensor -->

    <owl:Class rdf:about="http://purl.org/iot/vocab/m3-lite#SoilHumiditySensor">
        <rdfs:subClassOf rdf:resource="http://purl.org/iot/vocab/m3-lite#HumiditySensor"/>
        <rdfs:subClassOf>
            <owl:Restriction>
                <owl:onProperty rdf:resource="http://purl.org/iot/vocab/m3-lite#hasDomainOfInterest"/>
                <owl:someValuesFrom rdf:resource="http://purl.org/iot/vocab/m3-lite#Agriculture"/>
            </owl:Restriction>
        </rdfs:subClassOf>
        <rdfs:comment xml:lang="en">Soil Humidity sensor, Soil moisture, Hygrometer are an instrument used for measuring the soil moisture or soil humidity.</rdfs:comment>
        <rdfs:label xml:lang="en">Soil Humidity Sensor</rdfs:label>
    </owl:Class>
    


    <!-- http://purl.org/iot/vocab/m3-lite#SoilMoistureTension -->

    <owl:Class rdf:about="http://purl.org/iot/vocab/m3-lite#SoilMoistureTension">
        <rdfs:subClassOf rdf:resource="http://purl.org/NET/ssnx/qu/qu#QuantityKind"/>
        <rdfs:comment xml:lang="en">The force per unit area required to remove film water from soil.</rdfs:comment>
        <rdfs:label xml:lang="en">Soil Moisture Tension</rdfs:label>
    </owl:Class>
    


    <!-- http://purl.org/iot/vocab/m3-lite#SoilTemperature -->

    <owl:Class rdf:about="http://purl.org/iot/vocab/m3-lite#SoilTemperature">
        <rdfs:subClassOf rdf:resource="http://purl.org/iot/vocab/m3-lite#Temperature"/>
        <rdfs:comment xml:lang="en">Soil temperature is the bulk temperature of the soil, not the surface (skin) temperature.</rdfs:comment>
        <rdfs:label xml:lang="en">Soil Temperature</rdfs:label>
    </owl:Class>
    


    <!-- http://purl.org/iot/vocab/m3-lite#SoilThermometer -->

    <owl:Class rdf:about="http://purl.org/iot/vocab/m3-lite#SoilThermometer">
        <rdfs:subClassOf rdf:resource="http://purl.org/iot/vocab/m3-lite#Thermometer"/>
        <rdfs:comment xml:lang="en">This sensor reports Soil temperature.</rdfs:comment>
        <rdfs:label xml:lang="en">Soil Thermometer</rdfs:label>
    </owl:Class>
    


    <!-- http://purl.org/iot/vocab/m3-lite#SolarRadiation -->

    <owl:Class rdf:about="http://purl.org/iot/vocab/m3-lite#SolarRadiation">
        <rdfs:subClassOf rdf:resource="http://purl.org/NET/ssnx/qu/qu#QuantityKind"/>
        <rdfs:comment xml:lang="en">It is the power per unit area received from the Sun in the form of electromagnetic radiation in the wavelength range of the measuring instrument. (Source Wikipedia).</rdfs:comment>
        <rdfs:label xml:lang="en">Solar Radiation Measurement, PAR Measurement (Photosynthetically Active Radiation)</rdfs:label>
    </owl:Class>
    


    <!-- http://purl.org/iot/vocab/m3-lite#SolarRadiationSensor -->

    <owl:Class rdf:about="http://purl.org/iot/vocab/m3-lite#SolarRadiationSensor">
        <rdfs:subClassOf rdf:resource="http://purl.oclc.org/NET/ssnx/ssn#SensingDevice"/>
        <rdfs:subClassOf>
            <owl:Restriction>
                <owl:onProperty rdf:resource="http://purl.org/iot/vocab/m3-lite#hasDomainOfInterest"/>
                <owl:someValuesFrom rdf:resource="http://purl.org/iot/vocab/m3-lite#Agriculture"/>
            </owl:Restriction>
        </rdfs:subClassOf>
        <rdfs:subClassOf>
            <owl:Restriction>
                <owl:onProperty rdf:resource="http://purl.org/iot/vocab/m3-lite#hasDomainOfInterest"/>
                <owl:someValuesFrom rdf:resource="http://purl.org/iot/vocab/m3-lite#Weather"/>
            </owl:Restriction>
        </rdfs:subClassOf>
        <rdfs:comment xml:lang="en">Device used to detect Solar Radiation.</rdfs:comment>
        <rdfs:label xml:lang="en">Solar Radiation Sensor</rdfs:label>
        <rdfs:seeAlso rdf:resource="http://purl.oclc.org/NET/ssnx/meteo/aws#RadiationSensor"/>
        <rdfs:seeAlso rdf:resource="http://spitfire-project.eu/ontology/ns/Light"/>
    </owl:Class>
    


    <!-- http://purl.org/iot/vocab/m3-lite#Sound -->

    <owl:Class rdf:about="http://purl.org/iot/vocab/m3-lite#Sound">
        <rdfs:subClassOf rdf:resource="http://purl.org/NET/ssnx/qu/qu#QuantityKind"/>
        <rdfs:comment xml:lang="en">Measure of noise level in the environment</rdfs:comment>
        <rdfs:label xml:lang="en">Sound, Noise Level</rdfs:label>
    </owl:Class>
    


    <!-- http://purl.org/iot/vocab/m3-lite#SoundPressureLevel -->

    <owl:Class rdf:about="http://purl.org/iot/vocab/m3-lite#SoundPressureLevel">
        <rdfs:subClassOf rdf:resource="http://purl.org/NET/ssnx/qu/qu#QuantityKind"/>
        <rdfs:comment xml:lang="en">Sound pressure level is a logarithmic measure of the RMS sound pressure of a sound relative to a reference value, the threshold of hearing. The reference sound pressure was chosen conventionally to correspond to the quietest sound at 1000 Hz that the human ear can detect (20 uPa). In this case, the specific parameter is measured in an open environment.</rdfs:comment>
        <rdfs:label xml:lang="en">Sound Pressure Level</rdfs:label>
        <rdfs:seeAlso>http://purl.oclc.org/NET/ssnx/qu/quantity#soundPressure</rdfs:seeAlso>
    </owl:Class>
    


    <!-- http://purl.org/iot/vocab/m3-lite#SoundPressureLevelAmbient -->

    <owl:Class rdf:about="http://purl.org/iot/vocab/m3-lite#SoundPressureLevelAmbient">
        <rdfs:subClassOf rdf:resource="http://purl.org/iot/vocab/m3-lite#SoundPressureLevel"/>
        <rdfs:comment xml:lang="en">Similar to Sound.</rdfs:comment>
        <rdfs:label xml:lang="en">Sound Pressure Level Ambient</rdfs:label>
    </owl:Class>
    


    <!-- http://purl.org/iot/vocab/m3-lite#SoundSensor -->

    <owl:Class rdf:about="http://purl.org/iot/vocab/m3-lite#SoundSensor">
        <rdfs:subClassOf rdf:resource="http://purl.oclc.org/NET/ssnx/ssn#SensingDevice"/>
        <rdfs:subClassOf>
            <owl:Restriction>
                <owl:onProperty rdf:resource="http://purl.org/iot/vocab/m3-lite#hasDomainOfInterest"/>
                <owl:someValuesFrom rdf:resource="http://purl.org/iot/vocab/m3-lite#BuildingAutomation"/>
            </owl:Restriction>
        </rdfs:subClassOf>
        <rdfs:subClassOf>
            <owl:Restriction>
                <owl:onProperty rdf:resource="http://purl.org/iot/vocab/m3-lite#hasDomainOfInterest"/>
                <owl:someValuesFrom rdf:resource="http://purl.org/iot/vocab/m3-lite#Transportation"/>
            </owl:Restriction>
        </rdfs:subClassOf>
        <rdfs:comment xml:lang="en">Sensor used to detect Noise level. It can be Sound Sensor, Noise level Sensor, Volume sensor, Microphone</rdfs:comment>
        <rdfs:label xml:lang="en">Sound Sensor</rdfs:label>
        <rdfs:seeAlso rdf:resource="http://casas.wsu.edu/owl/cose.owl#Microphone"/>
    </owl:Class>
    


    <!-- http://purl.org/iot/vocab/m3-lite#SoundSource -->

    <owl:Class rdf:about="http://purl.org/iot/vocab/m3-lite#SoundSource">
        <rdfs:subClassOf rdf:resource="http://purl.org/iot/vocab/m3-lite#Source"/>
        <rdfs:comment xml:lang="en">Source where the sound originated.</rdfs:comment>
        <rdfs:label xml:lang="en">Sound Source</rdfs:label>
    </owl:Class>
    


    <!-- http://purl.org/iot/vocab/m3-lite#Source -->

    <owl:Class rdf:about="http://purl.org/iot/vocab/m3-lite#Source">
        <rdfs:comment xml:lang="en">Environmental Origin of a particular observation. With respect to one kind of Source (Sound source), it can be coming from traffic, siren of a police car, etc.</rdfs:comment>
        <rdfs:label xml:lang="en">Source</rdfs:label>
    </owl:Class>
    


    <!-- http://purl.org/iot/vocab/m3-lite#Speed -->

    <owl:Class rdf:about="http://purl.org/iot/vocab/m3-lite#Speed">
        <rdfs:subClassOf rdf:resource="http://purl.org/NET/ssnx/qu/qu#QuantityKind"/>
        <rdfs:comment xml:lang="en">The rate at which someone or something moves or operates or is able to move or operate.</rdfs:comment>
        <rdfs:label xml:lang="en">Speed</rdfs:label>
        <rdfs:seeAlso>http://purl.oclc.org/NET/ssnx/qu/quantity#speed</rdfs:seeAlso>
    </owl:Class>
    


    <!-- http://purl.org/iot/vocab/m3-lite#SpeedAverage -->

    <owl:Class rdf:about="http://purl.org/iot/vocab/m3-lite#SpeedAverage">
        <rdfs:subClassOf rdf:resource="http://purl.org/iot/vocab/m3-lite#Speed"/>
        <rdfs:comment>A measure of the average rate of motion of an object.</rdfs:comment>
        <rdfs:label xml:lang="en">Speed Average</rdfs:label>
    </owl:Class>
    


    <!-- http://purl.org/iot/vocab/m3-lite#SpeedInstantaneous -->

    <owl:Class rdf:about="http://purl.org/iot/vocab/m3-lite#SpeedInstantaneous">
        <rdfs:subClassOf rdf:resource="http://purl.org/iot/vocab/m3-lite#Speed"/>
        <rdfs:comment>A measure of the instantaneous rate of motion of an object.</rdfs:comment>
        <rdfs:label xml:lang="en">Speed Instantaneous</rdfs:label>
    </owl:Class>
    


    <!-- http://purl.org/iot/vocab/m3-lite#SpeedMedian -->

    <owl:Class rdf:about="http://purl.org/iot/vocab/m3-lite#SpeedMedian">
        <rdfs:subClassOf rdf:resource="http://purl.org/iot/vocab/m3-lite#Speed"/>
        <rdfs:comment>A measure of the median rate of motion of an object.</rdfs:comment>
        <rdfs:label xml:lang="en">Speed Median</rdfs:label>
    </owl:Class>
    


    <!-- http://purl.org/iot/vocab/m3-lite#SpeedSensor -->

    <owl:Class rdf:about="http://purl.org/iot/vocab/m3-lite#SpeedSensor">
        <rdfs:subClassOf rdf:resource="http://purl.oclc.org/NET/ssnx/ssn#SensingDevice"/>
        <rdfs:subClassOf>
            <owl:Restriction>
                <owl:onProperty rdf:resource="http://purl.org/iot/vocab/m3-lite#hasDomainOfInterest"/>
                <owl:someValuesFrom rdf:resource="http://purl.org/iot/vocab/m3-lite#Transportation"/>
            </owl:Restriction>
        </rdfs:subClassOf>
        <rdfs:comment xml:lang="en">Sensor used to detect speed.</rdfs:comment>
        <rdfs:label xml:lang="en">Speed Sensor</rdfs:label>
    </owl:Class>
    


    <!-- http://purl.org/iot/vocab/m3-lite#Step -->

    <owl:Class rdf:about="http://purl.org/iot/vocab/m3-lite#Step">
        <rdfs:subClassOf rdf:resource="http://purl.org/NET/ssnx/qu/qu#Unit"/>
        <rdfs:comment xml:lang="en">It is a measure of number of Step taken.</rdfs:comment>
        <rdfs:label xml:lang="en">Step</rdfs:label>
    </owl:Class>
    


    <!-- http://purl.org/iot/vocab/m3-lite#SunPositionDirection -->

    <owl:Class rdf:about="http://purl.org/iot/vocab/m3-lite#SunPositionDirection">
        <rdfs:subClassOf rdf:resource="http://purl.org/NET/ssnx/qu/qu#QuantityKind"/>
        <rdfs:comment xml:lang="en">The position of the Sun in the sky is a function of both time and the geographic coordinates of the observer on the surface of the Earth. (Source Wikipedia).</rdfs:comment>
        <rdfs:label xml:lang="en">Sun Position Direction</rdfs:label>
    </owl:Class>
    


    <!-- http://purl.org/iot/vocab/m3-lite#SunPositionDirectionSensor -->

    <owl:Class rdf:about="http://purl.org/iot/vocab/m3-lite#SunPositionDirectionSensor">
        <rdfs:subClassOf rdf:resource="http://purl.oclc.org/NET/ssnx/ssn#SensingDevice"/>
        <rdfs:subClassOf>
            <owl:Restriction>
                <owl:onProperty rdf:resource="http://purl.org/iot/vocab/m3-lite#hasDomainOfInterest"/>
                <owl:someValuesFrom rdf:resource="http://purl.org/iot/vocab/m3-lite#Weather"/>
            </owl:Restriction>
        </rdfs:subClassOf>
        <rdfs:comment xml:lang="en">Sensor used to detect sun position.</rdfs:comment>
        <rdfs:label xml:lang="en">Sun Position Direction Sensor</rdfs:label>
    </owl:Class>
    


    <!-- http://purl.org/iot/vocab/m3-lite#SunPositionElevation -->

    <owl:Class rdf:about="http://purl.org/iot/vocab/m3-lite#SunPositionElevation">
        <rdfs:subClassOf rdf:resource="http://purl.org/NET/ssnx/qu/qu#QuantityKind"/>
        <rdfs:comment xml:lang="en">It is the altitude of the sun, the angle between the horizon and the centre of the sun&apos;s disc.</rdfs:comment>
        <rdfs:label xml:lang="en">Sun Position Elevation</rdfs:label>
    </owl:Class>
    


    <!-- http://purl.org/iot/vocab/m3-lite#SunPositionElevationSensor -->

    <owl:Class rdf:about="http://purl.org/iot/vocab/m3-lite#SunPositionElevationSensor">
        <rdfs:subClassOf rdf:resource="http://purl.oclc.org/NET/ssnx/ssn#SensingDevice"/>
        <rdfs:subClassOf>
            <owl:Restriction>
                <owl:onProperty rdf:resource="http://purl.org/iot/vocab/m3-lite#hasDomainOfInterest"/>
                <owl:someValuesFrom rdf:resource="http://purl.org/iot/vocab/m3-lite#Weather"/>
            </owl:Restriction>
        </rdfs:subClassOf>
        <rdfs:comment xml:lang="en">Device used to detect sun elevation.</rdfs:comment>
        <rdfs:label xml:lang="en">Sun Position Elevation Sensor</rdfs:label>
    </owl:Class>
    


    <!-- http://purl.org/iot/vocab/m3-lite#SystolicBloodPressure -->

    <owl:Class rdf:about="http://purl.org/iot/vocab/m3-lite#SystolicBloodPressure">
        <rdfs:subClassOf rdf:resource="http://purl.org/iot/vocab/m3-lite#BloodPressure"/>
        <rdfs:comment xml:lang="en">It is the pressure when the heart beats while pumping blood.</rdfs:comment>
        <rdfs:label xml:lang="en">Systolic Blood Pressure</rdfs:label>
    </owl:Class>
    


    <!-- http://purl.org/iot/vocab/m3-lite#TV -->

    <owl:Class rdf:about="http://purl.org/iot/vocab/m3-lite#TV">
        <rdfs:subClassOf rdf:resource="http://purl.oclc.org/NET/UNIS/fiware/iot-lite#ActuatingDevice"/>
        <rdfs:subClassOf>
            <owl:Restriction>
                <owl:onProperty rdf:resource="http://purl.org/iot/vocab/m3-lite#hasDomainOfInterest"/>
                <owl:someValuesFrom rdf:resource="http://purl.org/iot/vocab/m3-lite#BuildingAutomation"/>
            </owl:Restriction>
        </rdfs:subClassOf>
        <rdfs:comment xml:lang="en">An actuator to automatically switch on/off the television.</rdfs:comment>
        <rdfs:label xml:lang="en">TV Actuating Device</rdfs:label>
    </owl:Class>
    


    <!-- http://purl.org/iot/vocab/m3-lite#Telephone -->

    <owl:Class rdf:about="http://purl.org/iot/vocab/m3-lite#Telephone">
        <rdfs:subClassOf rdf:resource="http://purl.oclc.org/NET/UNIS/fiware/iot-lite#ActuatingDevice"/>
        <rdfs:subClassOf>
            <owl:Restriction>
                <owl:onProperty rdf:resource="http://purl.org/iot/vocab/m3-lite#hasDomainOfInterest"/>
                <owl:someValuesFrom rdf:resource="http://purl.org/iot/vocab/m3-lite#BuildingAutomation"/>
            </owl:Restriction>
        </rdfs:subClassOf>
        <rdfs:comment xml:lang="en">An actuator to automatically switch on/off the Telephone.</rdfs:comment>
        <rdfs:label xml:lang="en">Telephone Actuating Device</rdfs:label>
    </owl:Class>
    


    <!-- http://purl.org/iot/vocab/m3-lite#Temperature -->

    <owl:Class rdf:about="http://purl.org/iot/vocab/m3-lite#Temperature">
        <rdfs:subClassOf rdf:resource="http://purl.org/NET/ssnx/qu/qu#QuantityKind"/>
        <rdfs:comment xml:lang="en">It is the air temperature.</rdfs:comment>
        <rdfs:label xml:lang="en">Temperature</rdfs:label>
        <rdfs:seeAlso rdf:resource="http://archive.knoesis.org/research/semsci/application_domain/sem_sensor/ont/sensor-observation.owlTemperatureProperty"/>
        <rdfs:seeAlso rdf:resource="http://openiot.eu/ontology/ns/Temperature"/>
        <rdfs:seeAlso rdf:resource="http://purl.oclc.org/NET/ssnx/meteo/aws#air_temperature"/>
    </owl:Class>
    


    <!-- http://purl.org/iot/vocab/m3-lite#TemperatureEngine -->

    <owl:Class rdf:about="http://purl.org/iot/vocab/m3-lite#TemperatureEngine">
        <rdfs:subClassOf rdf:resource="http://purl.org/iot/vocab/m3-lite#Temperature"/>
        <rdfs:comment xml:lang="en">The temperature of a vehicle engine.</rdfs:comment>
        <rdfs:label xml:lang="en">Temperature Engine</rdfs:label>
    </owl:Class>
    


    <!-- http://purl.org/iot/vocab/m3-lite#TemperatureWasteContainer -->

    <owl:Class rdf:about="http://purl.org/iot/vocab/m3-lite#TemperatureWasteContainer">
        <rdfs:subClassOf rdf:resource="http://purl.org/iot/vocab/m3-lite#Temperature"/>
        <rdfs:comment xml:lang="en">The temperature of the air that would be indicated by a thermometer exposed to the air inside a waste container.</rdfs:comment>
        <rdfs:label xml:lang="en">Temperature Waste Container</rdfs:label>
    </owl:Class>
    


    <!-- http://purl.org/iot/vocab/m3-lite#Tesla -->

    <owl:Class rdf:about="http://purl.org/iot/vocab/m3-lite#Tesla">
        <rdfs:subClassOf rdf:resource="http://purl.org/NET/ssnx/qu/qu#Unit"/>
        <rdfs:comment xml:lang="en">It is the SI unit of magnetic flux density.</rdfs:comment>
        <rdfs:label xml:lang="en">Tesla</rdfs:label>
    </owl:Class>
    


    <!-- http://purl.org/iot/vocab/m3-lite#Thermometer -->

    <owl:Class rdf:about="http://purl.org/iot/vocab/m3-lite#Thermometer">
        <rdfs:subClassOf rdf:resource="http://purl.oclc.org/NET/ssnx/ssn#SensingDevice"/>
        <rdfs:subClassOf>
            <owl:Restriction>
                <owl:onProperty rdf:resource="http://purl.org/iot/vocab/m3-lite#hasDomainOfInterest"/>
                <owl:someValuesFrom rdf:resource="http://purl.org/iot/vocab/m3-lite#BuildingAutomation"/>
            </owl:Restriction>
        </rdfs:subClassOf>
        <rdfs:subClassOf>
            <owl:Restriction>
                <owl:onProperty rdf:resource="http://purl.org/iot/vocab/m3-lite#hasDomainOfInterest"/>
                <owl:someValuesFrom rdf:resource="http://purl.org/iot/vocab/m3-lite#EnergyDOI"/>
            </owl:Restriction>
        </rdfs:subClassOf>
        <rdfs:subClassOf>
            <owl:Restriction>
                <owl:onProperty rdf:resource="http://purl.org/iot/vocab/m3-lite#hasDomainOfInterest"/>
                <owl:someValuesFrom rdf:resource="http://purl.org/iot/vocab/m3-lite#Environment"/>
            </owl:Restriction>
        </rdfs:subClassOf>
        <rdfs:subClassOf>
            <owl:Restriction>
                <owl:onProperty rdf:resource="http://purl.org/iot/vocab/m3-lite#hasDomainOfInterest"/>
                <owl:someValuesFrom rdf:resource="http://purl.org/iot/vocab/m3-lite#Weather"/>
            </owl:Restriction>
        </rdfs:subClassOf>
        <rdfs:comment xml:lang="en">A device to measure the temperature in a room or outside.</rdfs:comment>
        <rdfs:label xml:lang="en">Thermometer</rdfs:label>
        <rdfs:seeAlso rdf:resource="http://casas.wsu.edu/owl/cose.owl#TempuratureSensor"/>
        <rdfs:seeAlso rdf:resource="http://purl.oclc.org/NET/ssnx/meteo/aws#TemperatureSensor"/>
    </owl:Class>
    


    <!-- http://purl.org/iot/vocab/m3-lite#ThrottleSensor -->

    <owl:Class rdf:about="http://purl.org/iot/vocab/m3-lite#ThrottleSensor">
        <rdfs:subClassOf rdf:resource="http://purl.oclc.org/NET/ssnx/ssn#SensingDevice"/>
        <rdfs:subClassOf>
            <owl:Restriction>
                <owl:onProperty rdf:resource="http://purl.org/iot/vocab/m3-lite#hasDomainOfInterest"/>
                <owl:someValuesFrom rdf:resource="http://purl.org/iot/vocab/m3-lite#Transportation"/>
            </owl:Restriction>
        </rdfs:subClassOf>
        <rdfs:comment xml:lang="en">It is a device used to monitor the throttle position of a vehicle.</rdfs:comment>
        <rdfs:label xml:lang="en">Throttle Position Sensor</rdfs:label>
    </owl:Class>
    


    <!-- http://purl.org/iot/vocab/m3-lite#TimeRelatedState -->

    <owl:Class rdf:about="http://purl.org/iot/vocab/m3-lite#TimeRelatedState">
        <rdfs:subClassOf rdf:resource="http://purl.org/NET/ssnx/qu/qu#QuantityKind"/>
        <rdfs:comment xml:lang="en">Indicator of whether a person (or object) has overpassed a particular time threshold (e.g. maximum number of hours driving, etc.)</rdfs:comment>
        <rdfs:label xml:lang="en">Time Related State</rdfs:label>
    </owl:Class>
    


    <!-- http://purl.org/iot/vocab/m3-lite#TimeRelatedStateDriver -->

    <owl:Class rdf:about="http://purl.org/iot/vocab/m3-lite#TimeRelatedStateDriver">
        <rdfs:subClassOf rdf:resource="http://purl.org/iot/vocab/m3-lite#TimeRelatedState"/>
        <rdfs:comment xml:lang="en">Indicator of whether the driver of a vehicle approaches or exceeds his/her working time limits.</rdfs:comment>
        <rdfs:label xml:lang="en">Time Related State Driver</rdfs:label>
    </owl:Class>
    


    <!-- http://purl.org/iot/vocab/m3-lite#TimeRelatedStateDriver1 -->

    <owl:Class rdf:about="http://purl.org/iot/vocab/m3-lite#TimeRelatedStateDriver1">
        <rdfs:subClassOf rdf:resource="http://purl.org/iot/vocab/m3-lite#TimeRelatedStateDriver"/>
        <rdfs:comment xml:lang="en">Indicates if the first driver approaches or exceeds working time limits (or other limits).</rdfs:comment>
        <rdfs:label xml:lang="en">Time Related State Driver 1</rdfs:label>
    </owl:Class>
    


    <!-- http://purl.org/iot/vocab/m3-lite#TimeRelatedStateDriver2 -->

    <owl:Class rdf:about="http://purl.org/iot/vocab/m3-lite#TimeRelatedStateDriver2">
        <rdfs:subClassOf rdf:resource="http://purl.org/iot/vocab/m3-lite#TimeRelatedStateDriver"/>
        <rdfs:comment xml:lang="en">Indicates if the second driver approaches or exceeds working time limits (or other limits).</rdfs:comment>
        <rdfs:label xml:lang="en">Time Related State Driver 2</rdfs:label>
    </owl:Class>
    


    <!-- http://purl.org/iot/vocab/m3-lite#Timestamp -->

    <owl:Class rdf:about="http://purl.org/iot/vocab/m3-lite#Timestamp">
        <rdfs:subClassOf rdf:resource="http://purl.org/NET/ssnx/qu/qu#QuantityKind"/>
        <rdfs:comment>Sequence of characters or encoded information identifying when a certain event occurred, usually giving date and time of day, sometimes accurate to a small fraction of a second. This representation should be encoded following ISO8601.</rdfs:comment>
        <rdfs:label xml:lang="en">Timestamp</rdfs:label>
        <rdfs:seeAlso>http://sweet.jpl.nasa.gov/2.3/propTime.owl#Timestamp</rdfs:seeAlso>
    </owl:Class>
    


    <!-- http://purl.org/iot/vocab/m3-lite#Tonne -->

    <owl:Class rdf:about="http://purl.org/iot/vocab/m3-lite#Tonne">
        <rdfs:subClassOf rdf:resource="http://purl.org/iot/vocab/m3-lite#Gram"/>
        <rdfs:comment xml:lang="en">It is a non-SI metric unit of mass equal to 1,000 kilograms.</rdfs:comment>
        <rdfs:label xml:lang="en">Tonne</rdfs:label>
    </owl:Class>
    


    <!-- http://purl.org/iot/vocab/m3-lite#TouchSensor -->

    <owl:Class rdf:about="http://purl.org/iot/vocab/m3-lite#TouchSensor">
        <rdfs:subClassOf rdf:resource="http://purl.oclc.org/NET/ssnx/ssn#SensingDevice"/>
        <rdfs:comment xml:lang="en">Device that captures and records physical touch or embrace on a device and/or object.</rdfs:comment>
        <rdfs:label xml:lang="en">Touch Sensor</rdfs:label>
    </owl:Class>
    


    <!-- http://purl.org/iot/vocab/m3-lite#Tourism -->

    <owl:Class rdf:about="http://purl.org/iot/vocab/m3-lite#Tourism">
        <rdfs:subClassOf rdf:resource="http://purl.org/iot/vocab/m3-lite#DomainOfInterest"/>
        <rdfs:comment xml:lang="en">Tourism as an Internet of Things (IoT) applicative domain.</rdfs:comment>
        <rdfs:label xml:lang="en">Tourism DOI</rdfs:label>
    </owl:Class>
    


    <!-- http://purl.org/iot/vocab/m3-lite#Traffic -->

    <owl:Class rdf:about="http://purl.org/iot/vocab/m3-lite#Traffic">
        <rdfs:subClassOf rdf:resource="http://purl.org/iot/vocab/m3-lite#SoundSource"/>
        <rdfs:comment xml:lang="en">When the source of the sound was traffic.</rdfs:comment>
        <rdfs:label xml:lang="en">Traffic</rdfs:label>
    </owl:Class>
    


    <!-- http://purl.org/iot/vocab/m3-lite#TrafficIntensity -->

    <owl:Class rdf:about="http://purl.org/iot/vocab/m3-lite#TrafficIntensity">
        <rdfs:subClassOf rdf:resource="http://purl.org/NET/ssnx/qu/qu#QuantityKind"/>
        <rdfs:comment xml:lang="en">The intensity of a traffic flow is the number of vehicles passing a cross section of a road in a unit of time.</rdfs:comment>
        <rdfs:label xml:lang="en">Traffic Intensity</rdfs:label>
    </owl:Class>
    


    <!-- http://purl.org/iot/vocab/m3-lite#Transportation -->

    <owl:Class rdf:about="http://purl.org/iot/vocab/m3-lite#Transportation">
        <rdfs:subClassOf rdf:resource="http://purl.org/iot/vocab/m3-lite#DomainOfInterest"/>
        <rdfs:comment xml:lang="en">Transportation, Smart Car/Vehicle, Intelligent Transport System (ITS) as an Internet of Things (IoT) applicative domain.</rdfs:comment>
        <rdfs:label xml:lang="en">Transportation DOI</rdfs:label>
    </owl:Class>
    


    <!-- http://purl.org/iot/vocab/m3-lite#UltrasonicSensor -->

    <owl:Class rdf:about="http://purl.org/iot/vocab/m3-lite#UltrasonicSensor">
        <rdfs:subClassOf rdf:resource="http://purl.oclc.org/NET/ssnx/ssn#SensingDevice"/>
        <rdfs:subClassOf>
            <owl:Restriction>
                <owl:onProperty rdf:resource="http://purl.org/iot/vocab/m3-lite#hasDomainOfInterest"/>
                <owl:someValuesFrom rdf:resource="http://purl.org/iot/vocab/m3-lite#BuildingAutomation"/>
            </owl:Restriction>
        </rdfs:subClassOf>
        <rdfs:comment xml:lang="en">Ultrasonic sensors are used to deduce human posture in smart home for example.</rdfs:comment>
        <rdfs:label xml:lang="en">Ultrasonic Sensor</rdfs:label>
    </owl:Class>
    


    <!-- http://purl.org/iot/vocab/m3-lite#VOCSensor -->

    <owl:Class rdf:about="http://purl.org/iot/vocab/m3-lite#VOCSensor">
        <rdfs:subClassOf rdf:resource="http://purl.org/iot/vocab/m3-lite#GaseousPollutantSensor"/>
        <rdfs:comment xml:lang="en">Sensor that detects levels of Volatile Organic Components (VOC) in the environment.</rdfs:comment>
        <rdfs:label xml:lang="en">Volatile Organic Compound (VOC) Sensor</rdfs:label>
    </owl:Class>
    


    <!-- http://purl.org/iot/vocab/m3-lite#VehicleCountSensor -->

    <owl:Class rdf:about="http://purl.org/iot/vocab/m3-lite#VehicleCountSensor">
        <rdfs:subClassOf rdf:resource="http://purl.org/iot/vocab/m3-lite#Counter"/>
        <rdfs:subClassOf>
            <owl:Restriction>
                <owl:onProperty rdf:resource="http://purl.org/iot/vocab/m3-lite#hasDomainOfInterest"/>
                <owl:someValuesFrom rdf:resource="http://purl.org/iot/vocab/m3-lite#Transportation"/>
            </owl:Restriction>
        </rdfs:subClassOf>
        <rdfs:comment xml:lang="en">Device used to count the number of vehicles (e.g., used within the Citypulse project).</rdfs:comment>
        <rdfs:label xml:lang="en">Vehicle Count Sensor</rdfs:label>
    </owl:Class>
    


    <!-- http://purl.org/iot/vocab/m3-lite#VehicleOverspeedState -->

    <owl:Class rdf:about="http://purl.org/iot/vocab/m3-lite#VehicleOverspeedState">
        <rdfs:subClassOf rdf:resource="http://purl.org/NET/ssnx/qu/qu#QuantityKind"/>
        <rdfs:comment xml:lang="en">Measure to indicates whether the vehicle is exceeding the legal speed limit.</rdfs:comment>
        <rdfs:label xml:lang="en">Vehicle Overspeed State</rdfs:label>
    </owl:Class>
    


    <!-- http://purl.org/iot/vocab/m3-lite#VehiclePresenceDetector -->

    <owl:Class rdf:about="http://purl.org/iot/vocab/m3-lite#VehiclePresenceDetector">
        <rdfs:subClassOf rdf:resource="http://purl.org/iot/vocab/m3-lite#PresenceDetector"/>
        <rdfs:comment xml:lang="en">Device used to detect if an vehicle is present at a place.</rdfs:comment>
        <rdfs:label xml:lang="en"> Vehicle Presence Detector</rdfs:label>
    </owl:Class>
    


    <!-- http://purl.org/iot/vocab/m3-lite#VehiclesPerMinute -->

    <owl:Class rdf:about="http://purl.org/iot/vocab/m3-lite#VehiclesPerMinute">
        <rdfs:subClassOf rdf:resource="http://purl.org/NET/ssnx/qu/qu#Unit"/>
        <rdfs:comment xml:lang="en">Number of vehicles that traverse a concrete region of the space in one minute.</rdfs:comment>
        <rdfs:label xml:lang="en">Vehicles Per Minute</rdfs:label>
    </owl:Class>
    


    <!-- http://purl.org/iot/vocab/m3-lite#Ventilation -->

    <owl:Class rdf:about="http://purl.org/iot/vocab/m3-lite#Ventilation">
        <rdfs:subClassOf rdf:resource="http://purl.oclc.org/NET/UNIS/fiware/iot-lite#ActuatingDevice"/>
        <rdfs:subClassOf>
            <owl:Restriction>
                <owl:onProperty rdf:resource="http://purl.org/iot/vocab/m3-lite#hasDomainOfInterest"/>
                <owl:someValuesFrom rdf:resource="http://purl.org/iot/vocab/m3-lite#BuildingAutomation"/>
            </owl:Restriction>
        </rdfs:subClassOf>
        <rdfs:comment xml:lang="en">An actuator to automatically open/close the ventilation.</rdfs:comment>
        <rdfs:label xml:lang="en">Ventilation Actuating Device</rdfs:label>
    </owl:Class>
    


    <!-- http://purl.org/iot/vocab/m3-lite#Visibility -->

    <owl:Class rdf:about="http://purl.org/iot/vocab/m3-lite#Visibility">
        <rdfs:subClassOf rdf:resource="http://purl.org/NET/ssnx/qu/qu#QuantityKind"/>
        <rdfs:comment xml:lang="en">The state of being able to see or be seen.</rdfs:comment>
        <rdfs:label xml:lang="en">Visibility</rdfs:label>
        <rdfs:seeAlso rdf:resource="http://openiot.eu/ontology/ns/AtmosphereVisibility"/>
    </owl:Class>
    


    <!-- http://purl.org/iot/vocab/m3-lite#VisibilitySensor -->

    <owl:Class rdf:about="http://purl.org/iot/vocab/m3-lite#VisibilitySensor">
        <rdfs:subClassOf rdf:resource="http://purl.oclc.org/NET/ssnx/ssn#SensingDevice"/>
        <rdfs:subClassOf>
            <owl:Restriction>
                <owl:onProperty rdf:resource="http://purl.org/iot/vocab/m3-lite#hasDomainOfInterest"/>
                <owl:someValuesFrom rdf:resource="http://purl.org/iot/vocab/m3-lite#Transportation"/>
            </owl:Restriction>
        </rdfs:subClassOf>
        <rdfs:comment xml:lang="en">Device used to detect Visibility.</rdfs:comment>
        <rdfs:label xml:lang="en">Visibility Sensor</rdfs:label>
    </owl:Class>
    


    <!-- http://purl.org/iot/vocab/m3-lite#VoiceCommand -->

    <owl:Class rdf:about="http://purl.org/iot/vocab/m3-lite#VoiceCommand">
        <rdfs:subClassOf rdf:resource="http://purl.org/NET/ssnx/qu/qu#QuantityKind"/>
        <rdfs:comment xml:lang="en">A voice command to control a voice controlled system or environment, such as a smart home.</rdfs:comment>
        <rdfs:label xml:lang="en">Voice Command</rdfs:label>
    </owl:Class>
    


    <!-- http://purl.org/iot/vocab/m3-lite#VoiceCommandController -->

    <owl:Class rdf:about="http://purl.org/iot/vocab/m3-lite#VoiceCommandController">
        <rdfs:subClassOf rdf:resource="http://purl.oclc.org/NET/UNIS/fiware/iot-lite#ActuatingDevice"/>
        <rdfs:comment xml:lang="en">An actuating device called  that allows to semi-control the environment of the Voice Command Sensor.</rdfs:comment>
        <rdfs:label xml:lang="en">Voice Command Controller</rdfs:label>
    </owl:Class>
    


    <!-- http://purl.org/iot/vocab/m3-lite#VoiceCommandSensor -->

    <owl:Class rdf:about="http://purl.org/iot/vocab/m3-lite#VoiceCommandSensor">
        <rdfs:subClassOf rdf:resource="http://purl.oclc.org/NET/ssnx/ssn#SensingDevice"/>
        <rdfs:comment xml:lang="en">Sensor that uses automatic speech recognition technology to match or reject a recorded voice command according to a specified set of available voice commands.</rdfs:comment>
        <rdfs:label xml:lang="en">Voice Command Sensor</rdfs:label>
    </owl:Class>
    


    <!-- http://purl.org/iot/vocab/m3-lite#Volt -->

    <owl:Class rdf:about="http://purl.org/iot/vocab/m3-lite#Volt">
        <rdfs:subClassOf rdf:resource="http://purl.org/NET/ssnx/qu/qu#Unit"/>
        <rdfs:comment xml:lang="en">The SI unit of electromotive force, the difference of potential that would carry one ampere of current against one ohm resistance.</rdfs:comment>
        <rdfs:label xml:lang="en">Volt</rdfs:label>
        <rdfs:seeAlso rdf:resource="http://sweet.jpl.nasa.gov/ontology/units.owl#volt"/>
    </owl:Class>
    


    <!-- http://purl.org/iot/vocab/m3-lite#VoltAmpereReactive -->

    <owl:Class rdf:about="http://purl.org/iot/vocab/m3-lite#VoltAmpereReactive">
        <rdfs:subClassOf rdf:resource="http://purl.org/NET/ssnx/qu/qu#Unit"/>
        <rdfs:comment xml:lang="en">In electric power transmission and distribution, volt-ampere reactive (var) is a unit in which reactive power is expressed in an AC electric power system.</rdfs:comment>
        <rdfs:label xml:lang="en">Volt Ampere Reactive, VAR</rdfs:label>
        <rdfs:seeAlso>http://purl.oclc.org/NET/ssnx/qu/unit#var</rdfs:seeAlso>
    </owl:Class>
    


    <!-- http://purl.org/iot/vocab/m3-lite#Voltage -->

    <owl:Class rdf:about="http://purl.org/iot/vocab/m3-lite#Voltage">
        <rdfs:subClassOf rdf:resource="http://purl.org/NET/ssnx/qu/qu#QuantityKind"/>
        <rdfs:comment xml:lang="en">An electromotive force or potential difference expressed in volts (Source Google).</rdfs:comment>
        <rdfs:label xml:lang="en">Voltage</rdfs:label>
    </owl:Class>
    


    <!-- http://purl.org/iot/vocab/m3-lite#VoltageSensor -->

    <owl:Class rdf:about="http://purl.org/iot/vocab/m3-lite#VoltageSensor">
        <rdfs:subClassOf rdf:resource="http://purl.oclc.org/NET/ssnx/ssn#SensingDevice"/>
        <rdfs:comment xml:lang="en">Device which can measure the difference in electric potential energy between two points per unit electric charge.</rdfs:comment>
        <rdfs:label xml:lang="en">Voltage Sensor</rdfs:label>
    </owl:Class>
    


    <!-- http://purl.org/iot/vocab/m3-lite#WashingMachine -->

    <owl:Class rdf:about="http://purl.org/iot/vocab/m3-lite#WashingMachine">
        <rdfs:subClassOf rdf:resource="http://purl.oclc.org/NET/UNIS/fiware/iot-lite#ActuatingDevice"/>
        <rdfs:subClassOf>
            <owl:Restriction>
                <owl:onProperty rdf:resource="http://purl.org/iot/vocab/m3-lite#hasDomainOfInterest"/>
                <owl:someValuesFrom rdf:resource="http://purl.org/iot/vocab/m3-lite#BuildingAutomation"/>
            </owl:Restriction>
        </rdfs:subClassOf>
        <rdfs:comment xml:lang="en">An actuator to automatically switch on/off the washing machine.</rdfs:comment>
        <rdfs:label xml:lang="en">Washing Machine Actuation Device</rdfs:label>
    </owl:Class>
    


    <!-- http://purl.org/iot/vocab/m3-lite#WaterConductivitySensor -->

    <owl:Class rdf:about="http://purl.org/iot/vocab/m3-lite#WaterConductivitySensor">
        <rdfs:subClassOf rdf:resource="http://purl.org/iot/vocab/m3-lite#ConductivitySensor"/>
        <rdfs:comment xml:lang="en">Device used to measure the conductivity of water.</rdfs:comment>
        <rdfs:label xml:lang="en">Water Conductivity Sensor</rdfs:label>
    </owl:Class>
    


    <!-- http://purl.org/iot/vocab/m3-lite#WaterLevel -->

    <owl:Class rdf:about="http://purl.org/iot/vocab/m3-lite#WaterLevel">
        <rdfs:subClassOf rdf:resource="http://purl.org/NET/ssnx/qu/qu#QuantityKind"/>
        <rdfs:comment xml:lang="en">The height reached by the water in a reservoir, river, storage tank, or similar.</rdfs:comment>
        <rdfs:label xml:lang="en">Water Level</rdfs:label>
    </owl:Class>
    


    <!-- http://purl.org/iot/vocab/m3-lite#WaterNH4IonSensor -->

    <owl:Class rdf:about="http://purl.org/iot/vocab/m3-lite#WaterNH4IonSensor">
        <rdfs:subClassOf rdf:resource="http://purl.oclc.org/NET/ssnx/ssn#SensingDevice"/>
        <rdfs:comment xml:lang="en">Sensor used to measure NH4 concentration level in the water.</rdfs:comment>
        <rdfs:label xml:lang="en">Water NH4 Ion Sensor</rdfs:label>
    </owl:Class>
    


    <!-- http://purl.org/iot/vocab/m3-lite#WaterNO3IonSensor -->

    <owl:Class rdf:about="http://purl.org/iot/vocab/m3-lite#WaterNO3IonSensor">
        <rdfs:subClassOf rdf:resource="http://purl.oclc.org/NET/ssnx/ssn#SensingDevice"/>
        <rdfs:comment xml:lang="en">Sensor used to measure NO3 concentration level in the water.</rdfs:comment>
        <rdfs:label xml:lang="en">Water NO3 Ion Sensor</rdfs:label>
    </owl:Class>
    


    <!-- http://purl.org/iot/vocab/m3-lite#WaterO2IonSensor -->

    <owl:Class rdf:about="http://purl.org/iot/vocab/m3-lite#WaterO2IonSensor">
        <rdfs:subClassOf rdf:resource="http://purl.oclc.org/NET/ssnx/ssn#SensingDevice"/>
        <rdfs:comment xml:lang="en">Sensor used to measure O2 concentration level in the water.</rdfs:comment>
        <rdfs:label xml:lang="en">Water O2 Ion Sensor</rdfs:label>
    </owl:Class>
    


    <!-- http://purl.org/iot/vocab/m3-lite#WaterPHSensor -->

    <owl:Class rdf:about="http://purl.org/iot/vocab/m3-lite#WaterPHSensor">
        <rdfs:subClassOf rdf:resource="http://purl.org/iot/vocab/m3-lite#PHSensor"/>
        <rdfs:comment xml:lang="en">Device used to detect PH level of water.</rdfs:comment>
        <rdfs:label xml:lang="en">Water PH Sensor</rdfs:label>
    </owl:Class>
    


    <!-- http://purl.org/iot/vocab/m3-lite#WaterTemperature -->

    <owl:Class rdf:about="http://purl.org/iot/vocab/m3-lite#WaterTemperature">
        <rdfs:subClassOf rdf:resource="http://purl.org/iot/vocab/m3-lite#Temperature"/>
        <rdfs:comment xml:lang="en">Sea surface temperature (SST) is the water temperature close to the ocean&apos;s surface.</rdfs:comment>
        <rdfs:label xml:lang="en">Water Temperature</rdfs:label>
    </owl:Class>
    


    <!-- http://purl.org/iot/vocab/m3-lite#WaterThermometer -->

    <owl:Class rdf:about="http://purl.org/iot/vocab/m3-lite#WaterThermometer">
        <rdfs:subClassOf rdf:resource="http://purl.org/iot/vocab/m3-lite#Thermometer"/>
        <rdfs:comment xml:lang="en">This sensor reports Water temperature.</rdfs:comment>
        <rdfs:label xml:lang="en">Water Thermometer</rdfs:label>
    </owl:Class>
    


    <!-- http://purl.org/iot/vocab/m3-lite#Watt -->

    <owl:Class rdf:about="http://purl.org/iot/vocab/m3-lite#Watt">
        <rdfs:subClassOf rdf:resource="http://purl.org/NET/ssnx/qu/qu#Unit"/>
        <rdfs:comment xml:lang="en">It is the SI unit of power, equivalent to one joule per second, corresponding to the rate of consumption of energy in an electric circuit where the potential difference is one volt and the current one ampere.</rdfs:comment>
        <rdfs:label xml:lang="en">Watt (W)</rdfs:label>
        <rdfs:seeAlso rdf:resource="http://sweet.jpl.nasa.gov/ontology/units.owl#watt"/>
    </owl:Class>
    


    <!-- http://purl.org/iot/vocab/m3-lite#WattPerSquareMetre -->

    <owl:Class rdf:about="http://purl.org/iot/vocab/m3-lite#WattPerSquareMetre">
        <rdfs:subClassOf rdf:resource="http://purl.org/NET/ssnx/qu/qu#Unit"/>
        <rdfs:comment xml:lang="en">It is the SI unit for radiative and other energy fluxes.</rdfs:comment>
        <rdfs:label xml:lang="en">Watt Per Square Metre, Watt Per Square Meter</rdfs:label>
        <rdfs:seeAlso>http://purl.oclc.org/NET/ssnx/qu/unit#wattPerSquareMetre</rdfs:seeAlso>
    </owl:Class>
    


    <!-- http://purl.org/iot/vocab/m3-lite#Weather -->

    <owl:Class rdf:about="http://purl.org/iot/vocab/m3-lite#Weather">
        <rdfs:subClassOf rdf:resource="http://purl.org/iot/vocab/m3-lite#DomainOfInterest"/>
        <rdfs:comment xml:lang="en">Weather Forecasting, Meterology as an Internet of Things (IoT) applicative domain.</rdfs:comment>
        <rdfs:label xml:lang="en">Weather Forecasting DOI</rdfs:label>
        <rdfs:seeAlso rdf:resource="http://archive.knoesis.org/research/semsci/application_domain/sem_sensor/ont/sensor-observation.owlWeatherObservation"/>
    </owl:Class>
    


    <!-- http://purl.org/iot/vocab/m3-lite#WeatherLuminosity -->

    <owl:Class rdf:about="http://purl.org/iot/vocab/m3-lite#WeatherLuminosity">
        <rdfs:subClassOf rdf:resource="http://purl.org/iot/vocab/m3-lite#Illuminance"/>
        <rdfs:comment xml:lang="en">Luminosity.</rdfs:comment>
        <rdfs:label xml:lang="en">Weather Luminosity</rdfs:label>
    </owl:Class>
    


    <!-- http://purl.org/iot/vocab/m3-lite#WeatherPrecipitation -->

    <owl:Class rdf:about="http://purl.org/iot/vocab/m3-lite#WeatherPrecipitation">
        <rdfs:subClassOf rdf:resource="http://purl.org/iot/vocab/m3-lite#Precipitation"/>
        <rdfs:comment xml:lang="en">Weather Precipitation.</rdfs:comment>
        <rdfs:label xml:lang="en">Weather Precipitation</rdfs:label>
    </owl:Class>
    


    <!-- http://purl.org/iot/vocab/m3-lite#Weight -->

    <owl:Class rdf:about="http://purl.org/iot/vocab/m3-lite#Weight">
        <rdfs:subClassOf rdf:resource="http://purl.org/NET/ssnx/qu/qu#QuantityKind"/>
        <rdfs:comment xml:lang="en">A body&apos;s relative mass or the quantity of matter contained by it, giving rise to a downward force; the heaviness of a person or thing.</rdfs:comment>
        <rdfs:label xml:lang="en">Weight</rdfs:label>
    </owl:Class>
    


    <!-- http://purl.org/iot/vocab/m3-lite#WeightSensor -->

    <owl:Class rdf:about="http://purl.org/iot/vocab/m3-lite#WeightSensor">
        <rdfs:subClassOf rdf:resource="http://purl.oclc.org/NET/ssnx/ssn#SensingDevice"/>
        <rdfs:subClassOf>
            <owl:Restriction>
                <owl:onProperty rdf:resource="http://purl.org/iot/vocab/m3-lite#hasDomainOfInterest"/>
                <owl:someValuesFrom rdf:resource="http://purl.org/iot/vocab/m3-lite#Health"/>
            </owl:Restriction>
        </rdfs:subClassOf>
        <rdfs:comment xml:lang="en">Device used to weight an object.</rdfs:comment>
        <rdfs:label xml:lang="en">Weight Sensor</rdfs:label>
    </owl:Class>
    


    <!-- http://purl.org/iot/vocab/m3-lite#WiFiInterfaceEnergyMeter -->

    <owl:Class rdf:about="http://purl.org/iot/vocab/m3-lite#WiFiInterfaceEnergyMeter">
        <rdfs:subClassOf rdf:resource="http://purl.org/iot/vocab/m3-lite#EnergyMeter"/>
        <rdfs:comment xml:lang="en">Measure the average power consumption of the WiFi interface nodes.</rdfs:comment>
        <rdfs:label xml:lang="en">WiFi Interface Energy Meter</rdfs:label>
    </owl:Class>
    


    <!-- http://purl.org/iot/vocab/m3-lite#WindChill -->

    <owl:Class rdf:about="http://purl.org/iot/vocab/m3-lite#WindChill">
        <rdfs:subClassOf rdf:resource="http://purl.org/NET/ssnx/qu/qu#QuantityKind"/>
        <rdfs:comment xml:lang="en">The cooling effect of wind blowing on a surface.</rdfs:comment>
        <rdfs:label xml:lang="en">Wind Chill</rdfs:label>
        <rdfs:seeAlso rdf:resource="http://openiot.eu/ontology/ns/WindChill"/>
    </owl:Class>
    


    <!-- http://purl.org/iot/vocab/m3-lite#WindChillSensor -->

    <owl:Class rdf:about="http://purl.org/iot/vocab/m3-lite#WindChillSensor">
        <rdfs:subClassOf rdf:resource="http://purl.oclc.org/NET/ssnx/ssn#SensingDevice"/>
        <rdfs:subClassOf>
            <owl:Restriction>
                <owl:onProperty rdf:resource="http://purl.org/iot/vocab/m3-lite#hasDomainOfInterest"/>
                <owl:someValuesFrom rdf:resource="http://purl.org/iot/vocab/m3-lite#Weather"/>
            </owl:Restriction>
        </rdfs:subClassOf>
        <rdfs:comment xml:lang="en">Device used to detect Wind Chill.</rdfs:comment>
        <rdfs:label xml:lang="en">Wind Chill Sensor</rdfs:label>
    </owl:Class>
    


    <!-- http://purl.org/iot/vocab/m3-lite#WindDirection -->

    <owl:Class rdf:about="http://purl.org/iot/vocab/m3-lite#WindDirection">
        <rdfs:subClassOf rdf:resource="http://purl.org/NET/ssnx/qu/qu#QuantityKind"/>
        <rdfs:comment xml:lang="en">The geodetic azimuth of the direction from which the wind is blowing.</rdfs:comment>
        <rdfs:label xml:lang="en">Wind Direction</rdfs:label>
        <rdfs:seeAlso rdf:resource="http://paul.staroch.name/thesis/SmartHomeWeather.owl#DirectionalWind"/>
    </owl:Class>
    


    <!-- http://purl.org/iot/vocab/m3-lite#WindDirectionSensor -->

    <owl:Class rdf:about="http://purl.org/iot/vocab/m3-lite#WindDirectionSensor">
        <rdfs:subClassOf rdf:resource="http://purl.oclc.org/NET/ssnx/ssn#SensingDevice"/>
        <rdfs:subClassOf>
            <owl:Restriction>
                <owl:onProperty rdf:resource="http://purl.org/iot/vocab/m3-lite#hasDomainOfInterest"/>
                <owl:someValuesFrom rdf:resource="http://purl.org/iot/vocab/m3-lite#Weather"/>
            </owl:Restriction>
        </rdfs:subClassOf>
        <rdfs:comment xml:lang="en">Device used to detect wind direction.</rdfs:comment>
        <rdfs:label xml:lang="en">Wind Direction Sensor</rdfs:label>
    </owl:Class>
    


    <!-- http://purl.org/iot/vocab/m3-lite#WindSpeed -->

    <owl:Class rdf:about="http://purl.org/iot/vocab/m3-lite#WindSpeed">
        <rdfs:subClassOf rdf:resource="http://purl.org/NET/ssnx/qu/qu#QuantityKind"/>
        <rdfs:comment xml:lang="en">The ratio of the distance covered by moving air to the time quantity taken to cover it.</rdfs:comment>
        <rdfs:label xml:lang="en">Wind Velocity, Wind Speed</rdfs:label>
        <rdfs:seeAlso rdf:resource="http://openiot.eu/ontology/ns/WindSpeed"/>
    </owl:Class>
    


    <!-- http://purl.org/iot/vocab/m3-lite#WindSpeedSensor -->

    <owl:Class rdf:about="http://purl.org/iot/vocab/m3-lite#WindSpeedSensor">
        <rdfs:subClassOf rdf:resource="http://purl.org/iot/vocab/m3-lite#SpeedSensor"/>
        <rdfs:subClassOf>
            <owl:Restriction>
                <owl:onProperty rdf:resource="http://purl.org/iot/vocab/m3-lite#hasDomainOfInterest"/>
                <owl:someValuesFrom rdf:resource="http://purl.org/iot/vocab/m3-lite#Agriculture"/>
            </owl:Restriction>
        </rdfs:subClassOf>
        <rdfs:subClassOf>
            <owl:Restriction>
                <owl:onProperty rdf:resource="http://purl.org/iot/vocab/m3-lite#hasDomainOfInterest"/>
                <owl:someValuesFrom rdf:resource="http://purl.org/iot/vocab/m3-lite#Environment"/>
            </owl:Restriction>
        </rdfs:subClassOf>
        <rdfs:subClassOf>
            <owl:Restriction>
                <owl:onProperty rdf:resource="http://purl.org/iot/vocab/m3-lite#hasDomainOfInterest"/>
                <owl:someValuesFrom rdf:resource="http://purl.org/iot/vocab/m3-lite#Weather"/>
            </owl:Restriction>
        </rdfs:subClassOf>
        <rdfs:comment xml:lang="en">Wind Speed Sensor, Anemometer or Wind Velocity Sensor is used to measure the wind speed.</rdfs:comment>
        <rdfs:label xml:lang="en">Wind Speed Sensor</rdfs:label>
    </owl:Class>
    


    <!-- http://purl.org/iot/vocab/m3-lite#Window -->

    <owl:Class rdf:about="http://purl.org/iot/vocab/m3-lite#Window">
        <rdfs:subClassOf rdf:resource="http://purl.oclc.org/NET/UNIS/fiware/iot-lite#ActuatingDevice"/>
        <rdfs:subClassOf>
            <owl:Restriction>
                <owl:onProperty rdf:resource="http://purl.org/iot/vocab/m3-lite#hasDomainOfInterest"/>
                <owl:someValuesFrom rdf:resource="http://purl.org/iot/vocab/m3-lite#BuildingAutomation"/>
            </owl:Restriction>
        </rdfs:subClassOf>
        <rdfs:comment xml:lang="en">An actuator to automatically open/close the window.</rdfs:comment>
        <rdfs:label xml:lang="en">Window Actuating Device</rdfs:label>
    </owl:Class>
    


    <!-- http://purl.org/iot/vocab/m3-lite#WorkingState -->

    <owl:Class rdf:about="http://purl.org/iot/vocab/m3-lite#WorkingState">
        <rdfs:subClassOf rdf:resource="http://purl.org/NET/ssnx/qu/qu#QuantityKind"/>
        <rdfs:comment xml:lang="en">Indicator of whether a person (or object) is working or not</rdfs:comment>
        <rdfs:label xml:lang="en">Working State</rdfs:label>
    </owl:Class>
    


    <!-- http://purl.org/iot/vocab/m3-lite#WorkingStateDriver -->

    <owl:Class rdf:about="http://purl.org/iot/vocab/m3-lite#WorkingStateDriver">
        <rdfs:subClassOf rdf:resource="http://purl.org/iot/vocab/m3-lite#WorkingState"/>
        <rdfs:comment xml:lang="en">Indicator of whether the driver of a vehicle is present or not</rdfs:comment>
        <rdfs:label xml:lang="en">Working State Driver</rdfs:label>
    </owl:Class>
    


    <!-- http://purl.org/iot/vocab/m3-lite#WorkingStateDriver1 -->

    <owl:Class rdf:about="http://purl.org/iot/vocab/m3-lite#WorkingStateDriver1">
        <rdfs:subClassOf rdf:resource="http://purl.org/iot/vocab/m3-lite#WorkingStateDriver"/>
        <rdfs:comment>State of work of the first driver as defined in the FMS standard.</rdfs:comment>
        <rdfs:label xml:lang="en">Working State Driver 1</rdfs:label>
    </owl:Class>
    


    <!-- http://purl.org/iot/vocab/m3-lite#WorkingStateDriver2 -->

    <owl:Class rdf:about="http://purl.org/iot/vocab/m3-lite#WorkingStateDriver2">
        <rdfs:subClassOf rdf:resource="http://purl.org/iot/vocab/m3-lite#WorkingStateDriver"/>
        <rdfs:comment>State of work of the second driver as defined in the FMS standard.</rdfs:comment>
        <rdfs:label xml:lang="en">Working State Driver 2</rdfs:label>
    </owl:Class>
    


    <!-- http://purl.org/iot/vocab/m3-lite#Wout -->

    <owl:Class rdf:about="http://purl.org/iot/vocab/m3-lite#Wout">
        <rdfs:subClassOf rdf:resource="http://purl.org/NET/ssnx/qu/qu#Unit"/>
        <rdfs:comment xml:lang="en">This unit is used to measure delta dew point within the Com4Innov testbed. Natural number (W/out unit).</rdfs:comment>
        <rdfs:label xml:lang="en">W/out</rdfs:label>
    </owl:Class>
    


    <!-- http://purl.org/iot/vocab/m3-lite#Year -->

    <owl:Class rdf:about="http://purl.org/iot/vocab/m3-lite#Year">
        <rdfs:subClassOf rdf:resource="http://purl.org/iot/vocab/m3-lite#SecondTime"/>
        <rdfs:comment xml:lang="en">Year as a unit of time.</rdfs:comment>
        <rdfs:label xml:lang="en">Year</rdfs:label>
        <rdfs:seeAlso rdf:resource="http://sweet.jpl.nasa.gov/ontology/units.owl#year"/>
    </owl:Class>
    


    <!-- http://www.onem2m.org/ontology/Base_Ontology/base_ontology#Device -->

    <owl:Class rdf:about="http://www.onem2m.org/ontology/Base_Ontology/base_ontology#Device">
        <rdfs:comment>A Device (Class: Device) is a object designed to accomplish a particular task. A Device contains some logic and is producer and/or consumer of data that are exchanged via its Services with other oneM2M entities (Devices, Things) in the network. A Device may be a physical or non-physical entity.
In the context of oneM2M a Device is always assumed to be capable of communicating electronically via a network.
 - In order to accomplish its task, the device performs one or more functionalities 
 - These functionalities are exposed in the network as Services of the Device.
 - A Device can be composed of several (sub-) Devices 
 - Each Device (including sub-Devices) needs to be individually addressable in the network.</rdfs:comment>
        <rdfs:label xml:lang="en">Device</rdfs:label>
    </owl:Class>
    


    <!-- http://www.onem2m.org/ontology/Base_Ontology/base_ontology#MetaData -->

    <owl:Class rdf:about="http://www.onem2m.org/ontology/Base_Ontology/base_ontology#MetaData">
        <rdfs:comment>MetaData (Class: MetaData) contain data (like units, precision-ranges ) about a Variable or about an Aspect. 
E.g. the indoor temperature could have meta data: &quot;Degrees Celsius&quot;</rdfs:comment>
        <rdfs:label xml:lang="en">MetaData</rdfs:label>
    </owl:Class>
    


    <!-- http://www.onem2m.org/ontology/Base_Ontology/base_ontology#OperationOutput -->

    <owl:Class rdf:about="http://www.onem2m.org/ontology/Base_Ontology/base_ontology#OperationOutput">
        <rdfs:comment>OperationOutput (Class: OperationOutput) describes an output of an Operation. OperationOutput also describes the output of a Command. 
 - An Operation/Command may have multiple OperationInputs and/or OperationOutputs</rdfs:comment>
        <rdfs:label xml:lang="en">Operation Output</rdfs:label>
    </owl:Class>
    


    <!-- http://www.onem2m.org/ontology/Base_Ontology/base_ontology#Service -->

    <owl:Class rdf:about="http://www.onem2m.org/ontology/Base_Ontology/base_ontology#Service">
        <rdfs:comment rdf:resource="http://purl.oclc.org/NET/ssnx/ssn#Observation"/>
        <rdfs:comment>A Service (Class: Service) is a electronic representation of a Functionality in a network. The Service exposes the Functionality to the network and makes it discoverable, registerable and remotely controllable in the network. 
A Service is offered by a device that wants (a certain set of) its Functionalities to be discoverable, registerable, remotely controllable by other devices in the network. 
A Service can expose one or more Functionalities and a Functionality can be exposed by one or more Services.
The Input- and Output DataPoints and Operations of a Service may have the same names as for a different Service, however the Service to which they belong differentiates how they are addressed in the Device (e.g. via a port specific to the Service).
NOTE: While a Functionality  describes the  human understandable  meaning of a Service of the device the Service is used to describe how such functionality is represented in a communication network and can be accessed by electronic means. The Service and its Operations is therefore dependent on the technology of the network, hard- and software of the device.</rdfs:comment>
        <rdfs:label xml:lang="en">Service</rdfs:label>
    </owl:Class>
    


    <!-- http://www.onem2m.org/ontology/Base_Ontology/base_ontology#Thing -->

    <owl:Class rdf:about="http://www.onem2m.org/ontology/Base_Ontology/base_ontology#Thing">
        <rdfs:comment>A Thing in oneM2M  (Class: Thing) is an entity that can be identified in the oneM2M System. 
A Thing that is not a Device is not able to communicate electronically with its environment. However, the sub-class of Thing that is able to interact electronically is called a &quot;Device&quot;.
A Thing may have ThingProperties (Object Property: hasThingProperty). A Thing can have relations to other things (Object Property: hasThingRelation).
Since a Thing that is not a Device is not able to communicate electronically it cannot influence the value of its ThingProperties or being influenced by it. Similarly a Thing cannot document its - real-world - relationships (via hasThingRelation) to other Things.

E.g. A room that is modelled in oneM2M would be a Thing that could have a room-temperature as a ThingProperty and could have a relationship &quot;isAdjacentTo&quot; to another room</rdfs:comment>
        <rdfs:label xml:lang="en">Thing</rdfs:label>
    </owl:Class>
    


    <!-- http://www.onem2m.org/ontology/Base_Ontology/base_ontology#ThingProperty -->

    <owl:Class rdf:about="http://www.onem2m.org/ontology/Base_Ontology/base_ontology#ThingProperty">
        <rdfs:comment>A Value (Class: Value) denotes a property of a Thing. A Value can e.g. be observed or influenced by devices, or it constitutes static data about a Thing.
E.g. the indoor temperature of the room could be a Value of a Thing &quot;room&quot;.
A Value of a thing can concern a certain Aspect, e.g. the indoor temperature concerns the Aspect &quot;Temperature&quot; that could be measured by a temperature sensor.
A Value of a Thing can have meta data</rdfs:comment>
        <rdfs:label xml:lang="en">Thing Property</rdfs:label>
    </owl:Class>
    


    <!-- http://www.w3.org/2003/01/geo/wgs84_pos#Point -->

    <owl:Class rdf:about="http://www.w3.org/2003/01/geo/wgs84_pos#Point">
        <iot-lite:altRelative></iot-lite:altRelative>
        <iot-lite:relativeLocation></iot-lite:relativeLocation>
        <rdfs:label xml:lang="en">Point</rdfs:label>
        <geo:alt></geo:alt>
        <geo:lat></geo:lat>
        <geo:long></geo:long>
    </owl:Class>
    


    <!-- http://www.w3.org/2006/time#Instant -->

    <owl:Class rdf:about="http://www.w3.org/2006/time#Instant"/>
    


    <!-- 
    ///////////////////////////////////////////////////////////////////////////////////////
    //
    // Individuals
    //
    ///////////////////////////////////////////////////////////////////////////////////////
     -->

    


    <!-- http://purl.org/iot/ontology/fiesta-iot#WaterFlow01 -->

    <owl:NamedIndividual rdf:about="http://purl.org/iot/ontology/fiesta-iot#WaterFlow01">
        <rdf:type rdf:resource="http://purl.org/iot/ontology/fiesta-iot#Water_Flow"/>
        <ssn:madeObservation rdf:resource="http://purl.org/iot/ontology/fiesta-iot#WaterFlowObservation_01"/>
    </owl:NamedIndividual>
    


    <!-- http://purl.org/iot/ontology/fiesta-iot#WaterFlowObserValeu_01 -->

    <owl:NamedIndividual rdf:about="http://purl.org/iot/ontology/fiesta-iot#WaterFlowObserValeu_01">
        <rdf:type rdf:resource="http://purl.oclc.org/NET/ssnx/ssn#MeasurementProperty"/>
        <rdf:type rdf:resource="http://purl.oclc.org/NET/ssnx/ssn#ObservationValue"/>
        <dul:hasDataValue rdf:datatype="http://www.w3.org/2001/XMLSchema#double">2.0</dul:hasDataValue>
    </owl:NamedIndividual>
    


    <!-- http://purl.org/iot/ontology/fiesta-iot#WaterFlowObservation_01 -->

    <owl:NamedIndividual rdf:about="http://purl.org/iot/ontology/fiesta-iot#WaterFlowObservation_01">
        <rdf:type rdf:resource="http://purl.oclc.org/NET/ssnx/ssn#Observation"/>
        <ssn:observationResult rdf:resource="http://purl.org/iot/ontology/fiesta-iot#WaterFlow_SO_01"/>
    </owl:NamedIndividual>
    


    <!-- http://purl.org/iot/ontology/fiesta-iot#WaterFlow_SO_01 -->

    <owl:NamedIndividual rdf:about="http://purl.org/iot/ontology/fiesta-iot#WaterFlow_SO_01">
        <rdf:type rdf:resource="http://purl.oclc.org/NET/ssnx/ssn#SensorOutput"/>
        <ssn:hasValue rdf:resource="http://purl.org/iot/ontology/fiesta-iot#WaterFlowObserValeu_01"/>
    </owl:NamedIndividual>
    


    <!-- 
    ///////////////////////////////////////////////////////////////////////////////////////
    //
    // Rules
    //
    ///////////////////////////////////////////////////////////////////////////////////////
     -->

    <rdf:Description rdf:about="http://purl.org/iot/ontology/fiesta-iot#sensor">
        <rdf:type rdf:resource="http://www.w3.org/2003/11/swrl#Variable"/>
    </rdf:Description>
    <rdf:Description rdf:about="http://purl.org/iot/ontology/fiesta-iot#mdobserv">
        <rdf:type rdf:resource="http://www.w3.org/2003/11/swrl#Variable"/>
    </rdf:Description>
    <rdf:Description rdf:about="http://purl.org/iot/ontology/fiesta-iot#mdObservResult">
        <rdf:type rdf:resource="http://www.w3.org/2003/11/swrl#Variable"/>
    </rdf:Description>
    <rdf:Description rdf:about="http://purl.org/iot/ontology/fiesta-iot#outputSensor">
        <rdf:type rdf:resource="http://www.w3.org/2003/11/swrl#Variable"/>
    </rdf:Description>
    <rdf:Description rdf:about="http://purl.org/iot/ontology/fiesta-iot#value">
        <rdf:type rdf:resource="http://www.w3.org/2003/11/swrl#Variable"/>
    </rdf:Description>
    <rdf:Description>
        <swrla:isRuleEnabled rdf:datatype="http://www.w3.org/2001/XMLSchema#boolean">true</swrla:isRuleEnabled>
        <rdfs:comment rdf:datatype="http://www.w3.org/2001/XMLSchema#string"></rdfs:comment>
        <rdfs:label rdf:datatype="http://www.w3.org/2001/XMLSchema#string">S1</rdfs:label>
        <rdf:type rdf:resource="http://www.w3.org/2003/11/swrl#Imp"/>
        <swrl:body>
            <rdf:Description>
                <rdf:type rdf:resource="http://www.w3.org/2003/11/swrl#AtomList"/>
                <rdf:first>
                    <rdf:Description>
                        <rdf:type rdf:resource="http://www.w3.org/2003/11/swrl#ClassAtom"/>
                        <swrl:classPredicate rdf:resource="http://purl.org/iot/ontology/fiesta-iot#Water_Flow"/>
                        <swrl:argument1 rdf:resource="http://purl.org/iot/ontology/fiesta-iot#sensor"/>
                    </rdf:Description>
                </rdf:first>
                <rdf:rest>
                    <rdf:Description>
                        <rdf:type rdf:resource="http://www.w3.org/2003/11/swrl#AtomList"/>
                        <rdf:first>
                            <rdf:Description>
                                <rdf:type rdf:resource="http://www.w3.org/2003/11/swrl#IndividualPropertyAtom"/>
                                <swrl:propertyPredicate rdf:resource="http://purl.oclc.org/NET/ssnx/ssn#madeObservation"/>
                                <swrl:argument1 rdf:resource="http://purl.org/iot/ontology/fiesta-iot#sensor"/>
                                <swrl:argument2 rdf:resource="http://purl.org/iot/ontology/fiesta-iot#mdobserv"/>
                            </rdf:Description>
                        </rdf:first>
                        <rdf:rest>
                            <rdf:Description>
                                <rdf:type rdf:resource="http://www.w3.org/2003/11/swrl#AtomList"/>
                                <rdf:first>
                                    <rdf:Description>
                                        <rdf:type rdf:resource="http://www.w3.org/2003/11/swrl#IndividualPropertyAtom"/>
                                        <swrl:propertyPredicate rdf:resource="http://purl.oclc.org/NET/ssnx/ssn#observationResult"/>
                                        <swrl:argument1 rdf:resource="http://purl.org/iot/ontology/fiesta-iot#mdobserv"/>
                                        <swrl:argument2 rdf:resource="http://purl.org/iot/ontology/fiesta-iot#mdObservResult"/>
                                    </rdf:Description>
                                </rdf:first>
                                <rdf:rest>
                                    <rdf:Description>
                                        <rdf:type rdf:resource="http://www.w3.org/2003/11/swrl#AtomList"/>
                                        <rdf:first>
                                            <rdf:Description>
                                                <rdf:type rdf:resource="http://www.w3.org/2003/11/swrl#IndividualPropertyAtom"/>
                                                <swrl:propertyPredicate rdf:resource="http://purl.oclc.org/NET/ssnx/ssn#hasValue"/>
                                                <swrl:argument1 rdf:resource="http://purl.org/iot/ontology/fiesta-iot#mdObservResult"/>
                                                <swrl:argument2 rdf:resource="http://purl.org/iot/ontology/fiesta-iot#outputSensor"/>
                                            </rdf:Description>
                                        </rdf:first>
                                        <rdf:rest>
                                            <rdf:Description>
                                                <rdf:type rdf:resource="http://www.w3.org/2003/11/swrl#AtomList"/>
                                                <rdf:first>
                                                    <rdf:Description>
                                                        <rdf:type rdf:resource="http://www.w3.org/2003/11/swrl#DatavaluedPropertyAtom"/>
                                                        <swrl:propertyPredicate rdf:resource="http://www.loa.istc.cnr.it/ontologies/DUL.owl#hasDataValue"/>
                                                        <swrl:argument1 rdf:resource="http://purl.org/iot/ontology/fiesta-iot#outputSensor"/>
                                                        <swrl:argument2 rdf:resource="http://purl.org/iot/ontology/fiesta-iot#value"/>
                                                    </rdf:Description>
                                                </rdf:first>
                                                <rdf:rest>
                                                    <rdf:Description>
                                                        <rdf:type rdf:resource="http://www.w3.org/2003/11/swrl#AtomList"/>
                                                        <rdf:first>
                                                            <rdf:Description>
                                                                <rdf:type rdf:resource="http://www.w3.org/2003/11/swrl#BuiltinAtom"/>
                                                                <swrl:builtin rdf:resource="http://www.w3.org/2003/11/swrlb#greaterThan"/>
                                                                <swrl:arguments>
                                                                    <rdf:Description>
                                                                        <rdf:type rdf:resource="http://www.w3.org/1999/02/22-rdf-syntax-ns#List"/>
                                                                        <rdf:first rdf:resource="http://purl.org/iot/ontology/fiesta-iot#value"/>
                                                                        <rdf:rest>
                                                                            <rdf:Description>
                                                                                <rdf:type rdf:resource="http://www.w3.org/1999/02/22-rdf-syntax-ns#List"/>
                                                                                <rdf:first rdf:datatype="http://www.w3.org/2001/XMLSchema#integer">0</rdf:first>
                                                                                <rdf:rest rdf:resource="http://www.w3.org/1999/02/22-rdf-syntax-ns#nil"/>
                                                                            </rdf:Description>
                                                                        </rdf:rest>
                                                                    </rdf:Description>
                                                                </swrl:arguments>
                                                            </rdf:Description>
                                                        </rdf:first>
                                                        <rdf:rest rdf:resource="http://www.w3.org/1999/02/22-rdf-syntax-ns#nil"/>
                                                    </rdf:Description>
                                                </rdf:rest>
                                            </rdf:Description>
                                        </rdf:rest>
                                    </rdf:Description>
                                </rdf:rest>
                            </rdf:Description>
                        </rdf:rest>
                    </rdf:Description>
                </rdf:rest>
            </rdf:Description>
        </swrl:body>
        <swrl:head>
            <rdf:Description>
                <rdf:type rdf:resource="http://www.w3.org/2003/11/swrl#AtomList"/>
                <rdf:first>
                    <rdf:Description>
                        <rdf:type rdf:resource="http://www.w3.org/2003/11/swrl#DatavaluedPropertyAtom"/>
                        <swrl:propertyPredicate rdf:resource="http://purl.org/iot/ontology/fiesta-iot#hasWaterFlow"/>
                        <swrl:argument1 rdf:resource="http://purl.org/iot/ontology/fiesta-iot#sensor"/>
                        <swrl:argument2 rdf:datatype="http://www.w3.org/2001/XMLSchema#boolean">true</swrl:argument2>
                    </rdf:Description>
                </rdf:first>
                <rdf:rest rdf:resource="http://www.w3.org/1999/02/22-rdf-syntax-ns#nil"/>
            </rdf:Description>
        </swrl:head>
    </rdf:Description>
</rdf:RDF>



<!-- Generated by the OWL API (version 4.2.8.20170104-2310) https://github.com/owlcs/owlapi -->

